@base          <http://www.semanticweb.org/sveta/ontologies/2019/11/allotment_ontology#> .
@prefix :      <http://www.semanticweb.org/sveta/ontologies/2019/11/allotman_ontology> .
@prefix schema: <http://schema.org/> .
@prefix owl:   <http://www.w3.org/2002/07/owl#> .
@prefix ns:    <http://www.w3.org/2006/vcard/ns#> .
@prefix xsd:   <http://www.w3.org/2001/XMLSchema#> .
@prefix skos:  <http://www.w3.org/2004/02/skos/core#> .
@prefix rdfs:  <http://www.w3.org/2000/01/rdf-schema#> .
@prefix ns2:   <http://www.w3.org/2003/06/sw-vocab-status/ns#> .
@prefix ns1:   <http://purl.org/acco/ns#> .
@prefix pcd:   <http://purl.org/procurement/public-contracts-datatypes#> .
@prefix terms: <http://purl.org/dc/terms/> .
@prefix xml:   <http://www.w3.org/XML/1998/namespace> .
@prefix public-contracts: <http://purl.org/procurement/public-contracts#> .
@prefix pproc: <http://contsem.unizar.es/def/sector-publico/pproc#> .
@prefix dcterms: <http://purl.org/dc/terms/> .
@prefix vann:  <http://purl.org/vocab/vann/> .
@prefix wot:   <http://xmlns.com/wot/0.1/> .
@prefix foaf:  <http://xmlns.com/foaf/0.1/> .
@prefix acco:  <http://purl.org/acco/ns#> .
@prefix org:   <http://www.w3.org/ns/org#> .
@prefix cpv:   <http://purl.org/cpv/2008/> .
@prefix gr:    <http://purl.org/goodrelations/v1#> .
@prefix dc11:  <http://purl.org/dc/elements/1.1/> .
@prefix s:     <http://schema.org/> .
@prefix pc:    <http://purl.org/procurement/public-contracts#> .
@prefix allotment_ontology: <http://www.semanticweb.org/sveta/ontologies/2019/11/allotment_ontology#> .
@prefix rdf:   <http://www.w3.org/1999/02/22-rdf-syntax-ns#> .
@prefix v1:    <http://purl.org/goodrelations/v1#> .
@prefix ethon: <http://ethon.consensys.net/> .
@prefix dc:    <http://purl.org/dc/elements/1.1/> .

allotment_ontology:Included_Object_1
        a                        v1:TypeAndQuantityNode , owl:NamedIndividual ;
        v1:amountOfThisGood      "1.0"^^xsd:float ;
        v1:hasUnitOfMeasurement  "DAY" ;
        v1:typeOfGood            allotment_ontology:Room_101 .

allotment_ontology:blockchain_contract
        a                   owl:ObjectProperty ;
        rdfs:domain         pc:Contract ;
        rdfs:label          "blockchain contract" ;
        rdfs:range          ethon:ContractAccount ;
        rdfs:subPropertyOf  owl:topObjectProperty .

allotment_ontology:Date_of_signing
        a                   owl:DatatypeProperty ;
        rdfs:domain         pc:Contract ;
        rdfs:range          xsd:date ;
        rdfs:subPropertyOf  dcterms:date .

allotment_ontology:Room_101
        a                     owl:NamedIndividual , acco:HotelRoom ;
        ethon:partOf          allotment_ontology:Hotel_1 ;
        acco:bed              acco:Double , acco:Single , allotment_ontology:Bd1 ;
        acco:includedFeature  allotment_ontology:Safe , allotment_ontology:Balkon ;
        v1:description        "Room with one double and one single beds and a balcony." ;
        v1:name               "101" .

allotment_ontology:Hotel_2
        a       owl:NamedIndividual .

allotment_ontology:Employee_A
        a                         s:Person , owl:NamedIndividual ;
        s:affiliation             allotment_ontology:Agencija ;
        s:worksFor                allotment_ontology:Agencija ;
        allotment_ontology:signs  allotment_ontology:Ugovor_1 ;
        foaf:familyName           "Peric" ;
        foaf:givenName            "Pera" .

allotment_ontology:ContractEconomicConditions_1
        a                              pproc:ContractEconomicConditions ;
        pproc:estimatedValue           [ a                    pproc:BundlePriceSpecification ;
                                         v1:hasCurrency       "WEI" ;
                                         v1:hasCurrencyValue  "6040.0"^^xsd:float
                                       ] ;
        allotment_ontology:Advance_payment
                [ a                    v1:PaymentChargeSpecification ;
                  v1:hasCurrency       "WEI" ;
                  v1:hasCurrencyValue  "20"^^xsd:float
                ] ;
        allotment_ontology:Charge_fee  [ a                    v1:PriceSpecification ;
                                         v1:hasCurrency       "WEI" ;
                                         v1:hasCurrencyValue  "7"^^xsd:float
                                       ] ;
        allotment_ontology:Full_board_price
                [ a                    v1:UnitPriceSpecification ;
                  v1:hasCurrency       "WEI" ;
                  v1:hasCurrencyValue  "25"^^xsd:float
                ] ;
        allotment_ontology:Half_board_price
                [ a                    v1:UnitPriceSpecification ;
                  v1:hasCurrency       "WEI" ;
                  v1:hasCurrencyValue  "15"^^xsd:float
                ] ;
        allotment_ontology:Kids_price  [ a                    v1:UnitPriceSpecification ;
                                         v1:hasCurrency       "WEI" ;
                                         v1:hasCurrencyValue  "10"^^xsd:float
                                       ] ;
        allotment_ontology:Offseason_price
                [ a                    v1:UnitPriceSpecification ;
                  v1:hasCurrency       "WEI" ;
                  v1:hasCurrencyValue  "12"^^xsd:float
                ] .

allotment_ontology:Organizacija_3
        a             allotment_ontology:AccommodationOrg ;
        v1:legalName  "Park org" ;
        v1:owns       allotment_ontology:Smestaj_5 , allotment_ontology:Smestaj_4 ;
        s:address     allotment_ontology:Adresa_3 .

allotment_ontology:CEC
        a       pproc:ContractEconomicConditions , owl:NamedIndividual ;
        allotment_ontology:Advance_payment
                allotment_ontology:PFee_1 .

allotment_ontology:ContractingParty
        a       owl:Class .

allotment_ontology:Court
        a       owl:Class .

allotment_ontology:Full_board_price
        a                   owl:ObjectProperty ;
        rdfs:domain         pproc:ContractEconomicConditions ;
        rdfs:range          v1:UnitPriceSpecification ;
        rdfs:subPropertyOf  pproc:price .

allotment_ontology:location_of_signing
        a            owl:DatatypeProperty ;
        rdfs:domain  pc:Contract ;
        rdfs:range   xsd:string .

ethon:ContractAccount
        a       owl:Class .

allotment_ontology:Smestaj_4
        a          acco:Accommodation ;
        s:address  allotment_ontology:Adresa_h_4 ;
        s:name     "Vila Park" .

allotment_ontology:Adresa_2
        a                  s:PostalAddress ;
        s:addressCountry   "Srbija" ;
        s:addressLocality  "Novi Sad" ;
        s:streetAddress    "Fruskogorska 30" .

allotment_ontology:Zaposleni_5
        a                s:Person ;
        s:worksFor       allotment_ontology:Organizacija_3 ;
        ns:email         "jovica@gmail.com" ;
        ns:tel           "064/412-353" ;
        ns:title         "Sluzbenik" ;
        foaf:familyName  "Jovic" ;
        foaf:givenName   "Jovica" .

acco:Single  a            owl:NamedIndividual , acco:BedType ;
        rdfs:comment      "A single bed. The actual dimension may vary by country, see http://en.wikipedia.org/wiki/Bed_size."@en ;
        rdfs:isDefinedBy  acco: ;
        rdfs:label        "Single or twin bed (acco:BedType)"@en .

allotment_ontology:Javni_ugovor_1
        a       pproc:Contract , owl:NamedIndividual ;
        allotment_ontology:blockchain_contract
                allotment_ontology:Blockchain_contract_1 .

allotment_ontology:Offseason_price
        a                   owl:ObjectProperty ;
        rdfs:domain         pproc:ContractEconomicConditions ;
        rdfs:range          v1:UnitPriceSpecification ;
        rdfs:subPropertyOf  pproc:price .

allotment_ontology:Agencija
        a          allotment_ontology:Agency , owl:NamedIndividual ;
        v1:offers  allotment_ontology:Ponuda .

allotment_ontology:ContractAdditionalObligations_1
        a                              pproc:ContractAdditionalObligations ;
        pproc:finalFinancialGuarantee  "5.0"^^xsd:float ;
        allotment_ontology:informing_period
                "10"^^xsd:int ;
        allotment_ontology:withdrawal_period
                "7"^^xsd:int .

allotment_ontology:informing_period
        a                   owl:DatatypeProperty ;
        rdfs:domain         pproc:ContractAdditionalObligations ;
        rdfs:range          xsd:int ;
        rdfs:subPropertyOf  owl:topDataProperty .

allotment_ontology:Ugostitelj
        a             allotment_ontology:AccommodationOrg , owl:NamedIndividual ;
        v1:legalName  "Org ltd." ;
        v1:name       "Org 1" ;
        v1:owns       allotment_ontology:Hotel_1 ;
        s:employees   allotment_ontology:Employee_U , allotment_ontology:Employee_A ;
        ns:adr        allotment_ontology:Adresa_Org_1 .

allotment_ontology:Advance_payment
        a                   owl:ObjectProperty ;
        rdfs:domain         pproc:ContractEconomicConditions ;
        rdfs:range          v1:PaymentChargeSpecification ;
        rdfs:subPropertyOf  pproc:feePrice .

allotment_ontology:Hotel_1
        a                     v1:Individual , acco:Hotel , owl:NamedIndividual ;
        acco:includedFeature  allotment_ontology:Wi-fi , allotment_ontology:Pool ;
        v1:description        "Description of a hotel.\nIn a multiline text." ;
        v1:name               "Nice name for a hotel" .

allotment_ontology:Bd1
        a               acco:BedDetails , owl:NamedIndividual ;
        acco:quantity   2 ;
        acco:typeOfBed  acco:Double .

<>      a            owl:Ontology ;
        owl:imports  foaf: , <http://www.w3.org/2006/vcard/ns> , <http://purl.org/goodrelations/v1> , acco: , <http://ethon.consensys.net/v0/> , pproc: .

allotment_ontology:Organizacija_2
        a             allotment_ontology:AccommodationOrg ;
        v1:legalName  "Lims" ;
        v1:owns       allotment_ontology:Smestaj_3 , allotment_ontology:Smestaj_2 , allotment_ontology:Smestaj_1 ;
        s:address     allotment_ontology:Adresa_2 .

allotment_ontology:Ponuda
        a                         v1:Offering , owl:NamedIndividual ;
        v1:availabilityEnds       "2020-01-15T00:00:00Z"^^xsd:dateTime ;
        v1:availabilityStarts     "2019-12-15T00:00:00Z"^^xsd:dateTime ;
        v1:description            "Offering for hotel 1"^^rdfs:Literal ;
        v1:hasBusinessFunction    v1:LeaseOut ;
        v1:hasPriceSpecification  allotment_ontology:Price_spec ;
        v1:includesObject         allotment_ontology:Included_Object_1 ;
        v1:name                   "Sample offer"^^rdfs:Literal .

allotment_ontology:Zaposleni_4
        a                s:Person ;
        s:worksFor       allotment_ontology:Organizacija_3 ;
        ns:email         "jova@gmail.com" ;
        ns:tel           "068/987-65-43" ;
        ns:title         "Sluzbenik" ;
        foaf:familyName  "Jovanovic" ;
        foaf:givenName   "Jovan" .

allotment_ontology:Adresa_h_5
        a                  s:PostalAddress ;
        s:addressCountry   "Srbija" ;
        s:addressLocality  "Novi Sad" ;
        s:streetAddress    "Novosadskog sajma 35" .

allotment_ontology:Smestaj_3
        a          acco:Accommodation ;
        s:address  allotment_ontology:Adresa_h_3 ;
        s:name     "Hotel Garden" .

allotment_ontology:Adresa_1
        a                  s:PostalAddress ;
        s:addressCountry   "Srbija" ;
        s:addressLocality  "Novi Sad" ;
        s:streetAddress    "Bulevar Oslobođenja 30" .

allotment_ontology:signs
        a            owl:ObjectProperty ;
        rdfs:domain  s:Person ;
        rdfs:range   pc:Contract .

allotment_ontology:beds
        a            owl:DatatypeProperty ;
        rdfs:domain  acco:BedDetails ;
        rdfs:range   xsd:int .

allotment_ontology:PFee_1
        a                    v1:PaymentChargeSpecification , owl:NamedIndividual ;
        v1:hasCurrencyValue  "100.0"^^xsd:float .

v1:LeaseOut  a            owl:NamedIndividual , v1:BusinessFunction ;
        rdfs:comment      "This gr:BusinessFunction indicates that the gr:BusinessEntity offers (or seeks) the temporary right to use the specified gr:ProductOrService."@en ;
        rdfs:isDefinedBy  <http://purl.org/goodrelations/v1> ;
        rdfs:label        "Lease Out (business function)"@en .

allotment_ontology:withdrawal_period
        a                   owl:DatatypeProperty ;
        rdfs:domain         pproc:ContractAdditionalObligations ;
        rdfs:range          xsd:int ;
        rdfs:subPropertyOf  owl:topDataProperty .

allotment_ontology:Price_spec
        a                    v1:PriceSpecification , owl:NamedIndividual ;
        v1:hasCurrency       "EUR" ;
        v1:hasCurrencyValue  "500.0"^^xsd:float .

allotment_ontology:Balkon
        a         acco:AccommodationFeature , owl:NamedIndividual ;
        v1:name   "Balkon 101" ;
        ns:value  "yes" .

allotment_ontology:contracting_party
        a                   owl:ObjectProperty ;
        rdfs:domain         pproc:Contract ;
        rdfs:range          s:Organization ;
        rdfs:subPropertyOf  owl:topObjectProperty .

allotment_ontology:Rooms_configuration
        a                   owl:ObjectProperty ;
        rdfs:domain         v1:Offering ;
        rdfs:label          "rooms configuration (0..*)" ;
        rdfs:range          acco:BedDetails ;
        rdfs:subPropertyOf  owl:topObjectProperty .

allotment_ontology:Nalog_ugovora_1
        a              ethon:ContractAccount ;
        ethon:address  "0x07a457d878bf363e0bb5aa0b096092f941e19962"^^xsd:hexBinary .

ethon:partOf  a  owl:AnnotationProperty .

pproc:finalFinancialGuarantee
        a             owl:DatatypeProperty , owl:FunctionalProperty ;
        rdfs:comment  "El rango en esta propiedad indica un porcentaje, por lo que el rango del número real a utilizar debe estar comprendido entre 0.0 y 100.0."@es , "The range of this property must be a percentage (i.e. float between 0.0 and 100.0)"@en ;
        rdfs:domain   pproc:ContractAdditionalObligations ;
        rdfs:label    "Garantía definitiva"@es , "Final financial guarantee"@en ;
        rdfs:range    xsd:float .

allotment_ontology:ContractingPartyAgency
        a                owl:Class ;
        rdfs:subClassOf  allotment_ontology:ContractingParty .

allotment_ontology:ContractTemporalConditions_1
        a                       pproc:ContractTemporalConditions ;
        pproc:estimatedEndDate  "2021-11-30T11:00:00Z"^^xsd:dateTime ;
        allotment_ontology:Actual_start_date
                "2021-02-01T11:00:00Z"^^xsd:dateTime ;
        allotment_ontology:Main_season_end_date
                "2021-08-31T10:00:00Z"^^xsd:dateTime ;
        allotment_ontology:Main_season_start_date
                "2021-06-01T10:00:00Z"^^xsd:dateTime .

allotment_ontology:Organizacija_1
        a             allotment_ontology:Agency ;
        v1:legalName  "Sabra" ;
        s:address     allotment_ontology:Adresa_1 .

allotment_ontology:AccommodationOrg
        a                 owl:Class ;
        rdfs:subClassOf   s:Organization ;
        owl:disjointWith  allotment_ontology:Agency .

allotment_ontology:Kids_price
        a                   owl:ObjectProperty ;
        rdfs:domain         pproc:ContractEconomicConditions ;
        rdfs:range          v1:UnitPriceSpecification ;
        rdfs:subPropertyOf  pproc:price .

allotment_ontology:Smestaj_2
        a          acco:Accommodation ;
        s:address  allotment_ontology:Adresa_h_2 ;
        s:name     "Prezident Hotel" .

allotment_ontology:Offering_1
        a                       v1:Offering ;
        v1:hasEligibleQuantity  [ a                        v1:QuantitativeValue ;
                                  v1:hasUnitOfMeasurement  "C62" ;
                                  v1:hasValue              "20"^^xsd:int
                                ] ;
        v1:includesObject       allotment_ontology:Smestaj_5 , allotment_ontology:Smestaj_4 ;
        allotment_ontology:Rooms_configuration
                allotment_ontology:BedDetails_1_3 , allotment_ontology:BedDetails_1_2 , allotment_ontology:BedDetails_1_1 .

allotment_ontology:Adresa_h_4
        a                  s:PostalAddress ;
        s:addressCountry   "Srbija" ;
        s:addressLocality  "Subotica" ;
        s:streetAddress    "Nikole Tesle 1" .

allotment_ontology:Zaposleni_3
        a                s:Person ;
        s:worksFor       allotment_ontology:Organizacija_2 ;
        ns:email         "mika@yahoo.com" ;
        ns:tel           "068/987-65-43" ;
        ns:title         "Sluzbenik" ;
        foaf:familyName  "Mikic" ;
        foaf:givenName   "Miroslav" .

allotment_ontology:Contract_object
        a                pproc:ContractObject , owl:NamedIndividual ;
        pproc:provision  allotment_ontology:Ponuda .

allotment_ontology:Actual_start_date
        a                   owl:DatatypeProperty ;
        rdfs:domain         pproc:ContractTemporalConditions ;
        rdfs:range          xsd:dateTime ;
        rdfs:subPropertyOf  dcterms:date .

allotment_ontology:Contract_object_1
        a                pproc:ContractObject ;
        pproc:provision  allotment_ontology:Offering_1 .

<#Ugovor/1>  a                        pproc:Contract ;
        pproc:contractAdditionalObligations
                allotment_ontology:ContractAdditionalObligations_1 ;
        pproc:contractEconomicConditions
                allotment_ontology:ContractEconomicConditions_1 ;
        pproc:contractObject          allotment_ontology:Contract_object_1 ;
        pproc:contractTemporalConditions
                allotment_ontology:ContractTemporalConditions_1 ;
        pproc:legalDocumentReference  allotment_ontology:Zakon_o_obligacionim_odnosima ;
        allotment_ontology:Date_of_signing
                "2020-09-08T08:30:00.411Z"^^xsd:dateTime ;
        allotment_ontology:blockchain_contract
                allotment_ontology:Nalog_ugovora_1 ;
        allotment_ontology:contracting_party_accomodation
                allotment_ontology:Organizacija_3 ;
        allotment_ontology:contracting_party_agency
                allotment_ontology:Organizacija_1 ;
        allotment_ontology:jurisdiction
                allotment_ontology:Osnovni_sud_Novi_Sad ;
        allotment_ontology:signatory_accomodation
                allotment_ontology:Zaposleni_5 ;
        allotment_ontology:signatory_agency
                allotment_ontology:Zaposleni_1 .

allotment_ontology:Wi-fi
        a               acco:AccommodationFeature , owl:NamedIndividual ;
        v1:description  "Wi-fi internet connection is not avaliable in all hotel facilitites." ;
        v1:name         "Wi-fi internet connection" ;
        ns:value        "no" .

allotment_ontology:Employee_U
        a                         s:Person , owl:NamedIndividual ;
        allotment_ontology:signs  allotment_ontology:Ugovor_1 ;
        foaf:familyName           "Mikic" ;
        foaf:givenName            "MIka" .

allotment_ontology:Ugovor
        a       ethon:ContractAccount , owl:NamedIndividual .

allotment_ontology:jurisdiction
        a                   owl:ObjectProperty ;
        rdfs:domain         pproc:Contract ;
        rdfs:range          allotment_ontology:Court ;
        rdfs:subPropertyOf  owl:topObjectProperty .

allotment_ontology:Main_season_end_date
        a                   owl:DatatypeProperty ;
        rdfs:domain         pproc:ContractTemporalConditions ;
        rdfs:range          xsd:date ;
        rdfs:subPropertyOf  dcterms:date .

allotment_ontology:signatory_agency
        a                   owl:ObjectProperty ;
        rdfs:domain         pproc:Contract ;
        rdfs:range          s:Person ;
        rdfs:subPropertyOf  allotment_ontology:signatory .

allotment_ontology:Agency
        a                owl:Class ;
        rdfs:subClassOf  s:Organization .

s:employees  a  owl:ObjectProperty .

allotment_ontology:BedDetails_1_3
        a                        acco:BedDetails ;
        acco:quantity            3 ;
        allotment_ontology:beds  "3"^^xsd:int .

allotment_ontology:Smestaj_1
        a          acco:Accommodation ;
        s:address  allotment_ontology:Adresa_h_1 ;
        s:name     "Hotel Fontana" .

allotment_ontology:Adresa_h_3
        a                  s:PostalAddress ;
        s:addressCountry   "Srbija" ;
        s:addressLocality  "Novi Sad" ;
        s:streetAddress    "Primorska 50" .

allotment_ontology:Zaposleni_2
        a                s:Person ;
        s:worksFor       allotment_ontology:Organizacija_1 ;
        ns:email         "perica@gmail.com" ;
        ns:tel           "061/123-45-67" ;
        ns:title         "Sluzbenik" ;
        foaf:familyName  "Peric" ;
        foaf:givenName   "Perica" .

allotment_ontology:Safe
        a         acco:AccommodationFeature , owl:NamedIndividual ;
        v1:name   "Safe 101" ;
        ns:value  "yes" .

acco:Double  a            owl:NamedIndividual , acco:BedType ;
        rdfs:comment      "A double bed. The actual dimension may vary by country, see http://en.wikipedia.org/wiki/Bed_size."@en ;
        rdfs:isDefinedBy  acco: ;
        rdfs:label        "Double or full bed (acco:BedType)"@en .

s:worksFor  a   owl:ObjectProperty .

allotment_ontology:Adresa_Org_1
        a                  ns:Address , owl:NamedIndividual ;
        ns:country-name    "Serbia" ;
        ns:locality        "Novi Sad" ;
        ns:postal-code     "21000" ;
        ns:street-address  "Bulevar Oslobodjenja bb" .

allotment_ontology:BedDetails_1_2
        a                        acco:BedDetails ;
        acco:quantity            2 ;
        allotment_ontology:beds  "4"^^xsd:int .

allotment_ontology:Charge_fee
        a                   owl:ObjectProperty ;
        rdfs:domain         pproc:ContractEconomicConditions ;
        rdfs:range          v1:PriceSpecification ;
        rdfs:subPropertyOf  pproc:feePrice .

allotment_ontology:contracting_party_accomodation
        a                         owl:ObjectProperty ;
        rdfs:domain               pproc:Contract ;
        rdfs:range                allotment_ontology:AccommodationOrg ;
        rdfs:subPropertyOf        allotment_ontology:contracting_party ;
        owl:propertyDisjointWith  allotment_ontology:contracting_party_agency .

allotment_ontology:Adresa_4
        a                  s:PostalAddress ;
        s:addressCountry   "Srbija" ;
        s:addressLocality  "Novi Sad" ;
        s:streetAddress    "Grčkoškolska 10" .

allotment_ontology:Ugovor_1
        a                 pproc:LeaseContract , owl:NamedIndividual ;
        pc:actualEndDate  "2020-01-25"^^xsd:date ;
        allotment_ontology:Actual_start_date
                "2019-12-25"^^xsd:date ;
        allotment_ontology:Date_of_signing
                "2019-12-19"^^xsd:date ;
        allotment_ontology:location_of_signing
                "Novi Sad" .

allotment_ontology:ContractingPartyAccomodation
        a                 owl:Class ;
        rdfs:subClassOf   allotment_ontology:ContractingParty ;
        owl:disjointWith  allotment_ontology:ContractingPartyAgency .

allotment_ontology:Zakon_o_obligacionim_odnosima
        a       allotment_ontology:Law .

allotment_ontology:Adresa_h_2
        a                  s:PostalAddress ;
        s:addressCountry   "Srbija" ;
        s:addressLocality  "Novi Sad" ;
        s:streetAddress    "Futoška 109" .

allotment_ontology:Zaposleni_1
        a                s:Person ;
        s:worksFor       allotment_ontology:Organizacija_1 ;
        ns:email         "pera@gmail.com" ;
        ns:tel           "061/123-45-67" ;
        ns:title         "Sluzbenik" ;
        foaf:familyName  "Petrovic" ;
        foaf:givenName   "Petar" .

allotment_ontology:Blockchain_contract_1
        a              ethon:ContractAccount , owl:NamedIndividual ;
        ethon:address  "07a457d878bf363e0bb5aa0b096092f941e19962"^^xsd:hexBinary .

pproc:estimatedEndDate
        a                   owl:DatatypeProperty , owl:FunctionalProperty ;
        rdfs:domain         [ a            owl:Class ;
                              owl:unionOf  ( pproc:ContractTemporalConditions pproc:FrameworkAgreement pproc:InformationProvider v1:Offering )
                            ] ;
        rdfs:label          "Fecha estimada de finalización"@es , "Estimated end date"@en ;
        rdfs:range          xsd:date ;
        rdfs:subPropertyOf  dcterms:date .

allotment_ontology:Main_season_start_date
        a                   owl:DatatypeProperty ;
        rdfs:domain         pproc:ContractTemporalConditions ;
        rdfs:range          xsd:date ;
        rdfs:subPropertyOf  dcterms:date .

allotment_ontology:signatory_accomodation
        a                         owl:ObjectProperty ;
        rdfs:domain               pproc:Contract ;
        rdfs:range                s:Person ;
        rdfs:subPropertyOf        allotment_ontology:signatory ;
        owl:propertyDisjointWith  allotment_ontology:signatory_agency .

allotment_ontology:contracting_party_agency
        a                   owl:ObjectProperty ;
        rdfs:domain         pproc:Contract ;
        rdfs:range          allotment_ontology:Agency ;
        rdfs:subPropertyOf  allotment_ontology:contracting_party .

allotment_ontology:Organizacija_4
        a             allotment_ontology:Agency ;
        v1:legalName  "Kon Tiki Travel" ;
        s:address     allotment_ontology:Adresa_4 .

allotment_ontology:BedDetails_1_1
        a                        acco:BedDetails ;
        acco:quantity            1 ;
        allotment_ontology:beds  "3"^^xsd:int .

allotment_ontology:Pool
        a         acco:AccommodationFeature , owl:NamedIndividual ;
        v1:name   "Swimming pool" ;
        ns:value  "yes" .

allotment_ontology:signatory
        a                   owl:ObjectProperty ;
        rdfs:domain         pproc:Contract ;
        rdfs:range          s:Person ;
        rdfs:subPropertyOf  owl:topObjectProperty .

allotment_ontology:Osnovni_sud_Novi_Sad
        a       allotment_ontology:Court .

allotment_ontology:Law
        a       owl:Class .

allotment_ontology:Smestaj_5
        a          acco:Accommodation ;
        s:address  allotment_ontology:Adresa_h_5 ;
        s:name     "Hotel Park" .

allotment_ontology:Adresa_3
        a                  s:PostalAddress ;
        s:addressCountry   "Srbija" ;
        s:addressLocality  "Novi Sad" ;
        s:streetAddress    "Fruskogorska 20" .

allotment_ontology:Zaposleni_6
        a                s:Person ;
        s:worksFor       allotment_ontology:Organizacija_4 ;
        ns:email         "kontiki@gmail.com" ;
        ns:tel           "064/412-353" ;
        ns:title         "Sluzbenik" ;
        foaf:familyName  "Trajkovic" ;
        foaf:givenName   "Kristijan" .

s:affiliation  a  owl:ObjectProperty .

foaf:family_name  a         owl:DatatypeProperty , rdf:Property ;
        rdfs:comment        "The family name of some person." ;
        rdfs:domain         foaf:Person ;
        rdfs:isDefinedBy    foaf: ;
        rdfs:label          "family_name" ;
        rdfs:range          rdfs:Literal ;
        rdfs:subPropertyOf  foaf:familyName ;
        ns2:term_status     "archaic" .

allotment_ontology:Half_board_price
        a                   owl:ObjectProperty ;
        rdfs:domain         pproc:ContractEconomicConditions ;
        rdfs:range          v1:UnitPriceSpecification ;
        rdfs:subPropertyOf  pproc:price .

allotment_ontology:Adresa_h_1
        a                  s:PostalAddress ;
        s:addressCountry   "Srbija" ;
        s:addressLocality  "Novi Sad" ;
        s:streetAddress    "Nikole Pašića 27" .

v1:eligibleDuration  a    owl:ObjectProperty ;
        rdfs:comment      "The minimal and maximal duration for which the given gr:Offering or gr:License is valid. This is mostly used for offers regarding accommodation, the rental of objects, or software licenses. The duration is specified by attaching an instance of gr:QuantitativeValue. The lower and upper boundaries are specified using the properties gr:hasMinValue and gr:hasMaxValue to that instance. If they are the same, use the gr:hasValue property. The unit of measurement is specified using the property gr:hasUnitOfMeasurement with a string holding a UN/CEFACT code suitable for durations, e.g. MON (months), DAY (days), HUR (hours), or MIN (minutes).\n\nThe difference to the gr:validFrom and gr:validThrough properties is that those specify the absiolute interval during which the gr:Offering or gr:License is valid, while gr:eligibleDuration specifies the acceptable duration of the contract or usage."@en ;
        rdfs:domain       [ a            owl:Class ;
                            owl:unionOf  ( v1:Offering v1:License s:Offer )
                          ] ;
        rdfs:isDefinedBy  <http://purl.org/goodrelations/v1> ;
        rdfs:label        "eligible duration (0..1)"@en ;
        rdfs:range        v1:QuantitativeValue .

v1:FederalExpress  a      v1:DeliveryModeParcelService ;
        rdfs:comment      "Delivery via the parcel service Federal Express."@en ;
        rdfs:isDefinedBy  <http://purl.org/goodrelations/v1> ;
        rdfs:label        "Federal Express (delivery method)"@en .

v1:hasNext  a             owl:ObjectProperty ;
        rdfs:comment      "This ordering relation for gr:DayOfWeek indicates that the subject is directly followed by the object.\n\nExample: Monday hasNext Tuesday\n\nSince days of the week are a cycle, this property is not transitive."@en ;
        rdfs:domain       v1:DayOfWeek ;
        rdfs:isDefinedBy  <http://purl.org/goodrelations/v1> ;
        rdfs:label        "has next (0..1)"@en ;
        rdfs:range        v1:DayOfWeek ;
        owl:inverseOf     v1:hasPrevious .

v1:DirectDebit  a         v1:PaymentMethod ;
        rdfs:comment      "Payment by direct debit, i.e., the buying party will inform the offering gr:BusinessEntity about its bank account details and authorizes the gr:BusinessEntity to collect the agreed amount directly from that account."@en ;
        rdfs:isDefinedBy  <http://purl.org/goodrelations/v1> ;
        rdfs:label        "Direct debit (payment method)"@en .

v1:ProductOrServiceModel
        a                 owl:Class ;
        rdfs:comment      "A product or service model is a intangible entity that specifies some characteristics of a group of similar, usually mass-produced products, in the sense of a prototype. In case of mass-produced products, there exists a relation gr:hasMakeAndModel between the actual product or service (gr:Individual or gr:SomeItems) and the prototype (gr:ProductOrServiceModel). GoodRelations treats product or service models as \"prototypes\" instead of a completely separate kind of entities, because this allows using the same domain-specific properties (e.g. gr:weight) for describing makes and models and for describing actual products.\n\nExamples: Ford T, Volkswagen Golf, Sony Ericsson W123 cell phone\n\nNote: An actual product or service (gr:Individual) by default shares the features of its model (e.g. the weight). However, this requires non-standard reasoning. See http://wiki.goodrelations-vocabulary.org/Axioms for respective rule sets.\n\t\nCompatibility with schema.org: This class is (approximately) a subclass of http://schema.org/Product."@en ;
        rdfs:isDefinedBy  <http://purl.org/goodrelations/v1> ;
        rdfs:label        "Product or service model"@en ;
        rdfs:subClassOf   s:Product , v1:ProductOrService ;
        owl:disjointWith  v1:SomeItems , v1:Brand , v1:BusinessEntity , v1:Individual .

v1:Sunday  a                v1:DayOfWeek ;
        rdfs:comment        "Sunday as a day of the week."@en ;
        rdfs:isDefinedBy    <http://purl.org/goodrelations/v1> ;
        rdfs:label          "Sunday (day of week)"@en ;
        v1:displayPosition  7 ;
        v1:hasNext          v1:Monday ;
        v1:hasPrevious      v1:Saturday .

v1:Friday  a                v1:DayOfWeek ;
        rdfs:comment        "Friday as a day of the week."@en ;
        rdfs:isDefinedBy    <http://purl.org/goodrelations/v1> ;
        rdfs:label          "Friday (day of week)"@en ;
        v1:displayPosition  5 ;
        v1:hasNext          v1:Saturday ;
        v1:hasPrevious      v1:Thursday .

v1:hasPrevious  a         owl:ObjectProperty ;
        rdfs:comment      "This ordering relation for gr:DayOfWeek indicates that the subject is directly preceeded by the object.\n\nExample: Tuesday hasPrevious Monday\n\nSince days of the week are a cycle, this property is not transitive."@en ;
        rdfs:domain       v1:DayOfWeek ;
        rdfs:isDefinedBy  <http://purl.org/goodrelations/v1> ;
        rdfs:label        "has previous (0..1)"@en ;
        rdfs:range        v1:DayOfWeek ;
        owl:inverseOf     v1:hasNext .

v1:Discover  a            v1:PaymentMethodCreditCard ;
        rdfs:comment      "Payment by credit or debit cards issued by the Discover network."@en ;
        rdfs:isDefinedBy  <http://purl.org/goodrelations/v1> ;
        rdfs:label        "Discover (payment method)"@en .

v1:N-Ary-Relations  a     owl:Class ;
        rdfs:comment      "This is the superclass for all classes that are placeholders for n-ary relations, which OWL cannot represent.\nDEPRECATED. Do not use this class in data or queries."@en ;
        rdfs:isDefinedBy  <http://purl.org/goodrelations/v1> ;
        rdfs:label        "N-ary relations (DEPRECATED)"@en ;
        owl:deprecated    true .

v1:DeliveryModeMail  a    v1:DeliveryMethod ;
        rdfs:comment      "Delivery via regular mail service (private or public postal services)."@en ;
        rdfs:isDefinedBy  <http://purl.org/goodrelations/v1> ;
        rdfs:label        "Delivery mode mail (delivery method)"@en .

v1:eligibleTransactionVolume
        a                 owl:ObjectProperty ;
        rdfs:comment      "This property can be used to indicate the transaction volume, in a monetary unit, for which the gr:Offering or gr:PriceSpecification is valid. This is mostly used to specify a minimal purchasing volume, to express free shipping above a certain order volume, or to limit the acceptance of credit cards to purchases above a certain amount.\n\nThe object is a gr:PriceSpecification that uses the properties gr:hasMaxCurrencyValue and gr:hasMinCurrencyValue to indicate the lower and upper boundaries and gr:hasCurrency to indicate the currency using the ISO 4217 standard (3 characters)."@en ;
        rdfs:domain       [ a            owl:Class ;
                            owl:unionOf  ( v1:Offering v1:PriceSpecification s:Offer )
                          ] ;
        rdfs:isDefinedBy  <http://purl.org/goodrelations/v1> ;
        rdfs:label        "eligible transaction volume (0..1)"@en ;
        rdfs:range        v1:PriceSpecification .

v1:Cash  a                v1:PaymentMethod ;
        rdfs:comment      "Payment by cash upon delivery or pickup."@en ;
        rdfs:isDefinedBy  <http://purl.org/goodrelations/v1> ;
        rdfs:label        "Cash (payment method)"@en .

v1:DinersClub  a          v1:PaymentMethodCreditCard ;
        rdfs:comment      "Payment by credit or debit cards issued by the Diner's Club network."@en ;
        rdfs:isDefinedBy  <http://purl.org/goodrelations/v1> ;
        rdfs:label        "Diners Club (payment method)"@en .

v1:JCB  a                 v1:PaymentMethodCreditCard ;
        rdfs:comment      "Payment by credit or debit cards issued by the JCB network."@en ;
        rdfs:isDefinedBy  <http://purl.org/goodrelations/v1> ;
        rdfs:label        "JCB (payment method)"@en .

v1:hasMaxCurrencyValue
        a                 owl:DatatypeProperty ;
        rdfs:comment      "This property specifies the UPPER BOUND of the amount of money for a price RANGE per unit, shipping charges, or payment charges. The currency and other relevant details are attached to the respective gr:PriceSpecification etc.\nFor a gr:UnitPriceSpecification, this is the UPPER BOUND for the price for one unit or bundle (as specified in the unit of measurement of the unit price specification) of the respective gr:ProductOrService. For a gr:DeliveryChargeSpecification or a gr:PaymentChargeSpecification, it is the UPPER BOUND of the price per delivery or payment.\n\nUsing gr:hasCurrencyValue sets the upper and lower bounds to the same given value, i.e., x gr:hasCurrencyValue y implies x gr:hasMinCurrencyValue y, x gr:hasMaxCurrencyValue y."@en ;
        rdfs:domain       v1:PriceSpecification ;
        rdfs:isDefinedBy  <http://purl.org/goodrelations/v1> ;
        rdfs:label        "has max currency value (1..1)"@en ;
        rdfs:range        xsd:float .

v1:vatID  a               owl:DatatypeProperty ;
        rdfs:comment      "The Value-added Tax ID of the gr:BusinessEntity. See http://en.wikipedia.org/wiki/Value_added_tax_identification_number for details."@en ;
        rdfs:domain       [ a            owl:Class ;
                            owl:unionOf  ( v1:BusinessEntity s:Organization s:Person )
                          ] ;
        rdfs:isDefinedBy  <http://purl.org/goodrelations/v1> ;
        rdfs:label        "VAT ID (0..1)"@en ;
        rdfs:range        xsd:string .

v1:greater  a             owl:TransitiveProperty , owl:ObjectProperty ;
        rdfs:comment      "This ordering relation for qualitative values indicates that the subject is greater than the object."@en ;
        rdfs:domain       v1:QualitativeValue ;
        rdfs:isDefinedBy  <http://purl.org/goodrelations/v1> ;
        rdfs:label        "greater (0..*)"@en ;
        rdfs:range        v1:QualitativeValue ;
        owl:inverseOf     v1:lesser .

v1:isSimilarTo  a         owl:ObjectProperty ;
        rdfs:comment      "This states that a given gr:ProductOrService is similar to another product or service. Of course, this is a subjective statement; when interpreting it, the trust in the origin of the statement should be taken into account."@en ;
        rdfs:domain       [ a            owl:Class ;
                            owl:unionOf  ( v1:ProductOrService s:Product )
                          ] ;
        rdfs:isDefinedBy  <http://purl.org/goodrelations/v1> ;
        rdfs:label        "is similar to (0..*)"@en ;
        rdfs:range        v1:ProductOrService .

v1:hasOpeningHoursDayOfWeek
        a                 owl:ObjectProperty ;
        rdfs:comment      "This specifies the gr:DayOfWeek to which the gr:OpeningHoursSpecification is related.\n\nNote: Use multiple instances of gr:OpeningHoursSpecification for specifying the opening hours for multiple days if the opening hours differ."@en ;
        rdfs:domain       v1:OpeningHoursSpecification ;
        rdfs:isDefinedBy  <http://purl.org/goodrelations/v1> ;
        rdfs:label        "has opening hours day of week (1..*)"@en ;
        rdfs:range        v1:DayOfWeek .

v1:PayPal  a              v1:PaymentMethod ;
        rdfs:comment      "Payment via the PayPal payment service."@en ;
        rdfs:isDefinedBy  <http://purl.org/goodrelations/v1> ;
        rdfs:label        "PayPal (payment method)"@en .

v1:Wednesday  a             v1:DayOfWeek ;
        rdfs:comment        "Wednesday as a day of the week."@en ;
        rdfs:isDefinedBy    <http://purl.org/goodrelations/v1> ;
        rdfs:label          "Wednesday (day of week)"@en ;
        v1:displayPosition  3 ;
        v1:hasNext          v1:Thursday ;
        v1:hasPrevious      v1:Tuesday .

v1:PaymentMethod  a       owl:Class ;
        rdfs:comment      "A payment method is a standardized procedure for transferring the monetary amount for a purchase. Payment methods are characterized by the legal and technical structures used, and by the organization or group carrying out the transaction. This element is mostly used for specifying the types of payment accepted by a gr:BusinessEntity.\n\nExamples: VISA, MasterCard, Diners, cash, or bank transfer in advance."@en ;
        rdfs:isDefinedBy  <http://purl.org/goodrelations/v1> ;
        rdfs:label        "Payment method"@en ;
        owl:disjointWith  v1:TypeAndQuantityNode , v1:OpeningHoursSpecification , v1:Location , v1:Brand , v1:BusinessEntityType , v1:WarrantyScope , v1:BusinessEntity , v1:DayOfWeek , v1:BusinessFunction , v1:WarrantyPromise , v1:QuantitativeValue , v1:DeliveryMethod , v1:Offering , v1:PriceSpecification .

v1:closes  a              owl:DatatypeProperty ;
        rdfs:comment      "The closing  hour of the gr:Location on the given gr:DayOfWeek.\nIf no time-zone suffix is included, the time is given in the local time valid at the gr:Location.\n\nFor a time in GMT/UTC, simply add a \"Z\" following the time:\n\n09:30:10Z.\n\nAlternatively, you can specify an offset from the UTC time by adding a positive or negative time following the time:\n\n09:30:10-09:00\n\n09:30:10+09:00.\n\nNote 1: Use 00:00:00 for the first second of the respective day and 23:59:59 for the last second of that day.\nNote 2: If a store opens at 17:00 on Saturdays and closes at 03:00:00 a.m. next morning, use two instances of this class, one with 17:00:00 - 23:59:59 for Saturday and another one with 00:00:00 - 03:00:00 for Sunday.\nNote 3: If the shop re-opens on the same day of the week or set of days of the week, you must create a second instance of gr:OpeningHoursSpecification."@en ;
        rdfs:domain       v1:OpeningHoursSpecification ;
        rdfs:isDefinedBy  <http://purl.org/goodrelations/v1> ;
        rdfs:label        "closes (1..1)"@en ;
        rdfs:range        xsd:time .

v1:ProductOrService  a    owl:Class ;
        rdfs:comment      "The superclass of all classes describing products or services types, either by nature or purpose. Examples for such subclasses are \"TV set\", \"vacuum cleaner\", etc. An instance of this class can be either an actual product or service (gr:Individual), a placeholder instance for unknown instances of a mass-produced commodity (gr:SomeItems), or a model / prototype specification (gr:ProductOrServiceModel). When in doubt, use gr:SomeItems.\n\nExamples: \na) MyCellphone123, i.e. my personal, tangible cell phone (gr:Individual)\nb) Siemens1234, i.e. the Siemens cell phone make and model 1234 (gr:ProductOrServiceModel)\nc) dummyCellPhone123 as a placeholder for actual instances of a certain kind of cell phones (gr:SomeItems)\n\t\nNote: Your first choice for specializations of gr:ProductOrService should be http://www.productontology.org.\n\nCompatibility with schema.org: This class is (approximately) equivalent to http://schema.org/Product."@en ;
        rdfs:isDefinedBy  <http://purl.org/goodrelations/v1> ;
        rdfs:label        "Product or service"@en ;
        owl:disjointWith  v1:Brand , v1:DeliveryMethod , v1:WarrantyPromise , v1:QuantitativeValue , v1:OpeningHoursSpecification , v1:Offering , v1:TypeAndQuantityNode , v1:DayOfWeek , v1:WarrantyScope , v1:PriceSpecification , v1:BusinessFunction , v1:BusinessEntityType .

v1:lesserOrEqual  a       owl:TransitiveProperty , owl:ObjectProperty ;
        rdfs:comment      "This ordering relation for gr:QualitativeValue pairs indicates that the subject is lesser than or equal to the object."@en ;
        rdfs:domain       v1:QualitativeValue ;
        rdfs:isDefinedBy  <http://purl.org/goodrelations/v1> ;
        rdfs:label        "lesser or equal (0..*)"@en ;
        rdfs:range        v1:QualitativeValue ;
        owl:inverseOf     v1:greaterOrEqual .

v1:UPS  a                 v1:DeliveryModeParcelService ;
        rdfs:comment      "Delivery via the parcel service UPS."@en ;
        rdfs:isDefinedBy  <http://purl.org/goodrelations/v1> ;
        rdfs:label        "UPS (delivery method)"@en .

s:Organization  a        owl:Class ;
        rdfs:subClassOf  v1:BusinessEntity .

v1:valueAddedTaxIncluded
        a                 owl:DatatypeProperty ;
        rdfs:comment      "This property specifies whether the applicable value-added tax (VAT)  is included in the price of the gr:PriceSpecification or not.\n\nNote: This is a simple representation which may not properly reflect all details of local taxation."@en ;
        rdfs:domain       v1:PriceSpecification ;
        rdfs:isDefinedBy  <http://purl.org/goodrelations/v1> ;
        rdfs:label        "value added tax included (0..1)"@en ;
        rdfs:range        xsd:boolean .

v1:TypeAndQuantityNode
        a                 owl:Class ;
        rdfs:comment      "This class collates all the information about a gr:ProductOrService included in a bundle. If a gr:Offering contains just one item, you can directly link from the gr:Offering to the gr:ProductOrService using gr:includes. If the offering contains multiple items, use an instance of this class for each component to indicate the quantity, unit of measurement, and type of product, and link from the gr:Offering via gr:includesObject.\n\nExample: An offering may include of 100g of Butter and 1 kg of potatoes, or 1 cell phone and 2 headsets."@en ;
        rdfs:isDefinedBy  <http://purl.org/goodrelations/v1> ;
        rdfs:label        "Type and quantity node"@en ;
        owl:disjointWith  v1:DayOfWeek , v1:Location , v1:WarrantyScope , v1:ProductOrService , v1:Brand , v1:QuantitativeValue , v1:BusinessFunction , v1:PaymentMethod , v1:QualitativeValue , v1:DeliveryMethod , v1:WarrantyPromise , v1:BusinessEntityType , v1:PriceSpecification , v1:Offering , v1:OpeningHoursSpecification , v1:BusinessEntity .

v1:ConstructionInstallation
        a                 v1:BusinessFunction ;
        rdfs:comment      "This gr:BusinessFunction indicates that the gr:BusinessEntity offers (or seeks) the construction and/or installation of the specified gr:ProductOrService at the customer's location."@en ;
        rdfs:isDefinedBy  <http://purl.org/goodrelations/v1> ;
        rdfs:label        "Construction / installation (business function)"@en .

v1:PublicHolidays  a        v1:DayOfWeek ;
        rdfs:comment        "A placeholder for all official public holidays at the gr:Location. This allows specifying the opening hours on public holidays. If a given day is a public holiday, this specification supersedes the opening hours for the respective day of the week."@en ;
        rdfs:isDefinedBy    <http://purl.org/goodrelations/v1> ;
        rdfs:label          "Public holidays (day of week)"@en ;
        v1:displayPosition  8 .

v1:appliesToPaymentMethod
        a                 owl:ObjectProperty ;
        rdfs:comment      "This property specifies the gr:PaymentMethod to which the gr:PaymentChargeSpecification applies."@en ;
        rdfs:domain       v1:PaymentChargeSpecification ;
        rdfs:isDefinedBy  <http://purl.org/goodrelations/v1> ;
        rdfs:label        "applies to payment method (1..*)"@en ;
        rdfs:range        v1:PaymentMethod .

v1:eligibleRegions  a     owl:DatatypeProperty ;
        rdfs:comment      "This property specifies the geo-political region or regions for which the gr:Offering, gr:License, or gr:DeliveryChargeSpecification is valid using the two-character version of ISO 3166-1 (ISO 3166-1 alpha-2)  for regions or ISO 3166-2 , which breaks down the countries from ISO 3166-1 into administrative subdivisions.\n\nImportant: Do NOT use 3-letter ISO 3166-1 codes!"@en ;
        rdfs:domain       [ a            owl:Class ;
                            owl:unionOf  ( v1:DeliveryChargeSpecification v1:Offering v1:License s:Offer )
                          ] ;
        rdfs:isDefinedBy  <http://purl.org/goodrelations/v1> ;
        rdfs:label        "eligible regions (0..*)"@en ;
        rdfs:range        xsd:string .

v1:Brand  a               owl:Class ;
        rdfs:comment      "A brand is the identity of a specific product, service, or business. Use foaf:logo for attaching a brand logo and gr:name or rdfs:label for attaching the brand name.\t\n\n(Source: Wikipedia, the free encyclopedia, see http://en.wikipedia.org/wiki/Brand)"@en ;
        rdfs:isDefinedBy  <http://purl.org/goodrelations/v1> ;
        rdfs:label        "Brand"@en ;
        owl:disjointWith  v1:PaymentMethod , v1:QuantitativeValue , v1:WarrantyPromise , v1:TypeAndQuantityNode , v1:BusinessFunction , v1:DayOfWeek , v1:PriceSpecification , v1:ProductOrService , v1:Offering , v1:Location , v1:DeliveryMethod , v1:WarrantyScope , v1:BusinessEntity , v1:BusinessEntityType , v1:OpeningHoursSpecification .

v1:Reseller  a            v1:BusinessEntityType ;
        rdfs:comment      "The gr:BusinessEntityType representing such agents that are purchasing the scope of products included in the gr:Offering for resale on the market. Resellers are also businesses, i.e., they are officially registered with the public administration and strive for profits by their activities."@en ;
        rdfs:isDefinedBy  <http://purl.org/goodrelations/v1> ;
        rdfs:label        "Reseller (business entity type)"@en .

v1:Maintain  a            v1:BusinessFunction ;
        rdfs:comment      "This gr:BusinessFunction indicates that the gr:BusinessEntity offers (or seeks) typical maintenance tasks for the specified gr:ProductOrService. Maintenance tasks are actions that undo or compensate for wear or other deterioriation caused by regular usage, in order to restore the originally intended function of the product, or to prevent outage or malfunction."@en ;
        rdfs:isDefinedBy  <http://purl.org/goodrelations/v1> ;
        rdfs:label        "Maintain (business function)"@en .

v1:condition  a           owl:DatatypeProperty ;
        rdfs:comment      "A textual description of the condition of the product or service, or the products or services included in the offer (when attached to a gr:Offering)"@en ;
        rdfs:domain       [ a            owl:Class ;
                            owl:unionOf  ( v1:Offering v1:ProductOrService s:Product )
                          ] ;
        rdfs:isDefinedBy  <http://purl.org/goodrelations/v1> ;
        rdfs:label        "condition (0..1)"@en ;
        rdfs:range        rdfs:Literal .

v1:qualitativeProductOrServiceProperty
        a                 owl:ObjectProperty ;
        rdfs:comment      "This is the super property of all qualitative properties for products and services. All properties in product or service ontologies for which gr:QualitativeValue instances are specified are subproperties of this property."@en ;
        rdfs:domain       [ a            owl:Class ;
                            owl:unionOf  ( v1:ProductOrService s:Product )
                          ] ;
        rdfs:isDefinedBy  <http://purl.org/goodrelations/v1> ;
        rdfs:label        "qualitative product or service property (0..*)"@en ;
        rdfs:range        v1:QualitativeValue .

v1:successorOf  a         owl:TransitiveProperty , owl:ObjectProperty ;
        rdfs:comment      "This property indicates that the subject is a newer, often updated or improved variant of the gr:ProductOrServiceModel used as the object.\n\nExample: Golf III successorOf Golf II\n\nThis relation is transitive."@en ;
        rdfs:domain       v1:ProductOrServiceModel ;
        rdfs:isDefinedBy  <http://purl.org/goodrelations/v1> ;
        rdfs:label        "successor of (0..*)"@en ;
        rdfs:range        v1:ProductOrServiceModel ;
        owl:inverseOf     v1:predecessorOf .

v1:WarrantyScope  a       owl:Class ;
        rdfs:comment      "The warranty scope represents types of services that will be provided free of charge by the vendor or manufacturer in the case of a defect (e.g. labor and parts, just parts), as part of the warranty included in an gr:Offering. The actual services may be provided by the gr:BusinessEntity making the offering, by the manufacturer of the product, or by a third party. \n\nExamples: Parts and Labor, Parts"@en ;
        rdfs:isDefinedBy  <http://purl.org/goodrelations/v1> ;
        rdfs:label        "Warranty scope"@en ;
        owl:disjointWith  v1:DeliveryMethod , v1:WarrantyPromise , v1:BusinessEntityType , v1:PaymentMethod , v1:Brand , v1:BusinessFunction , v1:Location , v1:BusinessEntity , v1:TypeAndQuantityNode , v1:PriceSpecification , v1:QuantitativeValue , v1:ProductOrService , v1:OpeningHoursSpecification , v1:DayOfWeek , v1:Offering .

v1:greaterOrEqual  a      owl:TransitiveProperty , owl:ObjectProperty ;
        rdfs:comment      "This ordering relation for qualitative values indicates that the subject is greater than or equal to the object."@en ;
        rdfs:domain       v1:QualitativeValue ;
        rdfs:isDefinedBy  <http://purl.org/goodrelations/v1> ;
        rdfs:label        "greater or equal (0..*)"@en ;
        rdfs:range        v1:QualitativeValue ;
        owl:inverseOf     v1:lesserOrEqual .

dc:creator  a   owl:AnnotationProperty .

v1:name  a                owl:DatatypeProperty ;
        rdfs:comment      "A short text describing the respective resource.\n\nThis property is semantically equivalent to dcterms:title and rdfs:label and just meant as a handy shortcut for marking up data."@en ;
        rdfs:domain       [ a            owl:Class ;
                            owl:unionOf  ( owl:Thing v1:Brand v1:BusinessEntity v1:BusinessEntityType v1:BusinessFunction v1:DayOfWeek v1:DeliveryChargeSpecification v1:DeliveryMethod v1:DeliveryModeParcelService v1:Individual v1:Location v1:Offering v1:OpeningHoursSpecification v1:PaymentChargeSpecification v1:PaymentMethod v1:PaymentMethodCreditCard v1:PriceSpecification v1:ProductOrService v1:ProductOrServiceModel v1:QualitativeValue v1:QuantitativeValue v1:QuantitativeValueFloat v1:QuantitativeValueInteger v1:SomeItems v1:TypeAndQuantityNode v1:UnitPriceSpecification v1:WarrantyPromise v1:WarrantyScope )
                          ] ;
        rdfs:domain       [ a            owl:Class ;
                            owl:unionOf  ( owl:Thing acco:Accommodation acco:AccommodationFeature acco:Meal acco:Allinclusive acco:BedType acco:DwellingType acco:CompoundPrice )
                          ] ;
        rdfs:isDefinedBy  <http://purl.org/goodrelations/v1> ;
        rdfs:label        "name (0..1)"@en ;
        rdfs:range        rdfs:Literal .

v1:hasGlobalLocationNumber
        a                 owl:DatatypeProperty ;
        rdfs:comment      "The Global Location Number (GLN, sometimes also referred to as International Location Number or ILN) of the respective gr:BusinessEntity or gr:Location.\nThe Global Location Number is a thirteen-digit number used to identify parties and physical locations."@en ;
        rdfs:domain       [ a            owl:Class ;
                            owl:unionOf  ( v1:BusinessEntity v1:Location s:Place s:Organization )
                          ] ;
        rdfs:isDefinedBy  <http://purl.org/goodrelations/v1> ;
        rdfs:label        "has Global Location Number (0..1)"@en ;
        rdfs:range        xsd:string .

v1:datatypeProductOrServiceProperty
        a                 owl:DatatypeProperty ;
        rdfs:comment      "This property is the super property for all pure datatype properties that can be used to describe a gr:ProductOrService.\n\nIn products and services ontologies, only such properties that are no quantitative properties and that have no predefined gr:QualitativeValue instances are subproperties of this property. In practice, this refers to a few integer properties for which the integer value represents qualitative aspects, for string datatypes (as long as no predefined values exist), for boolean datatype properties, and for dates and times."@en ;
        rdfs:domain       [ a            owl:Class ;
                            owl:unionOf  ( v1:ProductOrService s:Product )
                          ] ;
        rdfs:isDefinedBy  <http://purl.org/goodrelations/v1> ;
        rdfs:label        "datatype product or service property (0..*)"@en ;
        rdfs:range        rdfs:Literal .

v1:hasPOS  a              owl:ObjectProperty ;
        rdfs:comment      "This property states that the respective gr:Location is a point of sale for the respective gr:BusinessEntity. It allows linking those two types of entities without the need for a particular gr:Offering."@en ;
        rdfs:domain       [ a            owl:Class ;
                            owl:unionOf  ( v1:BusinessEntity s:Organization )
                          ] ;
        rdfs:isDefinedBy  <http://purl.org/goodrelations/v1> ;
        rdfs:label        "has POS (0..*)"@en ;
        rdfs:range        v1:Location .

v1:depth  a                 owl:ObjectProperty ;
        rdfs:comment        "The depth of the product.\nTypical unit code(s): CMT for centimeters, INH for inches"@en ;
        rdfs:domain         [ a            owl:Class ;
                              owl:unionOf  ( v1:ProductOrService s:Product )
                            ] ;
        rdfs:isDefinedBy    <http://purl.org/goodrelations/v1> ;
        rdfs:label          "depth (0..1)"@en ;
        rdfs:range          v1:QuantitativeValue ;
        rdfs:subPropertyOf  v1:quantitativeProductOrServiceProperty .

v1:hasMPN  a                owl:DatatypeProperty ;
        rdfs:comment        "The Manufacturer Part Number or MPN is a unique identifier for a product, service, or bundle from the perspective of a particular manufacturer. MPNs can be assigned to products or product datasheets, or bundles. Accordingly, the domain of this property is the union of gr:ProductOrService (the common superclass of goods and datasheets), and gr:Offering.\n\nImportant: Be careful when assuming two products or services instances or offering instances to be identical based on the MPN. Since MPNs are unique only for the same gr:BusinessEntity, this holds only when the two MPN values refer to the same gr:BusinessEntity. Such can be done by taking into account the provenance of the data. \n\nUsually, the properties gr:hasEAN_UCC-13 and gr:hasGTIN-14 are much more reliable identifiers, because they are globally unique.\n\nSee also http://en.wikipedia.org/wiki/Part_number"@en ;
        rdfs:domain         [ a            owl:Class ;
                              owl:unionOf  ( v1:Offering v1:ProductOrService s:Product )
                            ] ;
        rdfs:isDefinedBy    <http://purl.org/goodrelations/v1> ;
        rdfs:label          "has MPN (0..*)"@en ;
        rdfs:range          xsd:string ;
        rdfs:subPropertyOf  s:productID .

v1:isConsumableFor  a     owl:ObjectProperty ;
        rdfs:comment      "This states that a particular gr:ProductOrService is a consumable for another product or service."@en ;
        rdfs:domain       [ a            owl:Class ;
                            owl:unionOf  ( v1:ProductOrService s:Product )
                          ] ;
        rdfs:isDefinedBy  <http://purl.org/goodrelations/v1> ;
        rdfs:label        "is consumable for (0..*)"@en ;
        rdfs:range        v1:ProductOrService .

v1:durationOfWarrantyInMonths
        a                 owl:DatatypeProperty ;
        rdfs:comment      "This property specifies the duration of the gr:WarrantyPromise in months."@en ;
        rdfs:domain       v1:WarrantyPromise ;
        rdfs:isDefinedBy  <http://purl.org/goodrelations/v1> ;
        rdfs:label        "duration of warranty in months (0..1)"@en ;
        rdfs:range        xsd:int .

v1:ProductOrServicesSomeInstancesPlaceholder
        a                    owl:Class ;
        rdfs:comment         "DEPRECATED - This class is superseded by gr:SomeItems. Replace all occurrences of gr:ProductOrServicesSomeInstancesPlaceholder by gr:SomeItems, if possible."@en ;
        rdfs:isDefinedBy     <http://purl.org/goodrelations/v1> ;
        rdfs:label           "Product or services some instances placeholder (DEPRECATED)"@en ;
        rdfs:subClassOf      v1:ProductOrService ;
        owl:deprecated       true ;
        owl:equivalentClass  v1:SomeItems .

dc:title  a     owl:AnnotationProperty .

v1:Monday  a                v1:DayOfWeek ;
        rdfs:comment        "Monday as a day of the week."@en ;
        rdfs:isDefinedBy    <http://purl.org/goodrelations/v1> ;
        rdfs:label          "Monday (day of week)"@en ;
        v1:displayPosition  1 ;
        v1:hasNext          v1:Tuesday ;
        v1:hasPrevious      v1:Sunday .

v1:hasStockKeepingUnit
        a                   owl:DatatypeProperty ;
        rdfs:comment        "The Stock Keeping Unit, or SKU is a unique identifier for a product, service, or bundle from the perspective of a particular supplier, i.e. SKUs are mostly assigned and serialized at the merchant level. \nExamples of SKUs are the ordering or parts numbers used by a particular Web shop or catalog.\n\nConsequently, the domain of gr:hasStockKeepingUnit is the union of the classes gr:Offering and gr:ProductOrService. \nIf attached to a gr:Offering, the SKU will usually reflect a merchant-specific identifier, i.e. one valid only for that particular retailer or shop. \nIf attached to a gr:ProductOrServiceModel, the SKU can reflect either the identifier used by the merchant or the part number used by the official manufacturer of that part. For the latter, gr:hasMPN is a better choice.\n\nImportant: Be careful when assuming two products or services instances or offering instances to be identical based on the SKU. Since SKUs are unique only for the same gr:BusinessEntity, this can be assumed only when you are sure that the two SKU values refer to the same business entity. Such can be done by taking into account the provenance of the data. As long as instances of gr:Offering are concerned, you can also check that the offerings are being offered by the same gr:Business Entity.\n\nUsually, the properties gr:hasEAN_UCC-13 and gr:hasGTIN-14 are much more reliable identifiers, because they are globally unique.\n\nSee also http://en.wikipedia.org/wiki/Stock_Keeping_Unit."@en ;
        rdfs:domain         [ a            owl:Class ;
                              owl:unionOf  ( v1:Offering v1:ProductOrService s:Offer s:Product )
                            ] ;
        rdfs:isDefinedBy    <http://purl.org/goodrelations/v1> ;
        rdfs:label          "has Stock Keeping Unit (0..*)"@en ;
        rdfs:range          xsd:string ;
        rdfs:subPropertyOf  s:productID .

v1:advanceBookingRequirement
        a                 owl:ObjectProperty ;
        rdfs:comment      "The minimal and maximal amount of time that is required between accepting the gr:Offering and the actual usage of the resource or service. This is mostly relevant for offers regarding hotel rooms, the rental of objects, or the provisioning of services. The duration is specified relatively to the beginning of the usage of the contracted object. It is represented by attaching an instance of the class gr:QuantitativeValueInteger. The lower and upper boundaries are specified using the properties gr:hasMinValueInteger and gr:hasMaxValueInteger to that instance. The unit of measurement is specified using the property gr:hasUnitOfMeasurement with a string holding a UN/CEFACT code suitable for durations, e.g. MON (months), DAY (days), HUR (hours), or MIN (minutes).\n\nThe difference to the gr:validFrom and gr:validThrough properties is that those specify the interval during which the gr:Offering is valid, while gr:advanceBookingRequirement specifies the acceptable relative amount of time between accepting the offer and the fulfilment or usage."@en ;
        rdfs:domain       [ a            owl:Class ;
                            owl:unionOf  ( v1:Offering s:Offer )
                          ] ;
        rdfs:isDefinedBy  <http://purl.org/goodrelations/v1> ;
        rdfs:label        "advance booking requirement (0..1)"@en ;
        rdfs:range        v1:QuantitativeValueInteger .

v1:DeliveryMethod  a      owl:Class ;
        rdfs:comment      "A delivery method is a standardized procedure for transferring the product or service to the destination of fulfilment chosen by the customer. Delivery methods are characterized by the means of transportation used, and by the organization or group that is the contracting party for the sending gr:BusinessEntity (this is important, since the contracted party may subcontract the fulfilment to smaller, regional businesses).\n\nExamples: Delivery by mail, delivery by direct download, delivery by UPS"@en ;
        rdfs:isDefinedBy  <http://purl.org/goodrelations/v1> ;
        rdfs:label        "Delivery method"@en ;
        owl:disjointWith  v1:WarrantyPromise , v1:BusinessFunction , v1:DayOfWeek , v1:QuantitativeValue , v1:Brand , v1:ProductOrService , v1:BusinessEntity , v1:Offering , v1:Location , v1:WarrantyScope , v1:PriceSpecification , v1:PaymentMethod , v1:TypeAndQuantityNode , v1:OpeningHoursSpecification , v1:BusinessEntityType .

v1:License  a             owl:Class ;
        rdfs:comment      "A license is the specification of a bundle of rights that determines the type of activity or access offered by the gr:BusinessEntity on the gr:ProductOrService through the gr:Offering.\n\t\nLicenses can be standardized (e.g. LPGL, Creative Commons, ...), vendor-specific, or individually defined for a single offer or product. Whether there is a fee for obtaining the license is specified using the gr:UnitPriceSpecification attached to the gr:Offering. Use foaf:page for linking to a document containing the license, e.g. in PDF or HTML."@en ;
        rdfs:isDefinedBy  <http://purl.org/goodrelations/v1> ;
        rdfs:label        "License"@en ;
        rdfs:subClassOf   v1:BusinessFunction .

v1:QuantitativeValueFloat
        a                 owl:Class ;
        rdfs:comment      "An instance of this class is an actual float value for a quantitative property of a product. This instance is usually characterized by a minimal value, a maximal value, and a unit of measurement.\n\nExamples: The intervals \"between 10.0  and 25.4 kilogramms\" or \"10.2 and 15.5 milimeters\".\n\nCompatibility with schema.org: This class is a subclass of http://schema.org/Quantity."@en ;
        rdfs:isDefinedBy  <http://purl.org/goodrelations/v1> ;
        rdfs:label        "Quantitative value float"@en ;
        rdfs:subClassOf   v1:QuantitativeValue ;
        owl:disjointWith  v1:QuantitativeValueInteger .

v1:UnitPriceSpecification
        a                 owl:Class ;
        rdfs:comment      "A unit price specification is a conceptual entity that specifies the price asked for a given gr:Offering by the respective gr:Business Entity. An offering may be linked to multiple unit price specifications that specify alternative prices for non-overlapping sets of conditions (e.g. quantities or sales regions) or with differing validity periods. \n\nA unit price specification is characterized by (1) the lower and upper limits and the unit of measurement of the eligible quantity, (2) by a monetary amount per unit of the product or service, and (3)  whether this prices includes local sales taxes, namely VAT.\n\t\nExample: The price, including VAT, for 1 kg of a given material is 5 Euros per kg for 0 - 5 kg and 4 Euros for quantities above 5 kg.\n\nThe eligible quantity interval for a given price is specified using the object property gr:hasEligibleQuantity, which points to an instance of gr:QuantitativeValue. The currency is specified using the gr:hasCurrency property, which points to an ISO 4217 currency code. The unit of measurement for the eligible quantity is specified using the gr:hasUnitOfMeasurement datatype property, which points to an UN/CEFACT Common Code (3 characters).\n\t\nIn most cases, the appropriate unit of measurement is the UN/CEFACT Common Code \"C62\" for \"Unit or piece\", since a gr:Offering is defined by the quantity and unit of measurement of all items included (e.g. \"1 kg of bananas plus a 2 kg of apples\"). As long at the offering consists of only one item, it is also possible to use an unit of measurement of choice for specifying the price per unit. For bundles, however, only  \"C62\" for \"Unit or piece\" is a valid unit of measurement.\n\nYou can assume that the price is given per unit or piece if there is no gr:hasUnitOfMeasurement property attached to the price.\n\t\nWhether VAT and sales taxes are included in this price is specified using the property gr:valueAddedTaxIncluded (xsd:boolean).\n\t\nThe price per unit of measurement is specified as a float value of the gr:hasCurrencyValue property. The currency is specified via the gr:hasCurrency datatype property. Whether the price includes VAT or not is indicated by the gr:valueAddedTaxIncluded datatype property.\n\nThe property priceType can be used to indicate that the price is a retail price recommendation only (i.e. a list price). \n\nIf the price can only be given as a range, use gr:hasMaxCurrencyValue and gr:hasMinCurrencyValue for the upper and lower bounds.\n\nImportant: When querying for the price, always use gr:hasMaxCurrencyValue and gr:hasMinCurrencyValue.\n\nNote 1: Due to the complexity of pricing scenarios in various industries, it may be necessary to create extensions of this fundamental model of price specifications. Such can be done easily by importing and refining the GoodRelations ontology.\n\nNote 2: For Google, attaching a gr:validThrough statement to a gr:UnitPriceSpecification is mandatory. \n"@en ;
        rdfs:isDefinedBy  <http://purl.org/goodrelations/v1> ;
        rdfs:label        "Unit price specification"@en ;
        rdfs:subClassOf   v1:PriceSpecification ;
        owl:disjointWith  v1:DeliveryChargeSpecification , v1:PaymentChargeSpecification .

s:Person  a              owl:Class ;
        rdfs:subClassOf  v1:BusinessEntity .

foaf:homepage  a            owl:AnnotationProperty , rdf:Property , owl:ObjectProperty , owl:InverseFunctionalProperty ;
        rdfs:comment        "A homepage for some thing." ;
        rdfs:domain         owl:Thing ;
        rdfs:isDefinedBy    foaf: ;
        rdfs:label          "homepage" ;
        rdfs:range          foaf:Document ;
        rdfs:subPropertyOf  foaf:page , foaf:isPrimaryTopicOf ;
        ns2:term_status     "stable" .

v1:appliesToDeliveryMethod
        a                 owl:ObjectProperty ;
        rdfs:comment      "This property specifies the gr:DeliveryMethod to which the gr:DeliveryChargeSpecification applies."@en ;
        rdfs:domain       v1:DeliveryChargeSpecification ;
        rdfs:isDefinedBy  <http://purl.org/goodrelations/v1> ;
        rdfs:label        "applies to delivery method (0..*)"@en ;
        rdfs:range        v1:DeliveryMethod .

v1:DeliveryModeFreight
        a                 v1:DeliveryMethod ;
        rdfs:comment      "Delivery by an unspecified air, sea, or ground freight carrier or cargo company."@en ;
        rdfs:isDefinedBy  <http://purl.org/goodrelations/v1> ;
        rdfs:label        "Delivery mode freight (delivery method)"@en .

v1:quantitativeProductOrServiceProperty
        a                 owl:ObjectProperty ;
        rdfs:comment      "This is the super property of all quantitative  properties for products and services. All properties in product or service ontologies that specify quantitative characteristics, for which an interval is at least theoretically an appropriate value, are subproperties of this property."@en ;
        rdfs:domain       [ a            owl:Class ;
                            owl:unionOf  ( v1:ProductOrService s:Product )
                          ] ;
        rdfs:isDefinedBy  <http://purl.org/goodrelations/v1> ;
        rdfs:label        "quantitative product or service property (0..*)"@en ;
        rdfs:range        v1:QuantitativeValue .

v1:hasPriceSpecification
        a                 owl:ObjectProperty ;
        rdfs:comment      "This links a gr:Offering to a gr:PriceSpecification or specifications. There can be unit price specifications, payment charge specifications, and delivery charge specifications. For each type, multiple specifications for the same gr:Offering are possible, e.g. for different quantity ranges or for different currencies, or for different combinations of gr:DeliveryMethod and target destinations.\n\nRecommended retail prices etc. can be marked by the gr:priceType property of the gr:UnitPriceSpecification."@en ;
        rdfs:domain       [ a            owl:Class ;
                            owl:unionOf  ( v1:Offering s:Offer )
                          ] ;
        rdfs:isDefinedBy  <http://purl.org/goodrelations/v1> , v1: ;
        rdfs:label        "has price specification (0..*)"@en , "Especificación del precio"@es , "Price specification"@en ;
        rdfs:range        v1:PriceSpecification .

v1:Saturday  a              v1:DayOfWeek ;
        rdfs:comment        "Saturday as a day of the week."@en ;
        rdfs:isDefinedBy    <http://purl.org/goodrelations/v1> ;
        rdfs:label          "Saturday (day of week)"@en ;
        v1:displayPosition  6 ;
        v1:hasNext          v1:Sunday ;
        v1:hasPrevious      v1:Friday .

v1:hasBrand  a            owl:ObjectProperty ;
        rdfs:comment      "This specifies the brand or brands (gr:Brand) associated with a gr:ProductOrService, or the brand or brands maintained by a gr:BusinessEntity."@en ;
        rdfs:domain       [ a            owl:Class ;
                            owl:unionOf  ( v1:BusinessEntity v1:ProductOrService s:Organization s:Product )
                          ] ;
        rdfs:isDefinedBy  <http://purl.org/goodrelations/v1> ;
        rdfs:label        "has brand (0..*)"@en ;
        rdfs:range        v1:Brand .

v1:Offering  a            owl:Class ;
        rdfs:comment      "An offering represents the public, not necessarily binding, not necessarily exclusive, announcement by a gr:BusinessEntity to provide (or seek) a certain gr:BusinessFunction for a certain gr:ProductOrService to a specified target audience. An offering is specified by the type of product or service or bundle it refers to, what business function is being offered (sales, rental, ...), and a set of commercial properties. It can either refer to \n(1) a clearly specified instance (gr:Individual),\n(2) to a set of anonymous instances of a given type (gr:SomeItems),\n(3) a product model specification (gr:ProductOrServiceModel), see also section 3.3.3 of the GoodRelations Technical Report. \n\nAn offering may be constrained in terms of the eligible type of business partner, countries, quantities, and other commercial properties. The definition of the commercial properties, the type of product offered, and the business function are explained in other parts of this vocabulary in more detail.\n\nExample: Peter Miller offers to repair TV sets made by Siemens, Volkswagen Innsbruck sells a particular instance of a Volkswagen Golf at $10,000.\n\nCompatibility with schema.org: This class is a superclass to http://schema.org/Offer, since gr:Offering can also represent demand."@en ;
        rdfs:isDefinedBy  <http://purl.org/goodrelations/v1> , v1: ;
        rdfs:label        "Offering"@en , "Oferta"@es ;
        owl:disjointWith  v1:OpeningHoursSpecification , v1:WarrantyPromise , v1:Brand , v1:QuantitativeValue , v1:BusinessFunction , v1:BusinessEntityType , v1:PriceSpecification , v1:DayOfWeek , v1:TypeAndQuantityNode , v1:BusinessEntity , v1:DeliveryMethod , v1:PaymentMethod , v1:Location , v1:QualitativeValue , v1:ProductOrService , v1:WarrantyScope .

v1:WarrantyPromise  a     owl:Class ;
        rdfs:comment      "This is a conceptual entity that holds together all aspects of the n-ary relation gr:hasWarrantyPromise.\n\nA Warranty promise is an entity representing the duration and scope of services that will be provided to a customer free of charge in case of a defect or malfunction of the gr:ProductOrService. A warranty promise is characterized by its temporal duration (usually starting with the date of purchase) and its gr:WarrantyScope. The warranty scope represents the types of services provided (e.g. labor and parts, just parts) of the warranty included in an gr:Offering. The actual services may be provided by the gr:BusinessEntity making the offering, by the manufacturer of the product, or by a third party. There may be multiple warranty promises associated with a particular offering, which differ in duration and scope (e.g. pick-up service during the first 12 months, just parts and labor for 36 months).\n\nExamples: 12 months parts and labor, 36 months parts"@en ;
        rdfs:isDefinedBy  <http://purl.org/goodrelations/v1> ;
        rdfs:label        "Warranty promise"@en ;
        owl:disjointWith  v1:Brand , v1:BusinessFunction , v1:Location , v1:TypeAndQuantityNode , v1:BusinessEntityType , v1:ProductOrService , v1:OpeningHoursSpecification , v1:WarrantyScope , v1:QuantitativeValue , v1:Offering , v1:PriceSpecification , v1:PaymentMethod , v1:DeliveryMethod , v1:DayOfWeek , v1:BusinessEntity .

v1:hasEAN_UCC-13  a         owl:DatatypeProperty ;
        rdfs:comment        "The EAN·UCC-13 code of the given gr:ProductOrService or gr:Offering. This code is now officially called GTIN-13 (Global Trade Identifier Number) or EAN·UCC-13. Former 12-digit UPC codes can be converted into EAN·UCC-13 code by simply adding a preceeding zero.\n\nNote 1: When using this property for searching by 12-digit UPC codes, you must add a preceeding zero digit.\nNote 2: As of January 1, 2007, the former ISBN numbers for books etc. have been integrated into the EAN·UCC-13 code. For each old ISBN-10 code, there exists a proper translation into EAN·UCC-13 by adding \"978\" or \"979\" as prefix. Since the old ISBN-10 is now deprecated, GoodRelations does not provide a property for ISBNs."@en ;
        rdfs:domain         [ a            owl:Class ;
                              owl:unionOf  ( v1:Offering v1:ProductOrService s:Product )
                            ] ;
        rdfs:isDefinedBy    <http://purl.org/goodrelations/v1> ;
        rdfs:label          "has EAN/UCC-13 (0..*)"@en ;
        rdfs:range          xsd:string ;
        rdfs:subPropertyOf  s:productID .

v1:QuantitativeValue  a   owl:Class ;
        rdfs:comment      "A quantitative value is a numerical interval that represents the range of a certain gr:quantitativeProductOrServiceProperty in terms of the lower and upper bounds for a particular gr:ProductOrService. It is to be interpreted in combination with the respective unit of measurement. Most quantitative values are intervals even if they are in practice often treated as a single point value.\n\t\nExample: a weight between 10 and 25 kilogramms, a length between 10 and 15 milimeters.\n\nCompatibility with schema.org: This class is equivalent to http://schema.org/Quantity."@en ;
        rdfs:isDefinedBy  <http://purl.org/goodrelations/v1> ;
        rdfs:label        "Quantitative value"@en ;
        owl:disjointWith  v1:Location , v1:DeliveryMethod , v1:BusinessEntity , v1:WarrantyPromise , v1:PriceSpecification , v1:BusinessEntityType , v1:PaymentMethod , v1:TypeAndQuantityNode , v1:Brand , v1:OpeningHoursSpecification , v1:Offering , v1:QualitativeValue , v1:BusinessFunction , v1:ProductOrService , v1:DayOfWeek , v1:WarrantyScope .

v1:COD  a                 v1:PaymentMethod ;
        rdfs:comment      "Collect on delivery / Cash on delivery - A payment method where the recipient of goods pays at the time of delivery. Usually, the amount of money is collected by the transportation company handling the goods."@en ;
        rdfs:isDefinedBy  <http://purl.org/goodrelations/v1> ;
        rdfs:label        "COD (payment method)"@en .

s:Offer  a               owl:Class ;
        rdfs:subClassOf  v1:Offering .

v1:Dispose  a             v1:BusinessFunction ;
        rdfs:comment      "This gr:BusinessFunction indicates that the gr:BusinessEntity offers (or seeks) the acceptance of the specified gr:ProductOrService for proper disposal, recycling, or any other kind of allowed usages, freeing the current owner from all rights and obligations of ownership."@en ;
        rdfs:isDefinedBy  <http://purl.org/goodrelations/v1> ;
        rdfs:label        "Dispose (business function)"@en .

v1:width  a                 owl:ObjectProperty ;
        rdfs:comment        "The width of the gr:ProductOrService.\nTypical unit code(s): CMT for centimeters, INH for inches"@en ;
        rdfs:domain         [ a            owl:Class ;
                              owl:unionOf  ( v1:ProductOrService s:Product )
                            ] ;
        rdfs:isDefinedBy    <http://purl.org/goodrelations/v1> ;
        rdfs:label          "width (0..1)"@en ;
        rdfs:range          v1:QuantitativeValue ;
        rdfs:subPropertyOf  v1:quantitativeProductOrServiceProperty .

v1:SomeItems  a              owl:Class ;
        rdfs:comment         "A placeholder instance for unknown instances of a mass-produced commodity. This is used as a computationally cheap work-around for such instances that are not individually exposed on the Web but just stated to exist (i.e., which are existentially quantified).\n\nExample: An instance of this class can represent an anonymous set of green Siemens1234 phones. It is different from the gr:ProductOrServiceModel Siemens1234, since this refers to the make and model, and it is different from a particular instance of this make and model (e.g. my individual phone) since the latter can be sold only once.\n\nNote: This class is the new, shorter form of the former gr:ProductOrServicesSomeInstancesPlaceholder.\n\t\t\nCompatibility with schema.org: This class is (approximately) a subclass of http://schema.org/Product."@en ;
        rdfs:isDefinedBy     <http://purl.org/goodrelations/v1> ;
        rdfs:label           "Some items"@en ;
        rdfs:subClassOf      s:Product , v1:ProductOrService ;
        owl:disjointWith     v1:Individual , v1:ProductOrServiceModel ;
        owl:equivalentClass  v1:ProductOrServicesSomeInstancesPlaceholder .

v1:AmericanExpress  a     v1:PaymentMethodCreditCard ;
        rdfs:comment      "Payment by credit or debit cards issued by the American Express network."@en ;
        rdfs:isDefinedBy  <http://purl.org/goodrelations/v1> ;
        rdfs:label        "American Express (payment method)"@en .

v1:LocationOfSalesOrServiceProvisioning
        a                    owl:Class ;
        rdfs:comment         "DEPRECATED - This class is superseded by gr:Location. Replace all occurrences of gr:LocationOfSalesOrServiceProvisioning by gr:Location, if possible."@en ;
        rdfs:isDefinedBy     <http://purl.org/goodrelations/v1> ;
        rdfs:label           "Location of sales or service provisioning (DEPRECATED)"@en ;
        owl:deprecated       true ;
        owl:equivalentClass  v1:Location .

v1:Individual  a             owl:Class ;
        rdfs:comment         "A gr:Individual is an actual product or service instance, i.e., a single identifiable object or action that creates some increase in utility (in the economic sense) for the individual possessing or using this very object (product) or for the individual in whose favor this very action is being taken (service). Products or services are types of goods in the economic sense. For an overview of goods and commodities in economics, see Milgate (1987).\n\nExamples: MyThinkpad T60, the pint of beer standing in front of me, my Volkswagen Golf, the haircut that I received or will be receiving at a given date and time.\n\nNote 1: In many cases, product or service instances are not explicitly exposed on the Web but only claimed to exist (i.e. existentially quantified). In this case, use gr:SomeItems.\nNote 2: This class is the new, shorter form of the former gr:ActualProductOrServiceInstance.\n\nCompatibility with schema.org: This class is a subclass of http://schema.org/Product."@en ;
        rdfs:isDefinedBy     <http://purl.org/goodrelations/v1> ;
        rdfs:label           "Individual"@en ;
        rdfs:subClassOf      s:Product , v1:ProductOrService ;
        owl:disjointWith     v1:ProductOrServiceModel , v1:SomeItems ;
        owl:equivalentClass  v1:ActualProductOrServiceInstance .

v1:deliveryLeadTime  a    owl:ObjectProperty ;
        rdfs:comment      "This property can be used to indicate the promised delay between the receipt of the order and the goods leaving the warehouse.\n\nThe duration is specified by attaching an instance of gr:QuantitativeValueInteger. The lower and upper boundaries are specified using the properties gr:hasMinValueInteger and gr:hasMaxValueInteger to that instance. A point value can be modeled with the gr:hasValueInteger property. The unit of measurement is specified using the property gr:hasUnitOfMeasurement with a string holding a UN/CEFACT code suitable for durations, e.g. MON (months), DAY (days), HUR (hours), or MIN (minutes)."@en ;
        rdfs:domain       [ a            owl:Class ;
                            owl:unionOf  ( v1:Offering s:Offer )
                          ] ;
        rdfs:isDefinedBy  <http://purl.org/goodrelations/v1> ;
        rdfs:label        "delivery lead time (0..1)"@en ;
        rdfs:range        v1:QuantitativeValueInteger .

v1:DayOfWeek  a           owl:Class ;
        rdfs:comment      "The day of the week, used to specify  to which day the opening hours of a gr:OpeningHoursSpecification refer.\n\nExamples: Monday, Tuesday, Wednesday,..."@en ;
        rdfs:isDefinedBy  <http://purl.org/goodrelations/v1> ;
        rdfs:label        "Day of week"@en ;
        owl:disjointWith  v1:PaymentMethod , v1:Brand , v1:OpeningHoursSpecification , v1:Offering , v1:PriceSpecification , v1:Location , v1:DeliveryMethod , v1:WarrantyScope , v1:ProductOrService , v1:TypeAndQuantityNode , v1:WarrantyPromise , v1:BusinessEntityType , v1:BusinessFunction , v1:BusinessEntity , v1:QuantitativeValue .

v1:hasWarrantyScope  a    owl:ObjectProperty ;
        rdfs:comment      "This states the gr:WarrantyScope of a given gr:WarrantyPromise."@en ;
        rdfs:domain       v1:WarrantyPromise ;
        rdfs:isDefinedBy  <http://purl.org/goodrelations/v1> ;
        rdfs:label        "has warranty scope (0..1)"@en ;
        rdfs:range        v1:WarrantyScope .

v1:isListPrice  a         owl:DatatypeProperty ;
        rdfs:comment      "This boolean attribute indicates whether a gr:UnitPriceSpecification is a list price (usually a vendor recommendation) or not. \"true\"  indicates it is a list price, \"false\" indicates it is not.\nDEPRECATED. Use the gr:priceType property instead."@en ;
        rdfs:domain       v1:UnitPriceSpecification ;
        rdfs:isDefinedBy  <http://purl.org/goodrelations/v1> ;
        rdfs:label        "is list price (DEPRECATED)"@en ;
        rdfs:range        xsd:boolean ;
        owl:deprecated    true .

v1:BusinessFunction  a    owl:Class ;
        rdfs:comment      "The business function specifies the type of activity or access (i.e., the bundle of rights) offered by the gr:BusinessEntity on the gr:ProductOrService through the gr:Offering. Typical are sell, rental or lease, maintenance or repair, manufacture / produce, recycle / dispose, engineering / construction, or installation.\n\nLicenses and other proprietary specifications of access rights are also instances of this class.\n\nExamples: A particular offering made by Miller Rentals Ltd. says that they (1) sell Volkswagen Golf convertibles, (2) lease out a particular Ford pick-up truck, and (3) dispose car wrecks of any make and model."@en ;
        rdfs:isDefinedBy  <http://purl.org/goodrelations/v1> ;
        rdfs:label        "Business function"@en ;
        owl:disjointWith  v1:WarrantyPromise , v1:PaymentMethod , v1:PriceSpecification , v1:BusinessEntityType , v1:Location , v1:ProductOrService , v1:Offering , v1:TypeAndQuantityNode , v1:WarrantyScope , v1:OpeningHoursSpecification , v1:QuantitativeValue , v1:BusinessEntity , v1:Brand , v1:DayOfWeek , v1:DeliveryMethod .

v1:priceType  a           owl:DatatypeProperty ;
        rdfs:comment      "This attribute can be used to distinguish multiple different price specifications for the same gr:Offering. It supersedes the former gr:isListPrice property. The following values are recommended:\n\nThe absence of this property marks the actual sales price.\n\nSRP: \"suggested retail price\" - applicable for all sorts of a non-binding retail price recommendations, e.g. such published by the manufacturer or the distributor. This value replaces the former gr:isListPrice property.\n\nINVOICE: The invoice price, mostly used in the car industry - this is the price a dealer pays to the manufacturer, excluding rebates and charges."@en ;
        rdfs:domain       v1:UnitPriceSpecification ;
        rdfs:isDefinedBy  <http://purl.org/goodrelations/v1> ;
        rdfs:label        "price type (0..1)"@en ;
        rdfs:range        xsd:string .

v1:Repair  a              v1:BusinessFunction ;
        rdfs:comment      "This gr:BusinessFunction indicates that the gr:BusinessEntity offers (or seeks) the evaluation of the chances for repairing, and, if positive, repair of the specified gr:ProductOrService. Repairing means actions that restore the originally intended function of a product that suffers from outage or malfunction."@en ;
        rdfs:isDefinedBy  <http://purl.org/goodrelations/v1> ;
        rdfs:label        "Repair (business function)"@en .

s:image  a                      owl:ObjectProperty ;
        rdfs:domain             [ a            owl:Class ;
                                  owl:unionOf  ( owl:Thing acco:Accommodation acco:AccommodationFeature acco:Meal acco:Allinclusive acco:BedType acco:DwellingType acco:CompoundPrice )
                                ] ;
        owl:equivalentProperty  foaf:depiction .

v1:billingIncrement  a    owl:DatatypeProperty ;
        rdfs:comment      "This property specifies the minimal quantity and rounding increment that will be the basis for the billing. \nThe unit of measurement is specified by the UN/CEFACT code attached to the gr:UnitPriceSpecification via the gr:hasUnitOfMeasurement property.\n\nExamples: \n- The price for gasoline is 4 USD per gallon at the pump, but you will be charged in units of 0.1 gallons.\n- The price for legal consulting is 100 USD per hour, but you will be charged in units of 15 minutes.\n\nThis property makes sense only for instances of gr:Offering that include not more than one type of good or service."@en ;
        rdfs:domain       v1:UnitPriceSpecification ;
        rdfs:isDefinedBy  <http://purl.org/goodrelations/v1> ;
        rdfs:label        "billing increment (0..1)"@en ;
        rdfs:range        xsd:float .

v1:CheckInAdvance  a      v1:PaymentMethod ;
        rdfs:comment      "Payment by sending a check in advance, i.e., the offering gr:BusinessEntity will deliver the goods upon receipt of a check over the due amount. There are variations in handling payment by check - sometimes, shipment will be upon receipt of the check as a document, sometimes the shipment will take place only upon successful crediting of the check."@en ;
        rdfs:isDefinedBy  <http://purl.org/goodrelations/v1> ;
        rdfs:label        "Check in advance (payment method)"@en .

v1:PartsAndLabor-PickUp
        a                 v1:WarrantyScope ;
        rdfs:comment      "In case of a defect or malfunction, the buying party has the right to request from the selling gr:Business Entity to pick-up the good from its current location to a suitable service location, where the functionality of the good will be restored. All transportation, labor, parts, and materials needed to fix the problem will be covered by the selling business entity or one of its partnering business entities.\n  \nNote: This is just a rough classification for filtering offers. It is up to the buying party to check the exact scope and terms and conditions of the gr:WarrantyPromise."@en ;
        rdfs:isDefinedBy  <http://purl.org/goodrelations/v1> ;
        rdfs:label        "Parts and labor / pick up (warranty scope)"@en .

v1:PartsAndLabor-BringIn
        a                 v1:WarrantyScope ;
        rdfs:comment      "In case of a defect or malfunction, the buying party has the right to transport the good to a service location determined by the the selling gr:BusinessEntity and will not be be charged for labor, parts, and materials needed to fix the problem. All those costs will be covered by the selling business entity or one of its partnering business entities.\n\nNote: This is just a rough classification for filtering offers. It is up to the buying party to check the exact scope and terms and conditions of the gr:WarrantyPromise."@en ;
        rdfs:isDefinedBy  <http://purl.org/goodrelations/v1> ;
        rdfs:label        "Parts and labor / bring-in (warranty scope)"@en .

v1:description  a         owl:DatatypeProperty ;
        rdfs:comment      "A short textual description of the resource. \n\nThis property is semantically equivalent to rdfs:comment and just meant as a handy shortcut for marking up data."@en ;
        rdfs:domain       [ a            owl:Class ;
                            owl:unionOf  ( owl:Thing v1:Brand v1:BusinessEntity v1:BusinessEntityType v1:BusinessFunction v1:DayOfWeek v1:DeliveryChargeSpecification v1:DeliveryMethod v1:DeliveryModeParcelService v1:Individual v1:Location v1:Offering v1:OpeningHoursSpecification v1:PaymentChargeSpecification v1:PaymentMethod v1:PaymentMethodCreditCard v1:PriceSpecification v1:ProductOrService v1:ProductOrServiceModel v1:QualitativeValue v1:QuantitativeValue v1:QuantitativeValueFloat v1:QuantitativeValueInteger v1:SomeItems v1:TypeAndQuantityNode v1:UnitPriceSpecification v1:WarrantyPromise v1:WarrantyScope )
                          ] ;
        rdfs:domain       [ a            owl:Class ;
                            owl:unionOf  ( owl:Thing acco:Accommodation acco:AccommodationFeature acco:Meal acco:Allinclusive acco:BedType acco:DwellingType acco:CompoundPrice )
                          ] ;
        rdfs:isDefinedBy  <http://purl.org/goodrelations/v1> ;
        rdfs:label        "description (0..1)"@en ;
        rdfs:range        rdfs:Literal .

v1:hasISICv4  a           owl:DatatypeProperty ;
        rdfs:comment      "The International Standard of Industrial Classification of All Economic Activities (ISIC), Revision 4 code for a particular gr:BusinessEntity or gr:Location. See http://unstats.un.org/unsd/cr/registry/isic-4.asp for more information.\n\nNote: While ISIC codes are sometimes misused for classifying products or services, they are designed and suited only for classifying business establishments."@en ;
        rdfs:domain       [ a            owl:Class ;
                            owl:unionOf  ( v1:BusinessEntity v1:Location s:Organization s:Place )
                          ] ;
        rdfs:isDefinedBy  <http://purl.org/goodrelations/v1> ;
        rdfs:label        "has ISIC v4 (0..*)"@en ;
        rdfs:range        xsd:int .

v1:isAccessoryOrSparePartFor
        a                 owl:ObjectProperty ;
        rdfs:comment      "This states that a particular gr:ProductOrService is an accessory or spare part for another product or service."@en ;
        rdfs:domain       [ a            owl:Class ;
                            owl:unionOf  ( v1:ProductOrService s:Product )
                          ] ;
        rdfs:isDefinedBy  <http://purl.org/goodrelations/v1> ;
        rdfs:label        "is accessory or spare part for (0..*)"@en ;
        rdfs:range        v1:ProductOrService .

v1:weight  a                owl:ObjectProperty ;
        rdfs:comment        "The weight of the gr:ProductOrService.\nTypical unit code(s): GRM for gram, KGM for kilogram, LBR for pound"@en ;
        rdfs:domain         [ a            owl:Class ;
                              owl:unionOf  ( v1:ProductOrService s:Product )
                            ] ;
        rdfs:isDefinedBy    <http://purl.org/goodrelations/v1> ;
        rdfs:label          "weight (0..1)"@en ;
        rdfs:range          v1:QuantitativeValue ;
        rdfs:subPropertyOf  v1:quantitativeProductOrServiceProperty .

v1:lesser  a              owl:TransitiveProperty , owl:ObjectProperty ;
        rdfs:comment      "This ordering relation for gr:QualitativeValue pairs indicates that the subject is lesser than the object."@en ;
        rdfs:domain       v1:QualitativeValue ;
        rdfs:isDefinedBy  <http://purl.org/goodrelations/v1> ;
        rdfs:label        "lesser (0..*)"@en ;
        rdfs:range        v1:QualitativeValue ;
        owl:inverseOf     v1:greater .

v1:Sell  a                v1:BusinessFunction ;
        rdfs:comment      "This gr:BusinessFunction indicates that the gr:BusinessEntity offers to permanently transfer all property rights on the specified gr:ProductOrService."@en ;
        rdfs:isDefinedBy  <http://purl.org/goodrelations/v1> ;
        rdfs:label        "Sell (business function)"@en .

v1:hasMinValueFloat  a      owl:DatatypeProperty ;
        rdfs:comment        "This property captures the lower limit of a gr:QuantitativeValueFloat instance."@en ;
        rdfs:domain         v1:QuantitativeValueFloat ;
        rdfs:isDefinedBy    <http://purl.org/goodrelations/v1> ;
        rdfs:label          "has min value float (1..1)"@en ;
        rdfs:range          xsd:float ;
        rdfs:subPropertyOf  v1:hasMinValue .

v1:PriceSpecification
        a                 owl:Class ;
        rdfs:comment      "The superclass of all price specifications."@en ;
        rdfs:isDefinedBy  <http://purl.org/goodrelations/v1> , v1: ;
        rdfs:label        "Price specification"@en , "Especificación del precio"@es ;
        owl:disjointWith  v1:Location , v1:DayOfWeek , v1:PaymentMethod , v1:BusinessEntity , v1:Brand , v1:ProductOrService , v1:BusinessFunction , v1:TypeAndQuantityNode , v1:BusinessEntityType , v1:DeliveryMethod , v1:WarrantyPromise , v1:QuantitativeValue , v1:WarrantyScope , v1:OpeningHoursSpecification , v1:Offering .

s:name  a                       owl:DatatypeProperty ;
        rdfs:isDefinedBy        s: ;
        rdfs:label              "Nombre"@es , "Name"@en ;
        owl:equivalentProperty  v1:name .

v1:seeks  a               owl:ObjectProperty ;
        rdfs:comment      "This links a gr:BusinessEntity to gr:Offering nodes that describe what the business entity is interested in (i.e., the buy side). If you want to express interest in offering something, use gr:offers instead. Note that this substitutes the former gr:BusinessFunction gr:Buy, which is now deprecated."@en ;
        rdfs:domain       [ a            owl:Class ;
                            owl:unionOf  ( v1:BusinessEntity s:Organization s:Person )
                          ] ;
        rdfs:isDefinedBy  <http://purl.org/goodrelations/v1> ;
        rdfs:label        "seeks (0..*)"@en ;
        rdfs:range        v1:Offering .

v1:eligibleCustomerTypes
        a                 owl:ObjectProperty ;
        rdfs:comment      "The types of customers (gr:BusinessEntityType) for which the given gr:Offering is valid."@en ;
        rdfs:domain       [ a            owl:Class ;
                            owl:unionOf  ( v1:Offering s:Offer )
                          ] ;
        rdfs:isDefinedBy  <http://purl.org/goodrelations/v1> ;
        rdfs:label        "eligible customer types (0..*)"@en ;
        rdfs:range        v1:BusinessEntityType .

s:Place  a                   owl:Class ;
        rdfs:isDefinedBy     s: ;
        rdfs:label           "Lugar"@es , "Place"@en ;
        owl:equivalentClass  v1:Location .

v1:hasMaxValueInteger
        a                   owl:DatatypeProperty ;
        rdfs:comment        "This property captures the upper limit of a gr:QuantitativeValueInteger instance."@en ;
        rdfs:domain         v1:QuantitativeValueInteger ;
        rdfs:isDefinedBy    <http://purl.org/goodrelations/v1> ;
        rdfs:label          "has max value integer (1..1)"@en ;
        rdfs:range          xsd:int ;
        rdfs:subPropertyOf  v1:hasMaxValue .

v1:includes  a            owl:ObjectProperty ;
        rdfs:comment      "This object property is a shortcut for the original gr:includesObject property for the common case of having exactly one single gr:ProductOrService instance included in an Offering. \n\nWhen linking to an instance of gr:SomeItems or gr:Individual, it is equivalent to using a gr:TypeAndQuantityNode with gr:hasUnitOfMeasurement=\"C62\"^^xsd:string and gr:amountOfThisGood=\"1.0\"^^xsd:float for that good.\n\nWhen linking to a gr:ProductOrServiceModel, it is equivalent to \n1. defining an blank node for a gr:SomeItems\n2. linking that blank node via gr:hasMakeAndModel to the gr:ProductOrServiceModel, and\n3. linking from the gr:Offering to that blank node using another blank node of type gr:TypeAndQuantityNode with gr:hasUnitOfMeasurement=\"C62\"^^xsd:string and gr:amountOfThisGood=\"1.0\"^^xsd:float for that good."@en ;
        rdfs:domain       v1:Offering ;
        rdfs:isDefinedBy  <http://purl.org/goodrelations/v1> ;
        rdfs:label        "includes (0..1)"@en ;
        rdfs:range        v1:ProductOrService .

v1:hasBusinessFunction
        a                 owl:ObjectProperty ;
        rdfs:comment      "This specifies the business function of the gr:Offering, i.e. whether the gr:BusinessEntity is offering to sell, to lease, or to repair the particular type of product. In the case of bundles, it is also possible to attach individual business functions to each gr:TypeAndQuantityNode. The business function of the main gr:Offering determines the business function for all included objects or services, unless a business function attached to a gr:TypeAndQuantityNode overrides it.\n\t\nNote: While it is possible that an entity is offering multiple types of business functions for the same set of objects (e.g. rental and sales), this should usually not be stated by attaching multiple business functions to the same gr:Offering, since the gr:UnitPriceSpecification for the varying business functions will typically be very different."@en ;
        rdfs:domain       [ a            owl:Class ;
                            owl:unionOf  ( v1:Offering v1:TypeAndQuantityNode s:Offer )
                          ] ;
        rdfs:isDefinedBy  <http://purl.org/goodrelations/v1> ;
        rdfs:label        "has business function (1..*)"@en ;
        rdfs:range        v1:BusinessFunction .

v1:hasMaxValue  a         owl:DatatypeProperty ;
        rdfs:comment      "This property captures the upper limit of a gr:QuantitativeValue instance."@en ;
        rdfs:domain       v1:QuantitativeValue ;
        rdfs:isDefinedBy  <http://purl.org/goodrelations/v1> ;
        rdfs:label        "has max value (0..1)"@en ;
        rdfs:range        rdfs:Literal .

v1:hasGTIN-8  a             owl:DatatypeProperty ;
        rdfs:comment        "The 8-digit Global Trade Item Number (GTIN-8) of the given gr:ProductOrService or gr:Offering, also known as EAN/UCC-8 (8-digit EAN)."@en ;
        rdfs:domain         [ a            owl:Class ;
                              owl:unionOf  ( v1:Offering v1:ProductOrService s:Product )
                            ] ;
        rdfs:isDefinedBy    <http://purl.org/goodrelations/v1> ;
        rdfs:label          "has GTIN-8 (0..*)"@en ;
        rdfs:range          xsd:string ;
        rdfs:subPropertyOf  s:productID .

v1:DeliveryModeDirectDownload
        a                 v1:DeliveryMethod ;
        rdfs:comment      "Delivery of the goods via direct download from the Internet, i.e., the offering gr:BusinessEntity provides the buying party with details on how to retrieve the goods online. Connection fees and other costs of using the infrastructure are to be carried by the buying party."@en ;
        rdfs:isDefinedBy  <http://purl.org/goodrelations/v1> ;
        rdfs:label        "Delivery mode direct download (delivery method)"@en .

v1:Tuesday  a               v1:DayOfWeek ;
        rdfs:comment        "Tuesday as a day of the week."@en ;
        rdfs:isDefinedBy    <http://purl.org/goodrelations/v1> ;
        rdfs:label          "Tuesday (day of week)"@en ;
        v1:displayPosition  2 ;
        v1:hasNext          v1:Wednesday ;
        v1:hasPrevious      v1:Monday .

v1:typeOfGood  a          owl:ObjectProperty ;
        rdfs:comment      "This specifies the gr:ProductOrService that the gr:TypeAndQuantityNode is referring to."@en ;
        rdfs:domain       v1:TypeAndQuantityNode ;
        rdfs:isDefinedBy  <http://purl.org/goodrelations/v1> ;
        rdfs:label        "type of good (1..1)"@en ;
        rdfs:range        [ a            owl:Class ;
                            owl:unionOf  ( v1:Individual v1:SomeItems )
                          ] .

v1:hasNAICS  a            owl:DatatypeProperty ;
        rdfs:comment      "The North American Industry Classification System (NAICS) code for a particular gr:BusinessEntity.\nSee http://www.census.gov/eos/www/naics/ for more details.\n\nNote: While NAICS codes are sometimes misused for classifying products or services, they are designed and suited only for classifying business establishments."@en ;
        rdfs:domain       [ a            owl:Class ;
                            owl:unionOf  ( v1:BusinessEntity s:Organization )
                          ] ;
        rdfs:isDefinedBy  <http://purl.org/goodrelations/v1> ;
        rdfs:label        "has NAICS (0..*)"@en ;
        rdfs:range        xsd:int .

v1:opens  a               owl:DatatypeProperty ;
        rdfs:comment      "The opening hour of the gr:Location on the given gr:DayOfWeek.\nIf no time-zone suffix is included, the time is given in the local time valid at the gr:Location.\n\nFor a time in GMT/UTC, simply add a \"Z\" following the time:\n\n09:30:10Z.\n\nAlternatively, you can specify an offset from the UTC time by adding a positive or negative time following the time:\n\n09:30:10-09:00\n\nor\n\n09:30:10+09:00.\n\nNote 1: Use 00:00:00 for the first second of the respective day and 23:59:59 for the last second of that day.\nNote 2: If a store opens at 17:00 on Saturdays and closes at 03:00:00 a.m. next morning, use 17:00:00 - 23:59:59 for Saturday and 00:00:00 - 03:00:00 for Sunday.\nNote 3: If the shop re-opens on the same day of the week or set of days of the week, you must create a second instance of gr:OpeningHoursSpecification."@en ;
        rdfs:domain       v1:OpeningHoursSpecification ;
        rdfs:isDefinedBy  <http://purl.org/goodrelations/v1> ;
        rdfs:label        "opens (1..1)"@en ;
        rdfs:range        xsd:time .

v1:hasMinValue  a         owl:DatatypeProperty ;
        rdfs:comment      "This property captures the lower limit of a gr:QuantitativeValue instance."@en ;
        rdfs:domain       v1:QuantitativeValue ;
        rdfs:isDefinedBy  <http://purl.org/goodrelations/v1> ;
        rdfs:label        "has min value (0..1)"@en ;
        rdfs:range        rdfs:Literal .

owl:deprecated  a  owl:AnnotationProperty .

v1:valueReference  a      owl:ObjectProperty ;
        rdfs:comment      "The superclass of properties that link a gr:QuantitativeValue or a gr:QualitativeValue to a second gr:QuantitativeValue or a gr:QualitativeValue that provides additional information on the original value. A good modeling practice is to define specializations of this property (e.g. foo:referenceTemperature) for your particular domain."@en ;
        rdfs:domain       [ a            owl:Class ;
                            owl:unionOf  ( v1:QualitativeValue v1:QuantitativeValue )
                          ] ;
        rdfs:isDefinedBy  <http://purl.org/goodrelations/v1> ;
        rdfs:label        "value reference (0..*)"@en ;
        rdfs:range        [ a            owl:Class ;
                            owl:unionOf  ( v1:QualitativeValue v1:QuantitativeValue )
                          ] .

v1:Location  a               owl:Class ;
        rdfs:comment         "A location is a point or area of interest from which a particular product or service is available, e.g. a store, a bus stop, a gas station, or a ticket booth. The difference to gr:BusinessEntity is that the gr:BusinessEntity is the legal entity (e.g. a person or corporation) making the offer, while gr:Location is the store, office, or place. A chain restaurant will e.g. have one legal entity but multiple restaurant locations. Locations are characterized by an address or geographical position and a set of opening hour specifications for various days of the week.\n\t\t\nExample: A rental car company may offer the Business Function Lease Out of cars from two locations, one in Fort Myers, Florida, and one in Boston, Massachussetts. Both stations are open 7:00 - 23:00 Mondays through Saturdays.\n\nNote: Typical address standards (vcard) and location data (geo, WGC84) should be attached to a gr:Location node. Since there already exist established vocabularies for this, the GoodRelations ontology does not provide respective attributes. Instead, the use of respective vocabularies is recommended. However, the gr:hasGlobalLocationNumber property is  provided for linking to public identifiers for business locations.\n\t\t\nCompatibility with schema.org: This class is equivalent to http://schema.org/Place."@en ;
        rdfs:isDefinedBy     <http://purl.org/goodrelations/v1> ;
        rdfs:label           "Location"@en ;
        owl:disjointWith     v1:Brand , v1:BusinessFunction , v1:PriceSpecification , v1:TypeAndQuantityNode , v1:WarrantyPromise , v1:Offering , v1:BusinessEntity , v1:WarrantyScope , v1:OpeningHoursSpecification , v1:DayOfWeek , v1:PaymentMethod , v1:DeliveryMethod , v1:QuantitativeValue , v1:BusinessEntityType ;
        owl:equivalentClass  v1:LocationOfSalesOrServiceProvisioning .

v1:hasWarrantyPromise
        a                 owl:ObjectProperty ;
        rdfs:comment      "This specifies the gr:WarrantyPromise made by the gr:BusinessEntity for the given gr:Offering."@en ;
        rdfs:domain       [ a            owl:Class ;
                            owl:unionOf  ( v1:Offering s:Offer )
                          ] ;
        rdfs:isDefinedBy  <http://purl.org/goodrelations/v1> ;
        rdfs:label        "has warranty promise (0..*)"@en ;
        rdfs:range        v1:WarrantyPromise .

v1:hasOpeningHoursSpecification
        a                 owl:ObjectProperty ;
        rdfs:comment      "This property links a gr:Location to a gr:OpeningHoursSpecification."@en ;
        rdfs:domain       [ a            owl:Class ;
                            owl:unionOf  ( v1:Location s:Place )
                          ] ;
        rdfs:isDefinedBy  <http://purl.org/goodrelations/v1> ;
        rdfs:label        "has opening hours specification (0..*)"@en ;
        rdfs:range        v1:OpeningHoursSpecification .

v1:availableAtOrFrom  a   owl:ObjectProperty ;
        rdfs:comment      "This states that a particular gr:Offering is available at or from the given gr:Location (e.g. shop or branch)."@en ;
        rdfs:domain       [ a            owl:Class ;
                            owl:unionOf  ( v1:Offering s:Offer )
                          ] ;
        rdfs:isDefinedBy  <http://purl.org/goodrelations/v1> ;
        rdfs:label        "available at or from (0..*)"@en ;
        rdfs:range        v1:Location .

v1:PaySwarm  a            v1:PaymentMethod ;
        rdfs:comment      "Payment via the PaySwarm distributed micropayment service."@en ;
        rdfs:isDefinedBy  <http://purl.org/goodrelations/v1> ;
        rdfs:label        "PaySwarm (payment method)"@en .

v1:hasMinValueInteger
        a                   owl:DatatypeProperty ;
        rdfs:comment        "This property captures the lower limit of a gr:QuantitativeValueInteger instance."@en ;
        rdfs:domain         v1:QuantitativeValueInteger ;
        rdfs:isDefinedBy    <http://purl.org/goodrelations/v1> ;
        rdfs:label          "has min value integer (1..1)"@en ;
        rdfs:range          xsd:int ;
        rdfs:subPropertyOf  v1:hasMinValue .

v1:PublicInstitution  a   v1:BusinessEntityType ;
        rdfs:comment      "The gr:BusinessEntityType representing such agents that are part of the adminstration or owned by the public."@en ;
        rdfs:isDefinedBy  <http://purl.org/goodrelations/v1> ;
        rdfs:label        "Public institution (business entity type)"@en .

v1:displayPosition  a     owl:AnnotationProperty ;
        rdfs:comment      "The position at which the option or element should be listed in a menu or user dialog, lower numbers come first.\n\nThe main usage of this property are the days of the week (gr:DayOfWeek), but it is also possible to apply it e.g. to product features or any other conceptual element.\nNote: Rely on this property only for data originating from a single RDF graph; otherwise, unpredictable results are possible."@en ;
        rdfs:isDefinedBy  <http://purl.org/goodrelations/v1> ;
        rdfs:label        "display position (0..1)"@en .

v1:DeliveryModePickUp
        a                 v1:DeliveryMethod ;
        rdfs:comment      "Delivery of the goods by picking them up at one of the stores etc. (gr:Location) during the opening hours as specified by respective instances of gr:OpeningHoursSpecification."@en ;
        rdfs:isDefinedBy  <http://purl.org/goodrelations/v1> ;
        rdfs:label        "Delivery mode pick up (delivery method)"@en .

v1:OpeningHoursSpecification
        a                 owl:Class ;
        rdfs:comment      "This is a conceptual entity that holds together all information about the opening hours on a given day (gr:DayOfWeek)."@en ;
        rdfs:isDefinedBy  <http://purl.org/goodrelations/v1> ;
        rdfs:label        "Opening hours specification"@en ;
        owl:disjointWith  v1:BusinessEntity , v1:DayOfWeek , v1:BusinessFunction , v1:WarrantyScope , v1:TypeAndQuantityNode , v1:WarrantyPromise , v1:ProductOrService , v1:PaymentMethod , v1:Brand , v1:PriceSpecification , v1:DeliveryMethod , v1:Offering , v1:BusinessEntityType , v1:QuantitativeValue , v1:Location .

v1:amountOfThisGood  a    owl:DatatypeProperty ;
        rdfs:comment      "This property specifies the quantity of the goods included in the gr:Offering via this gr:TypeAndQuantityNode. The quantity is given in the unit of measurement attached to the gr:TypeAndQuantityNode."@en ;
        rdfs:domain       v1:TypeAndQuantityNode ;
        rdfs:isDefinedBy  <http://purl.org/goodrelations/v1> ;
        rdfs:label        "amount of this good (1..1)"@en ;
        rdfs:range        xsd:float .

v1:BusinessEntityType
        a                 owl:Class ;
        rdfs:comment      "A business entity type is a conceptual entity representing the legal form, the size, the main line of business, the position in the value chain, or any combination thereof, of a gr:BusinessEntity. From the ontological point of view, business entity types are mostly roles that a business entity has in the market. Business entity types are important for specifying eligible customers, since a gr:Offering is often valid only for business entities of a certain size, legal structure, or role in the value chain. \n\nExamples: Consumers, Retailers, Wholesalers, or Public Institutions"@en ;
        rdfs:isDefinedBy  <http://purl.org/goodrelations/v1> ;
        rdfs:label        "Business entity type"@en ;
        owl:disjointWith  v1:BusinessFunction , v1:PriceSpecification , v1:OpeningHoursSpecification , v1:Brand , v1:WarrantyScope , v1:DeliveryMethod , v1:BusinessEntity , v1:Offering , v1:TypeAndQuantityNode , v1:PaymentMethod , v1:QuantitativeValue , v1:Location , v1:DayOfWeek , v1:WarrantyPromise , v1:ProductOrService .

s:manufacturer  a               owl:ObjectProperty ;
        owl:equivalentProperty  v1:hasManufacturer .

v1:nonEqual  a            owl:SymmetricProperty , owl:ObjectProperty ;
        rdfs:comment      "This ordering relation for gr:QualitativeValue pairs indicates that the subject is not equal to the object."@en ;
        rdfs:domain       v1:QualitativeValue ;
        rdfs:isDefinedBy  <http://purl.org/goodrelations/v1> ;
        rdfs:label        "non equal (0..*)"@en ;
        rdfs:range        v1:QualitativeValue ;
        owl:inverseOf     v1:nonEqual .

v1:DeliveryModeOwnFleet
        a                 v1:DeliveryMethod ;
        rdfs:comment      "Delivery of the goods by using a fleet of vehicles either owned and operated or subcontracted by the gr:BusinessEntity."@en ;
        rdfs:isDefinedBy  <http://purl.org/goodrelations/v1> ;
        rdfs:label        "Delivery mode own fleet (delivery method)"@en .

v1:hasValueFloat  a         owl:DatatypeProperty ;
        rdfs:comment        "This subproperty specifies that the upper and lower limit of the given gr:QuantitativeValueFloat are identical and have the respective float value. It is a shortcut for such cases where a quantitative property is (at least practically) a single point value and not an interval."@en ;
        rdfs:domain         v1:QuantitativeValueFloat ;
        rdfs:isDefinedBy    <http://purl.org/goodrelations/v1> ;
        rdfs:label          "has value float (0..1)"@en ;
        rdfs:range          xsd:float ;
        rdfs:subPropertyOf  v1:hasMinValueFloat , v1:hasMaxValueFloat .

v1:hasMaxValueFloat  a      owl:DatatypeProperty ;
        rdfs:comment        "This property captures the upper limit of a gr:QuantitativeValueFloat instance."@en ;
        rdfs:domain         v1:QuantitativeValueFloat ;
        rdfs:isDefinedBy    <http://purl.org/goodrelations/v1> ;
        rdfs:label          "has max value float (1..1)"@en ;
        rdfs:range          xsd:float ;
        rdfs:subPropertyOf  v1:hasMaxValue .

v1:availabilityEnds  a    owl:DatatypeProperty ;
        rdfs:comment      "This property specifies the end of the availability of the gr:ProductOrService included in the gr:Offering.\nThe difference to the properties gr:validFrom and gr:validThrough is that those specify the period of time during which the offer is valid and can be accepted.\n\nExample: I offer to lease my boat for the period of August 1 - August 31, 2010, but you must accept by offer no later than July 15.\n\nA time-zone should be specified. For a time in GMT/UTC, simply add a \"Z\" following the time:\n\n2008-05-30T09:30:10Z.\n\nAlternatively, you can specify an offset from the UTC time by adding a positive or negative time following the time:\n\n2008-05-30T09:30:10-09:00\n\nor\n\n2008-05-30T09:30:10+09:00.\n\nNote: There is another property gr:availableAtOrFrom, which is used to indicate the gr:Location (e.g. store or shop) from which the goods would be available."@en ;
        rdfs:domain       [ a            owl:Class ;
                            owl:unionOf  ( v1:Offering s:Offer )
                          ] ;
        rdfs:isDefinedBy  <http://purl.org/goodrelations/v1> ;
        rdfs:label        "availability ends (0..1)"@en ;
        rdfs:range        xsd:dateTime .

v1:VISA  a                v1:PaymentMethodCreditCard ;
        rdfs:comment      "Payment by credit or debit cards issued by the VISA network."@en ;
        rdfs:isDefinedBy  <http://purl.org/goodrelations/v1> ;
        rdfs:label        "VISA (payment method)"@en .

v1:Buy  a                 v1:BusinessFunction ;
        rdfs:comment      "This gr:BusinessFunction indicates that the gr:BusinessEntity is in general interested in purchasing the specified gr:ProductOrService.\nDEPRECATED. Use gr:seeks instead."@en ;
        rdfs:isDefinedBy  <http://purl.org/goodrelations/v1> ;
        rdfs:label        "Buy (business function, DEPRECATED)"@en ;
        owl:deprecated    true .

v1:offers  a              owl:ObjectProperty ;
        rdfs:comment      "This links a gr:BusinessEntity to the offers (gr:Offering) it makes. If you want to express interest in receiving offers, use gr:seeks instead."@en ;
        rdfs:domain       [ a            owl:Class ;
                            owl:unionOf  ( v1:BusinessEntity s:Organization )
                          ] ;
        rdfs:isDefinedBy  <http://purl.org/goodrelations/v1> ;
        rdfs:label        "offers (0..*)"@en ;
        rdfs:range        v1:Offering .

v1:PaymentChargeSpecification
        a                 owl:Class ;
        rdfs:comment      "A payment charge specification is a conceptual entity that specifies the additional costs asked for settling the payment after accepting a given gr:Offering using a particular gr:PaymentMethod. A payment charge specification is characterized by (1) a monetary amount per order specified as a literal value of type float in combination with a Currency, (2) the payment method, and (3) a whether this charge includes local sales taxes, namely VAT.\nA gr:Offering may be linked to multiple payment charge specifications that specify alternative charges for various payment methods.\n\nExamples: Payment by VISA or Mastercard costs a fee of 3 Euros including VAT, payment by bank transfer in advance is free of charge.\n\nThe total amount of this surcharge is specified as a float value of the gr:hasCurrencyValue property. The currency is specified via the gr:hasCurrency datatype property. Whether the price includes VAT or not is indicated by the gr:valueAddedTaxIncluded datatype property. The gr:PaymentMethod to which this charge applies is specified using the gr:appliesToPaymentMethod object property.\n\nIf the price can only be given as a range, use gr:hasMaxCurrencyValue and gr:hasMinCurrencyValue for the upper and lower bounds.\n\nImportant: When querying for the price, always use gr:hasMaxCurrencyValue and gr:hasMinCurrencyValue."@en ;
        rdfs:isDefinedBy  <http://purl.org/goodrelations/v1> ;
        rdfs:label        "Payment charge specification"@en ;
        rdfs:subClassOf   v1:PriceSpecification ;
        owl:disjointWith  v1:DeliveryChargeSpecification , v1:UnitPriceSpecification .

v1:hasManufacturer  a     owl:ObjectProperty ;
        rdfs:comment      "This object property links a gr:ProductOrService to the gr:BusinessEntity that produces it. Mostly used with gr:ProductOrServiceModel."@en ;
        rdfs:domain       [ a            owl:Class ;
                            owl:unionOf  ( v1:ProductOrService s:Product )
                          ] ;
        rdfs:isDefinedBy  <http://purl.org/goodrelations/v1> ;
        rdfs:label        "has manufacturer (0..1)"@en ;
        rdfs:range        v1:BusinessEntity .

v1:Labor-BringIn  a       v1:WarrantyScope ;
        rdfs:comment      "In case of a defect or malfunction, the buying party has the right to transport the good to a service location determined by the the selling gr:BusinessEntity and will be charged only for parts and materials needed to fix the problem. Labor will be covered by the selling business entity or one of its partnering business entities.\n\nNote: This is just a rough classification for filtering offers. It is up to the buying party to check the exact scope and terms and conditions of the gr:WarrantyPromise."@en ;
        rdfs:isDefinedBy  <http://purl.org/goodrelations/v1> ;
        rdfs:label        "Labor / bring-in (warranty scope)"@en .

[ a               v1:Offering ;
  v1:category     "42" ;
  v1:description  "VGhlIFNldmVuIE5vYWhpZGUgTGF3cw0KMS4gQmVsaWVmIGluIEctZA0KMi4gUmVzcGVjdCBHLWQgYW5kIHByYWlzZSBoaW0NCjMuIFJlc3BlY3QgaHVtYW4gbGlmZQ0KNC4gUmVzcGVjdCB0aGUgZmFtaWx5DQo1LiBSZXNwZWN0IGh1bWFuIGJlaW5ncw0KNi4gSGF2ZSBhIGp1ZGljaWFsIHN5c3RlbQ0KNy4gUmVzcGVjdCBhbGwgY3JlYXR1cmVz"
] .

v1:acceptedPaymentMethods
        a                 owl:ObjectProperty ;
        rdfs:comment      "The gr:PaymentMethod or methods accepted by the gr:BusinessEntity for the given gr:Offering."@en ;
        rdfs:domain       [ a            owl:Class ;
                            owl:unionOf  ( v1:Offering s:Offer )
                          ] ;
        rdfs:isDefinedBy  <http://purl.org/goodrelations/v1> ;
        rdfs:label        "accepted payment methods (0..*)"@en ;
        rdfs:range        v1:PaymentMethod .

v1:GoogleCheckout  a      v1:PaymentMethod ;
        rdfs:comment      "Payment via the Google Checkout payment service."@en ;
        rdfs:isDefinedBy  <http://purl.org/goodrelations/v1> ;
        rdfs:label        "Google Checkout (payment method)"@en .

v1:addOn  a               owl:ObjectProperty ;
        rdfs:comment      "This property points from a gr:Offering to additional offerings that can only be obtained in combination with the first offering. This can be used to model supplements and extensions that are available for a surcharge. Any gr:PriceSpecification attached to the secondary offering is to be understood as an additional charge."@en ;
        rdfs:domain       [ a            owl:Class ;
                            owl:unionOf  ( v1:Offering s:Offer )
                          ] ;
        rdfs:isDefinedBy  <http://purl.org/goodrelations/v1> ;
        rdfs:label        "add-on (0..*)"@en ;
        rdfs:range        v1:Offering .

v1:hasMakeAndModel  a     owl:ObjectProperty ;
        rdfs:comment      "This states that an actual product instance (gr:Individual) or a placeholder instance for multiple, unidentified such instances (gr:SomeItems) is one occurence of a particular gr:ProductOrServiceModel.\n\nExample: myFordT hasMakeAndModel FordT."@en ;
        rdfs:domain       [ a            owl:Class ;
                            owl:unionOf  ( v1:Individual v1:SomeItems s:Product )
                          ] ;
        rdfs:isDefinedBy  <http://purl.org/goodrelations/v1> ;
        rdfs:label        "has make and model (0..1)"@en ;
        rdfs:range        v1:ProductOrServiceModel .

dc:rights  a    owl:AnnotationProperty .

v1:hasDUNS  a             owl:DatatypeProperty ;
        rdfs:comment      "The Dun & Bradstreet DUNS number for identifying a gr:BusinessEntity. The Dun & Bradstreet DUNS is a nine-digit number used to identify legal entities (but usually not branches or locations of logistical importance only)."@en ;
        rdfs:domain       [ a            owl:Class ;
                            owl:unionOf  ( v1:BusinessEntity s:Organization )
                          ] ;
        rdfs:isDefinedBy  <http://purl.org/goodrelations/v1> ;
        rdfs:label        "has DUNS (0..1)"@en ;
        rdfs:range        xsd:string .

s:Product  a                 owl:Class ;
        owl:equivalentClass  v1:ProductOrService .

v1:DHL  a                 v1:DeliveryModeParcelService ;
        rdfs:comment      "Delivery via the parcel service DHL."@en ;
        rdfs:isDefinedBy  <http://purl.org/goodrelations/v1> ;
        rdfs:label        "DHL (delivery method)"@en .

v1:hasInventoryLevel  a   owl:ObjectProperty ;
        rdfs:comment      "This property specifies the current approximate inventory level for gr:SomeItems. The unit of measurement and the point value or interval are indicated using the attached gr:QuantitativeValueFloat instance.\n\nThis property can also be attached to a gr:Offering in cases where the included products are not modeled in more detail."@en ;
        rdfs:domain       [ a            owl:Class ;
                            owl:unionOf  ( v1:Offering v1:SomeItems s:Offer )
                          ] ;
        rdfs:isDefinedBy  <http://purl.org/goodrelations/v1> ;
        rdfs:label        "has inventory level (0..1)"@en ;
        rdfs:range        v1:QuantitativeValueFloat .

v1:Thursday  a              v1:DayOfWeek ;
        rdfs:comment        "Thursday as a day of the week."@en ;
        rdfs:isDefinedBy    <http://purl.org/goodrelations/v1> ;
        rdfs:label          "Thursday (day of week)"@en ;
        v1:displayPosition  4 ;
        v1:hasNext          v1:Friday ;
        v1:hasPrevious      v1:Wednesday .

v1:serialNumber  a        owl:DatatypeProperty ;
        rdfs:comment      "The serial number or any alphanumeric identifier of a particular product. Note that serial number are unique only for the same brand or the same model, so you cannot infer from two occurrences of the same serial number that the objects to which they are attached are identical.\n\nThis property can also be attached to a gr:Offering in cases where the included products are not modeled in more detail."@en ;
        rdfs:domain       [ a            owl:Class ;
                            owl:unionOf  ( v1:Individual v1:Offering s:Product )
                          ] ;
        rdfs:isDefinedBy  <http://purl.org/goodrelations/v1> ;
        rdfs:label        "serial number (0..*)"@en ;
        rdfs:range        xsd:string .

v1:ActualProductOrServiceInstance
        a                    owl:Class ;
        rdfs:comment         "DEPRECATED - This class is superseded by gr:Individual. Replace all occurrences of gr:ActualProductOrServiceInstance by gr:Individual, if possible."@en ;
        rdfs:isDefinedBy     <http://purl.org/goodrelations/v1> ;
        rdfs:label           "Actual product or service instance (DEPRECATED)"@en ;
        rdfs:subClassOf      v1:ProductOrService ;
        owl:deprecated       true ;
        owl:equivalentClass  v1:Individual .

v1:height  a                owl:ObjectProperty ;
        rdfs:comment        "The height of the product.\nTypical unit code(s): CMT for centimeters, INH for inches"@en ;
        rdfs:domain         [ a            owl:Class ;
                              owl:unionOf  ( v1:ProductOrService s:Product )
                            ] ;
        rdfs:isDefinedBy    <http://purl.org/goodrelations/v1> ;
        rdfs:label          "height (0..1)"@en ;
        rdfs:range          v1:QuantitativeValue ;
        rdfs:subPropertyOf  v1:quantitativeProductOrServiceProperty .

v1:DeliveryModeParcelService
        a                 owl:Class ;
        rdfs:comment      "A private parcel service as the delivery mode available for a certain offering.\n\nExamples: UPS, DHL"@en ;
        rdfs:isDefinedBy  <http://purl.org/goodrelations/v1> ;
        rdfs:label        "Delivery mode parcel service"@en ;
        rdfs:subClassOf   v1:DeliveryMethod .

s:description  a                owl:DatatypeProperty ;
        owl:equivalentProperty  v1:description .

dc:subject  a   owl:AnnotationProperty .

v1:Business  a            v1:BusinessEntityType ;
        rdfs:comment      "The gr:BusinessEntityType representing such agents that are themselves offering commercial services or products on the market. Usually, businesses are characterized by the fact that they are officially registered with the public administration and strive for profits by their activities."@en ;
        rdfs:isDefinedBy  <http://purl.org/goodrelations/v1> ;
        rdfs:label        "Business (business entity type)"@en .

s:productID  a  owl:DatatypeProperty .

v1:hasEligibleQuantity
        a                 owl:ObjectProperty ;
        rdfs:comment      "This specifies the interval and unit of measurement of ordering quantities for which the gr:Offering or gr:PriceSpecification is valid. This allows e.g. specifying that a certain freight charge is valid only for a certain quantity.\nNote that if an offering is a bundle, i.e. it consists of more than one unit of a single type of good, or if the unit of measurement for the good is different from unit (Common Code C62), then gr:hasEligibleQuantity refers to units of this bundle. In other words, \"C62\" for \"Units or pieces\" is usually the appropriate unit of measurement."@en ;
        rdfs:domain       [ a            owl:Class ;
                            owl:unionOf  ( v1:Offering v1:PriceSpecification s:Offer )
                          ] ;
        rdfs:isDefinedBy  <http://purl.org/goodrelations/v1> ;
        rdfs:label        "has eligible quantity (0..1)"@en ;
        rdfs:range        v1:QuantitativeValue .

v1:hasValueInteger  a       owl:DatatypeProperty ;
        rdfs:comment        "This subproperty specifies that the upper and lower limit of the given gr:QuantitativeValueInteger are identical and have the respective integer value. It is a shortcut for such cases where a quantitative property is (at least practically) a single point value and not an interval."@en ;
        rdfs:domain         v1:QuantitativeValueInteger ;
        rdfs:isDefinedBy    <http://purl.org/goodrelations/v1> ;
        rdfs:label          "has value integer (0..1)"@en ;
        rdfs:range          xsd:int ;
        rdfs:subPropertyOf  v1:hasMaxValueInteger , v1:hasMinValueInteger .

v1:Enduser  a             v1:BusinessEntityType ;
        rdfs:comment      "The gr:BusinessEntityType representing such agents that are purchasing the good or service for private consumption, in particular not for resale or for usage within an industrial enterprise. By default, a Business Entity is an Enduser."@en ;
        rdfs:isDefinedBy  <http://purl.org/goodrelations/v1> ;
        rdfs:label        "Enduser (business entity type)"@en .

v1:validFrom  a           owl:DatatypeProperty ;
        rdfs:comment      "This property specifies the beginning of the validity of the gr:Offering, gr:PriceSpecification, gr:License, or gr:OpeningHoursSpecification.\nA time-zone should be specified. For a time in GMT/UTC, simply add a \"Z\" following the time:\n\n2008-05-30T09:30:10Z.\n\nAlternatively, you can specify an offset from the UTC time by adding a positive or negative time following the time:\n\n2008-05-30T09:30:10-09:00\n\nor\n\n2008-05-30T09:30:10+09:00.\n\nNote: If multiple contradicting instances of a gr:Offering, gr:PriceSpecification, or gr:OpeningHoursSpecification exist, it is a good heuristics to assume that\n1. Information with validity information for the respective period of time ranks higher than information without validity information.\n2. Among conflicting nodes both having validity information, the one with the shorter validity span ranks higher."@en ;
        rdfs:domain       [ a            owl:Class ;
                            owl:unionOf  ( v1:Offering v1:OpeningHoursSpecification v1:PriceSpecification v1:License s:Offer )
                          ] ;
        rdfs:isDefinedBy  <http://purl.org/goodrelations/v1> ;
        rdfs:label        "valid from (0..1)"@en ;
        rdfs:range        xsd:dateTime .

v1:ProvideService  a      v1:BusinessFunction ;
        rdfs:comment      "This gr:BusinessFunction indicates that the gr:BusinessEntity offers (or seeks) the respective type of service.\n\nNote: Maintain and Repair are also types of Services. However, products and services ontologies often provide classes for tangible products as well as for types of services. The business function gr:ProvideService is to be used with such goods that are services, while gr:Maintain and gr:Repair can be used with goods for which only the class of product exists in the ontology, but not the respective type of service.\n\nExample: Car maintenance could be expressed both as \"provide the service car maintenance\" or \"maintain cars\"."@en ;
        rdfs:isDefinedBy  <http://purl.org/goodrelations/v1> ;
        rdfs:label        "Provide service (business function)"@en .

dc:contributor  a  owl:AnnotationProperty .

v1:hasCurrencyValue  a      owl:DatatypeProperty ;
        rdfs:comment        "This property specifies the amount of money for a price per unit, shipping charges, or payment charges. The currency and other relevant details are attached to the respective gr:PriceSpecification etc.\n\nFor a gr:UnitPriceSpecification, this is the price for one unit or bundle (as specified in the unit of measurement of the unit price specification) of the respective gr:ProductOrService. For a gr:DeliveryChargeSpecification or a gr:PaymentChargeSpecification, it is the price per delivery or payment.\n\nGoodRelations also supports giving price information as intervals only. If this is needed, use gr:hasMaxCurrencyValue for the upper bound and gr:hasMinCurrencyValue for the lower bound. \n\nUsing gr:hasCurrencyValue sets the upper and lower bounds to the same given value, i.e., x gr:hasCurrencyValue y implies x gr:hasMinCurrencyValue y, x gr:hasMaxCurrencyValue y."@en ;
        rdfs:domain         v1:PriceSpecification ;
        rdfs:isDefinedBy    <http://purl.org/goodrelations/v1> ;
        rdfs:label          "has currency value (0..1)"@en ;
        rdfs:range          xsd:float ;
        rdfs:subPropertyOf  v1:hasMaxCurrencyValue , v1:hasMinCurrencyValue .

v1:predecessorOf  a       owl:TransitiveProperty , owl:ObjectProperty ;
        rdfs:comment      "This property indicates that the subject is a previous, often discontinued variant of the gr:ProductOrServiceModel used as the object.\n\nExample: Golf III predecessorOf Golf IV\n\nThis relation is transitive."@en ;
        rdfs:domain       v1:ProductOrServiceModel ;
        rdfs:isDefinedBy  <http://purl.org/goodrelations/v1> ;
        rdfs:label        "predecessor of (0..*)"@en ;
        rdfs:range        v1:ProductOrServiceModel ;
        owl:inverseOf     v1:successorOf .

v1:hasCurrency  a         owl:DatatypeProperty ;
        rdfs:comment      "The currency for all prices in the gr:PriceSpecification given using the ISO 4217 standard (3 characters)."@en ;
        rdfs:domain       v1:PriceSpecification ;
        rdfs:isDefinedBy  <http://purl.org/goodrelations/v1> ;
        rdfs:label        "has currency (1..1)"@en ;
        rdfs:range        xsd:string .

v1:availabilityStarts
        a                 owl:DatatypeProperty ;
        rdfs:comment      "This property specifies the beginning of the availability of the gr:ProductOrService included in the gr:Offering.\nThe difference to the properties gr:validFrom and gr:validThrough is that those specify the period of time during which the offer is valid and can be accepted.\n\nExample: I offer to lease my boat for the period of August 1 - August 31, 2010, but you must accept by offer no later than July 15.\n\nA time-zone should be specified. For a time in GMT/UTC, simply add a \"Z\" following the time:\n\n2008-05-30T09:30:10Z.\n\nAlternatively, you can specify an offset from the UTC time by adding a positive or negative time following the time:\n\n2008-05-30T09:30:10-09:00\n\nor\n\n2008-05-30T09:30:10+09:00.\n\nNote: There is another property gr:availableAtOrFrom, which is used to indicate the gr:Location (e.g. store or shop) from which the goods would be available."@en ;
        rdfs:domain       [ a            owl:Class ;
                            owl:unionOf  ( v1:Offering s:Offer )
                          ] ;
        rdfs:isDefinedBy  <http://purl.org/goodrelations/v1> ;
        rdfs:label        "availability starts (0..1)"@en ;
        rdfs:range        xsd:dateTime .

v1:owns  a                owl:ObjectProperty ;
        rdfs:comment      "This property indicates that a particular person or business owns a particular product. It can be used to expose the products in one's posession in order to empower recommender systems to suggest matching offers.\n\nNote that the product must be an instance of the class gr:Individual.\n\nThis property can also be safely applied to foaf:Agent instances."@en ;
        rdfs:domain       [ a            owl:Class ;
                            owl:unionOf  ( v1:BusinessEntity s:Organization s:Person )
                          ] ;
        rdfs:isDefinedBy  <http://purl.org/goodrelations/v1> ;
        rdfs:label        "owns (0..*)"@en ;
        rdfs:range        v1:Individual .

v1:BusinessEntity  a         owl:Class ;
        rdfs:comment         "An instance of this class represents the legal agent making (or seeking) a particular offering. This can be a legal body or a person. A business entity has at least a primary mailing address and contact details. For this, typical address standards (vCard) and location data (geo, WGS84) can be attached. Note that the location of the business entity is not necessarily the location from which the product or service is being available (e.g. the branch or store). Use gr:Location for stores and branches.\n\t\t\nExample: Siemens Austria AG, Volkswagen Ltd., Peter Miller's Cell phone Shop LLC\n\nCompatibility with schema.org: This class is equivalent to the union of http://schema.org/Person and http://schema.org/Organization.\t\t\n"@en ;
        rdfs:isDefinedBy     <http://purl.org/goodrelations/v1> ;
        rdfs:label           "Business entity"@en ;
        owl:disjointWith     v1:Offering , v1:PriceSpecification , v1:TypeAndQuantityNode , v1:WarrantyPromise , v1:Location , v1:WarrantyScope , v1:BusinessFunction , v1:OpeningHoursSpecification , v1:DeliveryMethod , v1:QuantitativeValue , v1:BusinessEntityType , v1:Brand , v1:PaymentMethod , v1:DayOfWeek ;
        owl:equivalentClass  [ a            owl:Class ;
                               owl:unionOf  ( s:Person s:Organization )
                             ] .

v1:equal  a               owl:SymmetricProperty , owl:TransitiveProperty , owl:ObjectProperty ;
        rdfs:comment      "This ordering relation for qualitative values indicates that the subject is equal to the object."@en ;
        rdfs:domain       v1:QualitativeValue ;
        rdfs:isDefinedBy  <http://purl.org/goodrelations/v1> ;
        rdfs:label        "equal (0..*)"@en ;
        rdfs:range        v1:QualitativeValue ;
        owl:inverseOf     v1:equal .

v1:taxID  a               owl:DatatypeProperty ;
        rdfs:comment      "The Tax / Fiscal ID of the gr:BusinessEntity, e.g. the TIN in the US or the CIF/NIF in Spain. It is usually assigned by the country of residence"@en ;
        rdfs:domain       [ a            owl:Class ;
                            owl:unionOf  ( v1:BusinessEntity s:Organization s:Person )
                          ] ;
        rdfs:isDefinedBy  <http://purl.org/goodrelations/v1> ;
        rdfs:label        "Tax ID (0..1)"@en ;
        rdfs:range        xsd:string .

v1:relatedWebService  a   owl:AnnotationProperty ;
        rdfs:comment      "The URI of a SOAP or REST Web Service from which additional information about the gr:BusinessEntity, gr:Offering, gr:PriceSpecification, or gr:ProductOrService, or any other element,  can be obtained. The recommended range is xsd:anyURI i.e., the URI of a SOAP or REST Web Service.\n\nIn principle, any existing or upcoming vocabulary for Web Services can be used in combination with GoodRelations, because the association between (a) the service description and (b) the GoodRelations description can be found via the Web Service URI value used with this gr:relatedWebService property."@en ;
        rdfs:isDefinedBy  <http://purl.org/goodrelations/v1> ;
        rdfs:label        "related Web Service (0..*)"@en .

v1:PaymentMethodCreditCard
        a                 owl:Class ;
        rdfs:comment      "The subclass of gr:PaymentMethod represents all variants and brands of credit or debit cards as a standardized procedure for transferring the monetary amount for a purchase. It is mostly used for specifying the types of payment accepted by a gr:Business Entity.\n\nExamples: VISA, MasterCard, or American Express."@en ;
        rdfs:isDefinedBy  <http://purl.org/goodrelations/v1> ;
        rdfs:label        "Payment method credit card"@en ;
        rdfs:subClassOf   v1:PaymentMethod .

v1:hasGTIN-14  a            owl:DatatypeProperty ;
        rdfs:comment        "The Global Trade Item Number (GTIN-14) of the given gr:ProductOrService or gr:Offering."@en ;
        rdfs:domain         [ a            owl:Class ;
                              owl:unionOf  ( v1:Offering v1:ProductOrService s:Product )
                            ] ;
        rdfs:isDefinedBy    <http://purl.org/goodrelations/v1> ;
        rdfs:label          "has GTIN-14 (0..*)"@en ;
        rdfs:range          xsd:string ;
        rdfs:subPropertyOf  s:productID .

v1:isVariantOf  a         owl:ObjectProperty ;
        rdfs:comment      "This states that a particular gr:ProductOrServiceModel is a variant of another product or service model. It is pretty safe to infer that the variant inherits all gr:quantitativeProductOrServiceProperty, gr:qualitativeProductOrServiceProperty, and gr:datatypeProductOrServiceProperty values that are defined for the first gr:ProductOrServiceModel.\n\nExample:\nfoo:Red_Ford_T_Model gr:isVariantOf foo:Ford_T_Model"@en ;
        rdfs:domain       v1:ProductOrServiceModel ;
        rdfs:isDefinedBy  <http://purl.org/goodrelations/v1> ;
        rdfs:label        "is variant of (0..1)"@en ;
        rdfs:range        v1:ProductOrServiceModel .

v1:validThrough  a        owl:DatatypeProperty ;
        rdfs:comment      "This property specifies the end of the validity of the gr:Offering, gr:PriceSpecification, gr:License, or gr:OpeningHoursSpecification.\nA time-zone should be specified. For a time in GMT/UTC, simply add a \"Z\" following the time:\n\n2008-05-30T09:30:10Z.\n\nAlternatively, you can specify an offset from the UTC time by adding a positive or negative time following the time:\n\n2008-05-30T09:30:10-09:00\n\nor\n2008-05-30T09:30:10+09:00.\n\nNote 1: If multiple contradicting instances of a gr:Offering, gr:PriceSpecification, or gr:OpeningHoursSpecification exist, it is a good heuristics to assume that\n1. Information with validity information for the respective period of time ranks higher than information without validity information.\n2. Among conflicting nodes both having validity information, the one with the shorter validity span ranks higher.\nNote 2: For Google, attaching a gr:validThrough statement to a gr:UnitPriceSpecification is mandatory. \n"@en ;
        rdfs:domain       [ a            owl:Class ;
                            owl:unionOf  ( v1:Offering v1:OpeningHoursSpecification v1:PriceSpecification v1:License s:Offer )
                          ] ;
        rdfs:isDefinedBy  <http://purl.org/goodrelations/v1> ;
        rdfs:label        "valid through (0..1)"@en ;
        rdfs:range        xsd:dateTime .

v1:includesObject  a      owl:ObjectProperty ;
        rdfs:comment      "This object property links a gr:Offering to one or multiple gr:TypeAndQuantityNode or nodes that specify the components that are included in the respective offer."@en ;
        rdfs:domain       [ a            owl:Class ;
                            owl:unionOf  ( v1:Offering s:Offer )
                          ] ;
        rdfs:isDefinedBy  <http://purl.org/goodrelations/v1> ;
        rdfs:label        "includes object (0..*)"@en ;
        rdfs:range        v1:TypeAndQuantityNode .

v1:category  a            owl:DatatypeProperty ;
        rdfs:comment      "The name of a category to which this gr:ProductOrService, gr:Offering, gr:BusinessEntity, or gr:Location belongs.\n\t\nNote 1: For products, it is better to add an rdf:type statement referring to a GoodRelations-compliant ontology for vertical industries instead, but if you just have a short text label, gr:category is simpler.\nNote 2: You can use greater signs or slashes to informally indicate a category hierarchy, e.g. \"restaurants/asian_restaurants\" or \"cables > usb_cables\"\n"@en ;
        rdfs:domain       [ a            owl:Class ;
                            owl:unionOf  ( v1:ProductOrService v1:Offering v1:Location v1:BusinessEntity s:Offer s:Product s:Place s:Organization )
                          ] ;
        rdfs:isDefinedBy  <http://purl.org/goodrelations/v1> ;
        rdfs:label        "category (0..*)"@en ;
        rdfs:range        rdfs:Literal .

v1:ByBankTransferInAdvance
        a                 v1:PaymentMethod ;
        rdfs:comment      "Payment by bank transfer in advance, i.e., the offering gr:BusinessEntity will inform the buying party about their bank account details and will deliver the goods upon receipt of the due amount.\nThis is equivalent to payment by wire transfer."@en ;
        rdfs:isDefinedBy  <http://purl.org/goodrelations/v1> ;
        rdfs:label        "By bank transfer in advance (payment method)"@en .

v1:QualitativeValue  a    owl:Class ;
        rdfs:comment      "A qualitative value is a predefined value for a product characteristic. \n\t\nExamples: the color \"green\" or the power cord plug type \"US\"; the garment sizes \"S\", \"M\", \"L\", and \"XL\".\n\t\nNote: Value sets are supported by creating subclasses of this class. Ordinal relations between values (gr:greater, gr:lesser, ...) are provided directly by GoodRelations.\n\nCompatibility with schema.org: This class is equivalent to http://schema.org/Enumeration."@en ;
        rdfs:isDefinedBy  <http://purl.org/goodrelations/v1> ;
        rdfs:label        "Qualitative value"@en ;
        owl:disjointWith  v1:Offering , v1:TypeAndQuantityNode , v1:QuantitativeValue .

v1:MasterCard  a          v1:PaymentMethodCreditCard ;
        rdfs:comment      "Payment by credit or debit cards issued by the MasterCard network."@en ;
        rdfs:isDefinedBy  <http://purl.org/goodrelations/v1> ;
        rdfs:label        "MasterCard (payment method)"@en .

v1:hasMinCurrencyValue
        a                 owl:DatatypeProperty ;
        rdfs:comment      "This property specifies the LOWER BOUND of the amount of money for a price RANGE per unit, shipping charges, or payment charges. The currency and other relevant details are attached to the respective gr:PriceSpecification etc.\nFor a gr:UnitPriceSpecification, this is the LOWER BOUND for the price for one unit or bundle (as specified in the unit of measurement of the unit price specification) of the respective gr:ProductOrService. For a gr:DeliveryChargeSpecification or a gr:PaymentChargeSpecification, it is the LOWER BOUND of the price per delivery or payment.\n\nUsing gr:hasCurrencyValue sets the upper and lower bounds to the same given value, i.e., x gr:hasCurrencyValue y implies x gr:hasMinCurrencyValue y, x gr:hasMaxCurrencyValue y."@en ;
        rdfs:domain       v1:PriceSpecification ;
        rdfs:isDefinedBy  <http://purl.org/goodrelations/v1> ;
        rdfs:label        "has min currency value (1..1)"@en ;
        rdfs:range        xsd:float .

v1:DeliveryChargeSpecification
        a                 owl:Class ;
        rdfs:comment      "A delivery charge specification is a conceptual entity that specifies the additional costs asked for the delivery of a given gr:Offering using a particular gr:DeliveryMethod by the respective gr:BusinessEntity. A delivery charge specification is characterized by (1) a monetary amount per order, specified as a literal value of type float in combination with a currency, (2) the delivery method, (3) the target country or region, and (4)  whether this charge includes local sales taxes, namely VAT.\nA gr:Offering may be linked to multiple gr:DeliveryChargeSpecification nodes that specify alternative charges for disjoint combinations of target countries or regions, and delivery methods.\n\nExamples: Delivery by direct download is free of charge worldwide, delivery by UPS to Germany is 10 Euros per order, delivery by mail within the US is 5 Euros per order.\n\nThe total amount of this charge is specified as a float value of the gr:hasCurrencyValue property. The currency is specified via the gr:hasCurrency datatype property. Whether the price includes VAT or not is indicated by the gr:valueAddedTaxIncluded property. The gr:DeliveryMethod to which this charge applies is specified using the gr:appliesToDeliveryMethod object property. The region or regions to which this charge applies is specified using the gr:eligibleRegions property, which uses ISO 3166-1 and ISO 3166-2 codes.\n\nIf the price can only be given as a range, use gr:hasMaxCurrencyValue and gr:hasMinCurrencyValue for the upper and lower bounds.\n\nImportant: When querying for the price, always use gr:hasMaxCurrencyValue and gr:hasMinCurrencyValue."@en ;
        rdfs:isDefinedBy  <http://purl.org/goodrelations/v1> ;
        rdfs:label        "Delivery charge specification"@en ;
        rdfs:subClassOf   v1:PriceSpecification ;
        owl:disjointWith  v1:UnitPriceSpecification , v1:PaymentChargeSpecification .

v1:hasUnitOfMeasurement
        a                 owl:DatatypeProperty ;
        rdfs:comment      "The unit of measurement for a gr:QuantitativeValue, a gr:UnitPriceSpecification, or a gr:TypeAndQuantityNode given using the UN/CEFACT Common Code (3 characters)."@en ;
        rdfs:domain       [ a            owl:Class ;
                            owl:unionOf  ( v1:QuantitativeValue v1:TypeAndQuantityNode v1:UnitPriceSpecification )
                          ] ;
        rdfs:isDefinedBy  <http://purl.org/goodrelations/v1> ;
        rdfs:label        "has unit of measurement (1..1)"@en ;
        rdfs:range        xsd:string .

dcterms:license  a  owl:AnnotationProperty .

foaf:depiction  a         owl:ObjectProperty , rdf:Property ;
        rdfs:comment      "A depiction of some thing." ;
        rdfs:domain       owl:Thing ;
        rdfs:domain       [ a            owl:Class ;
                            owl:unionOf  ( owl:Thing acco:Accommodation acco:AccommodationFeature acco:Meal acco:Allinclusive acco:BedType acco:DwellingType acco:CompoundPrice )
                          ] ;
        rdfs:isDefinedBy  foaf: ;
        rdfs:label        "depiction" ;
        rdfs:range        foaf:Image ;
        owl:inverseOf     foaf:depicts ;
        ns2:term_status   "testing" .

v1:hasValue  a              owl:DatatypeProperty ;
        rdfs:comment        "This subproperty specifies that the upper and lower limit of the given gr:QuantitativeValue are identical and have the respective value. It is a shortcut for such cases where a quantitative property is (at least practically) a single point value and not an interval."@en ;
        rdfs:domain         v1:QuantitativeValue ;
        rdfs:isDefinedBy    <http://purl.org/goodrelations/v1> ;
        rdfs:label          "has value (0..1)"@en ;
        rdfs:range          rdfs:Literal ;
        rdfs:subPropertyOf  v1:hasMinValue , v1:hasMaxValue .

<http://purl.org/goodrelations/v1>
        a                owl:Ontology ;
        rdfs:comment     "The GoodRelations ontology provides the vocabulary for annotating e-commerce offerings (1) to sell, lease, repair, dispose, or maintain commodity products and (2) to provide commodity services.\n\nGoodRelations allows describing the relationship between (1) Web resources, (2) offerings made by those Web resources, (3) legal entities, (4) prices, (5) terms and conditions, and the aforementioned ontologies for products and services (6).\n \nFor more information, see http://purl.org/goodrelations/\n\nNote: The base URI of GoodRelations is http://purl.org/goodrelations/v1. Please make sure you are only using element identifiers in this namespace, e.g. http://purl.org/goodrelations/v1#BusinessEntity. There may be copies of the ontology file on the Web which can be retrieved from other locations, BUT THOSE LOCATIONS MUST NOT BE USED AS THE BASIS OF IDENTIFIERS.\n\nIf you use GoodRelations for scientific purposes, please cite our paper:\n\nHepp, Martin: GoodRelations: An Ontology for Describing Products and Services Offers on the Web, Proceedings of the 16th International Conference on Knowledge Engineering and Knowledge Management (EKAW2008), September 29 - October 3, 2008, Acitrezza, Italy, Springer LNCS, Vol. 5268, pp. 332-347.\n\nPDF at http://www.heppnetz.de/publications/"@en ;
        rdfs:label       "GoodRelations Ontology"@en ;
        dc:contributor   "Work on the GoodRelations ontology and related research and development has been partly supported by the Austrian BMVIT/FFG under the FIT-IT Semantic Systems project myOntology (grant no. 812515/9284), by a Young Researcher's Grant (Nachwuchsfoerderung 2005-2006) from the Leopold-Franzens-Universitaet Innsbruck, by the European Commission under the project SUPER (FP6-026850), and by the German Federal Ministry of Research (BMBF) by a grant under the KMU Innovativ program as part of the Intelligent Match project (FKZ 01IS10022B). The"@en ;
        dc:creator       "Martin Hepp"@en ;
        dc:rights        "The GoodRelations ontology is available under the Creative Commons Attribution 3.0 Unported license; see http://creativecommons.org/licenses/by/3.0/. In a nutshell, you are free to copy, distribute and transmit the work; to remix/adapt the work (e.g. to import the ontology and create specializations of its elements), as long as you attribute the work in the manner specified by the author or licensor (but not in any way that suggests that they endorse you or your use of the work). Proper Attribution: Simply include the statement \"This work is based on the GoodRelations ontology, developed by Martin Hepp\" and link back to http://purl.org/goodrelations/"@en ;
        dc:subject       "E-Commerce, E-Business, GoodRelations, Microdata, Ontology, Semantic SEO, RDFa, Linked Data, RDF, Semantic Web, Recommender Systems"@en ;
        dc:title         "The GoodRelations Vocabulary for Semantic Web-based E-Commerce"@en ;
        dcterms:license  <http://creativecommons.org/licenses/by/3.0/> ;
        owl:versionInfo  "V 1.0, Release 2011-10-01"@en ;
        foaf:homepage    <http://purl.org/goodrelations/> .

v1:QuantitativeValueInteger
        a                 owl:Class ;
        rdfs:comment      "An instance of this class is an actual integer value for a quantitative property of a product. This instance is usually characterized by a minimal value, a maximal value, and a unit of measurement. \n\nExample: A seating capacity between 1 and 8 persons.\n\nNote: Users must keep in mind that ranges in here mean that ALL possible values in this interval are covered. (Sometimes, the actual commitment may be less than that: \"We sell cars from 2 - 12 seats\" does often not really mean that they have cars with 2,3,4,...12 seats.). Someone renting out two types of rowing boats, one that fits for 1 or 2 people, and another that must be operated by 4 people cannot claim to rent boats with a seating capacity between 1 and 4 people. He or she is offering two boat types for 1-2 and 4 persons.\n\t\t\nCompatibility with schema.org: This class is a subclass of http://schema.org/Quantity."@en ;
        rdfs:isDefinedBy  <http://purl.org/goodrelations/v1> ;
        rdfs:label        "Quantitative value integer"@en ;
        rdfs:subClassOf   v1:QuantitativeValue ;
        owl:disjointWith  v1:QuantitativeValueFloat .

v1:legalName  a           owl:DatatypeProperty ;
        rdfs:comment      "The legal name of the gr:BusinessEntity."@en ;
        rdfs:domain       [ a            owl:Class ;
                            owl:unionOf  ( v1:BusinessEntity s:Organization )
                          ] ;
        rdfs:isDefinedBy  <http://purl.org/goodrelations/v1> ;
        rdfs:label        "legal name (0..1)"@en ;
        rdfs:range        rdfs:Literal .

v1:availableDeliveryMethods
        a                 owl:ObjectProperty ;
        rdfs:comment      "This specifies the gr:DeliveryMethod or methods available for a given gr:Offering."@en ;
        rdfs:domain       [ a            owl:Class ;
                            owl:unionOf  ( v1:Offering s:Offer )
                          ] ;
        rdfs:isDefinedBy  <http://purl.org/goodrelations/v1> ;
        rdfs:label        "available delivery methods (0..*)"@en ;
        rdfs:range        v1:DeliveryMethod .

v1:ByInvoice  a           v1:PaymentMethod ;
        rdfs:comment      "Payment by bank transfer after delivery, i.e., the offering gr:BusinessEntity will deliver first, inform the buying party about the due amount and their bank account details, and expect payment shortly after delivery."@en ;
        rdfs:isDefinedBy  <http://purl.org/goodrelations/v1> ;
        rdfs:label        "By invoice (payment method)"@en .

v1:color  a                 owl:DatatypeProperty ;
        rdfs:comment        "The color of the product."@en ;
        rdfs:domain         [ a            owl:Class ;
                              owl:unionOf  ( v1:ProductOrService s:Product )
                            ] ;
        rdfs:isDefinedBy    <http://purl.org/goodrelations/v1> ;
        rdfs:label          "color (0..1)"@en ;
        rdfs:range          rdfs:Literal ;
        rdfs:subPropertyOf  v1:datatypeProductOrServiceProperty .

acco:DwellingType  a      owl:Class ;
        rdfs:comment      "A type of dwelling, e.g. tent, mobile home, etc. for indicating the permitted usage on a campsite. Use DBpedia URIs whenever possible."@en ;
        rdfs:isDefinedBy  acco: ;
        rdfs:label        "Dwelling Type"@en ;
        rdfs:subClassOf   v1:QualitativeValue .

acco:validFrom  a           owl:DatatypeProperty ;
        rdfs:comment        "Indicates the beginning of a time interval during which a certain feature is valid or available. For example, a sauna or swimming pool may only be available during certain periods."@en ;
        rdfs:domain         acco:AccommodationFeature ;
        rdfs:isDefinedBy    acco: ;
        rdfs:label          "valid from (0..1)"@en ;
        rdfs:range          xsd:dateTime ;
        rdfs:subPropertyOf  v1:datatypeProductOrServiceProperty .

acco:CampingPitch  a      owl:Class ;
        rdfs:comment      "A camping pitch is an individual place for overnight stay in the outdoors, typically being part of a larger acco:CampSite."@en ;
        rdfs:isDefinedBy  acco: ;
        rdfs:label        "Camping Pitch (gr:ProductOrService, gr:Location)"@en ;
        rdfs:subClassOf   acco:Accommodation .

dcterms:subject  a  owl:AnnotationProperty .

acco:BedDetails  a        owl:Class ;
        rdfs:comment      "A node holding detailed information about the available bed types, e.g. the quantity of twin beds for a hotel room. For the single case of just one bed of a certain type, you can use acco:bed directly with acco:BedType instances."@en ;
        rdfs:isDefinedBy  acco: ;
        rdfs:label        "Bed Details"@en .

acco:quantity  a          owl:DatatypeProperty ;
        rdfs:comment      "The quantity of the given bed type available in the acco:HotelRoom, acco:Suite, acco:House, or acco:Apartment."@en ;
        rdfs:domain       acco:BedDetails ;
        rdfs:isDefinedBy  acco: ;
        rdfs:label        "quantity (1..1)"@en ;
        rdfs:range        xsd:integer .

acco:includedFeature  a     owl:ObjectProperty ;
        rdfs:comment        "A feature (e.g. a characteristic or service) of the acco:Accommodation that is included in the offer for the main accommodation, i.e. at no extra costs. "@en ;
        rdfs:domain         acco:Accommodation ;
        rdfs:isDefinedBy    acco: ;
        rdfs:label          "included feature (0..*)"@en ;
        rdfs:range          acco:AccommodationFeature ;
        rdfs:subPropertyOf  acco:feature .

acco:priceComponent  a    owl:ObjectProperty ;
        rdfs:comment      "This property links to all gr:UnitPriceSpecification nodes that apply in parallel for the acco:CompoundPrice node."@en ;
        rdfs:domain       acco:CompoundPrice ;
        rdfs:isDefinedBy  acco: ;
        rdfs:label        "price component (0..*)"@en ;
        rdfs:range        v1:UnitPriceSpecification .

acco:optionalFeature  a     owl:ObjectProperty ;
        rdfs:comment        "A feature (e.g. a characteristic or service) of the acco:Accommodation that is generally available but not included in the offer for the main accommodation, i.e. at  extra costs. "@en ;
        rdfs:domain         acco:Accommodation ;
        rdfs:isDefinedBy    acco: ;
        rdfs:label          "optional feature (0..*)"@en ;
        rdfs:range          acco:AccommodationFeature ;
        rdfs:subPropertyOf  acco:feature .

acco:Meal  a              owl:Class ;
        rdfs:comment      "A meal in the sense of this vocabulary is some combination of food or beverages."@en ;
        rdfs:isDefinedBy  acco: ;
        rdfs:label        "Meal (gr:ProductOrService)"@en ;
        rdfs:subClassOf   s:Product , v1:ProductOrService .

acco:permittedUsage  a      owl:ObjectProperty ;
        rdfs:comment        "The type of objects that you are allowed to put on the camping pitch, e.g. a tent, car, boat, or mobile homre. Use DBpedia URIs whenever possible."@en ;
        rdfs:domain         [ a            owl:Class ;
                              owl:unionOf  ( acco:CampingSite acco:CampingPitch )
                            ] ;
        rdfs:isDefinedBy    acco: ;
        rdfs:label          "permitted usage (0..*)"@en ;
        rdfs:range          acco:DwellingType ;
        rdfs:subPropertyOf  v1:qualitativeProductOrServiceProperty .

dcterms:creator  a  owl:AnnotationProperty .

dcterms:title  a          owl:AnnotationProperty , owl:DatatypeProperty ;
        rdfs:isDefinedBy  dcterms: ;
        rdfs:label        "Título"@es , "Title"@en .

acco:size  a                owl:ObjectProperty ;
        rdfs:comment        "The size of the accommodation, e.g. in square meter or squarefoot.\nTypical unit code(s): MTK for square meter, FTK for square foot, or YDK for square yard "@en ;
        rdfs:domain         acco:Accommodation ;
        rdfs:isDefinedBy    acco: ;
        rdfs:label          "size (0..1)"@en ;
        rdfs:range          v1:QuantitativeValue ;
        rdfs:subPropertyOf  v1:quantitativeProductOrServiceProperty .

acco:King  a              acco:BedType ;
        rdfs:comment      "An King or Super King bed. The actual dimension may vary by country, see http://en.wikipedia.org/wiki/Bed_size."@en ;
        rdfs:isDefinedBy  acco: ;
        rdfs:label        "King or Super King bed (acco:BedType)"@en .

foaf:logo  a              owl:ObjectProperty , owl:InverseFunctionalProperty , rdf:Property ;
        rdfs:comment      "A logo representing some thing." ;
        rdfs:domain       owl:Thing ;
        rdfs:domain       [ a            owl:Class ;
                            owl:unionOf  ( owl:Thing acco:Accommodation acco:AccommodationFeature acco:Meal acco:Allinclusive acco:BedType acco:DwellingType acco:CompoundPrice )
                          ] ;
        rdfs:isDefinedBy  foaf: ;
        rdfs:label        "logo" ;
        rdfs:range        owl:Thing ;
        ns2:term_status   "testing" .

s:geo   a            owl:ObjectProperty ;
        rdfs:domain  [ a            owl:Class ;
                       owl:unionOf  ( owl:Thing acco:Accommodation )
                     ] .

dcterms:contributor  a  owl:AnnotationProperty .

acco:Accommodation  a     owl:Class ;
        rdfs:comment      "An accommodation is a place that can accommodate human beings, e.g. a hotel room, a camping pitch, or a meeting room. Many accommodations are for overnight stays, but this is not a mandatory requirement.\n\nNote: For more specific types of accommodations not defined in this ontology, you can easily use any Wikipedia entry from \n\n    http://en.wikipedia.org/wiki/List_of_human_habitation_forms\n\nand replace the base URI\n\n    http://en.wikipedia.org/wiki/\n\nby\n\n    http://www.productontology.org/id/\n\nFor instance, if you want want to describe an igloo (http://en.wikipedia.org/wiki/Igloo) for rent, you can use the local part 'Igloo' as a class identifier as follows:\n\n    http://www.productontology.org/id/Igloo"@en ;
        rdfs:isDefinedBy  acco: ;
        rdfs:label        "Accommodation (gr:ProductOrService, gr:Location)"@en ;
        rdfs:subClassOf   s:Product , v1:Location , v1:ProductOrService , s:Place .

acco:Allinclusive  a      owl:Class ;
        rdfs:comment      "All-inclusive in the sense of this vocabulary is a comprehesive set of foods and beverages, and sometimes complementing services, provided throughout the entire day."@en ;
        rdfs:isDefinedBy  acco: ;
        rdfs:label        "All-inclusive (gr:ProductOrService)"@en ;
        rdfs:subClassOf   s:Product , v1:ProductOrService .

acco:referenceQuantity
        a                 owl:ObjectProperty ;
        rdfs:comment      "The reference quantity for which a certain price applies, e.g. 1 EUR per 4 kWh of electricity. This property is a replacement for gr:hasUnitOfMeasurement for the advanced cases where the price does not relate to a standard unit."@en ;
        rdfs:domain       v1:UnitPriceSpecification ;
        rdfs:isDefinedBy  acco: ;
        rdfs:label        "reference quantity (0..*)"@en ;
        rdfs:range        v1:QuantitativeValue .

acco:value  a               owl:DatatypeProperty ;
        rdfs:comment        "The point value for the feature unless it is an interval. If possible, use numerical datatypes, e.g. xsd:decimal, xsd:int, or xsd:float. Textual content is also acceptable, though."@en ;
        rdfs:domain         acco:AccommodationFeature ;
        rdfs:isDefinedBy    acco: ;
        rdfs:label          "value (0..1)"@en ;
        rdfs:range          rdfs:Literal ;
        rdfs:subPropertyOf  v1:datatypeProductOrServiceProperty .

acco:typeOfBed  a         owl:ObjectProperty ;
        rdfs:comment      "The type of bed to which the acco:BedDetail node refers, i.e. the type of bed available in the quantity indicated by acco:quantity."@en ;
        rdfs:domain       acco:BedDetails ;
        rdfs:isDefinedBy  acco: ;
        rdfs:label        "type of bed (1..1)"@en ;
        rdfs:range        acco:BedType .

acco:Queen  a             acco:BedType ;
        rdfs:comment      "A Queen King (UK/Ire.) or Wide Double (Japan) bed. The actual dimension may vary by country, see http://en.wikipedia.org/wiki/Bed_size."@en ;
        rdfs:isDefinedBy  acco: ;
        rdfs:label        "Queen King or Wide Double bed (acco:BedType)"@en .

acco:Breakfast  a         owl:Class ;
        rdfs:comment      "A breakfast is the first meal taken after rising from a night's sleep, most often eaten in the early morning before undertaking the day's work. (Source: Wikipedia, the free encyclopedia, see http://en.wikipedia.org/wiki/Breakfast)"@en ;
        rdfs:isDefinedBy  acco: ;
        rdfs:label        "Breakfast (gr:ProductOrService)"@en ;
        rdfs:subClassOf   acco:Meal .

acco:occupancyAdults  a     owl:ObjectProperty ;
        rdfs:comment        "The allowed total occupancy of adults (in the sense of fully paying guests) for the accommodation in persons. The exact definition of what constitutes an adult varies across regions and will typically not match the legal definition of being an adult. \nTypical unit code(s): C62 for person"@en ;
        rdfs:domain         acco:Accommodation ;
        rdfs:isDefinedBy    acco: ;
        rdfs:label          "occupancy adults (0..1)"@en ;
        rdfs:range          v1:QuantitativeValue ;
        rdfs:subPropertyOf  v1:quantitativeProductOrServiceProperty .

acco:occupancy  a           owl:ObjectProperty ;
        rdfs:comment        "The allowed total occupancy for the accommodation in persons (including infants etc.\nTypical unit code(s): C62 for person"@en ;
        rdfs:domain         acco:Accommodation ;
        rdfs:isDefinedBy    acco: ;
        rdfs:label          "occupancy (0..1)"@en ;
        rdfs:range          v1:QuantitativeValue ;
        rdfs:subPropertyOf  v1:quantitativeProductOrServiceProperty .

acco:partOf  a            owl:ObjectProperty ;
        rdfs:comment      "A naive parthood relation between two acco:Accommodation instances. Examples: A certain hotel room is part of a certain hotel, a certain house is part of a holiday resort, etc. "@en ;
        rdfs:domain       acco:Accommodation ;
        rdfs:isDefinedBy  acco: ;
        rdfs:label        "partOf (0..*)"@en ;
        rdfs:range        acco:Accommodation .

acco:numberOfRooms  a       owl:ObjectProperty ;
        rdfs:comment        "The number of rooms (excluding bathrooms and closets of the acco:Suite, acco:House, or acco:Apartment. \nTypical unit code(s): C62 for person"@en ;
        rdfs:domain         [ a            owl:Class ;
                              owl:unionOf  ( acco:HotelRoom acco:Suite acco:House acco:Apartment )
                            ] ;
        rdfs:isDefinedBy    acco: ;
        rdfs:label          "number of rooms (0..1)"@en ;
        rdfs:range          v1:QuantitativeValue ;
        rdfs:subPropertyOf  v1:quantitativeProductOrServiceProperty .

acco:House  a             owl:Class ;
        rdfs:comment      "A house is a building or structure that has the ability to be occupied for habitation by humans or other creatures. (Source: Wikipedia, the free encyclopedia, see http://en.wikipedia.org/wiki/House)"@en ;
        rdfs:isDefinedBy  acco: ;
        rdfs:label        "House (gr:ProductOrService, gr:Location)"@en ;
        rdfs:subClassOf   acco:Accommodation .

acco:gated  a               owl:DatatypeProperty ;
        rdfs:comment        "Indicates whether the accommodation is gated, i.e. access is controlled via a fence and some form of gate."@en ;
        rdfs:domain         [ a            owl:Class ;
                              owl:unionOf  ( acco:Resort acco:CampingSite )
                            ] ;
        rdfs:isDefinedBy    acco: ;
        rdfs:label          "gated (0..1)"@en ;
        rdfs:range          xsd:boolean ;
        rdfs:subPropertyOf  v1:datatypeProductOrServiceProperty .

acco:Apartment  a         owl:Class ;
        rdfs:comment      "An apartment (in American English) or flat (in British English) is a self-contained housing unit (a type of residential real estate) that occupies only part of a building. (Source: Wikipedia, the free encyclopedia, see http://en.wikipedia.org/wiki/Apartment)"@en ;
        rdfs:isDefinedBy  acco: ;
        rdfs:label        "Apartment (gr:ProductOrService, gr:Location)"@en ;
        rdfs:subClassOf   acco:Accommodation .

acco:CampingSite  a       owl:Class ;
        rdfs:comment      "A camping site, campsite, or campground is a place used for overnight stay in the outdoors. In British English a campsite is an area, usually divided into a number of pitches, where people can camp overnight using tents or camper vans or caravans; this British English use of the word is synonymous with the American English expression campground. In American English the term campsite generally means an area where an individual, family, group, or military unit can pitch a tent or parks a camper; a campground may contain many campsites. (Source: Wikipedia, the free encyclopedia, see http://en.wikipedia.org/wiki/Campsite)"@en ;
        rdfs:isDefinedBy  acco: ;
        rdfs:label        "Camping Site (gr:ProductOrService, gr:Location)"@en ;
        rdfs:subClassOf   acco:Accommodation .

<http://ontologies.sti-innsbruck.at/acco/ns.owl>
        a                  foaf:Document ;
        foaf:primaryTopic  acco: .

acco:unitCode  a            owl:DatatypeProperty ;
        rdfs:comment        "The UN/CEFACT Common Code for the unit of measurement, e.g. \"MTR\" for meter, \"HUR\" for hours, etc. If you only have a textual representation of the unit of measurement, use acco:unit instead."@en ;
        rdfs:domain         acco:AccommodationFeature ;
        rdfs:isDefinedBy    acco: ;
        rdfs:label          "unit code (0..1)"@en ;
        rdfs:range          xsd:string ;
        rdfs:subPropertyOf  v1:datatypeProductOrServiceProperty .

acco:Dinner  a            owl:Class ;
        rdfs:comment      "A dinner is the main meal of the day, often consumed in the evening of the day."@en ;
        rdfs:isDefinedBy  acco: ;
        rdfs:label        "Dinner (gr:ProductOrService)"@en ;
        rdfs:subClassOf   acco:Meal .

acco:Hotel  a             owl:Class ;
        rdfs:comment      "A hotel is an establishment that provides lodging paid on a short-term basis. (Source: Wikipedia, the free encyclopedia, see http://en.wikipedia.org/wiki/Hotel)"@en ;
        rdfs:isDefinedBy  acco: ;
        rdfs:label        "Hotel (gr:ProductOrService, gr:Location)"@en ;
        rdfs:subClassOf   acco:Accommodation .

dcterms:rights  a  owl:AnnotationProperty .

foaf:primaryTopic  a      owl:AnnotationProperty , owl:FunctionalProperty , rdf:Property , owl:ObjectProperty ;
        rdfs:comment      "The primary topic of some page or document." ;
        rdfs:domain       foaf:Document ;
        rdfs:isDefinedBy  foaf: ;
        rdfs:label        "primary topic" ;
        rdfs:range        owl:Thing ;
        owl:inverseOf     foaf:isPrimaryTopicOf ;
        ns2:term_status   "stable" .

acco:validThrough  a        owl:DatatypeProperty ;
        rdfs:comment        "Indicates the beginning of a time interval during which a certain feature is valid or available. For example, a sauna or swimming pool may only be available during certain periods."@en ;
        rdfs:domain         acco:AccommodationFeature ;
        rdfs:isDefinedBy    acco: ;
        rdfs:label          "valid from (0..1)"@en ;
        rdfs:range          xsd:dateTime ;
        rdfs:subPropertyOf  v1:datatypeProductOrServiceProperty .

<http://ontologies.sti-innsbruck.at/acco/ns>
        a                  foaf:Document ;
        foaf:primaryTopic  acco: .

acco:BedType  a           owl:Class ;
        rdfs:comment      "A type of bed. This is used for indicating the bed or beds available in an accommodation. Use DBpedia URIs whenever possible."@en ;
        rdfs:isDefinedBy  acco: ;
        rdfs:label        "Bed Type"@en ;
        rdfs:subClassOf   v1:QualitativeValue .

acco:OlympicQueen  a      acco:BedType ;
        rdfs:comment      "An Olympic Queen bed. The actual dimension may vary by country, see http://en.wikipedia.org/wiki/Bed_size."@en ;
        rdfs:isDefinedBy  acco: ;
        rdfs:label        "Olympic Queen bed (acco:BedType)"@en .

acco:max  a                 owl:DatatypeProperty ;
        rdfs:comment        "The upper bound of the value for the feature. It is best to use this property with numerical datatypes, e.g. xsd:decimal, xsd:int, or xsd:float."@en ;
        rdfs:domain         acco:AccommodationFeature ;
        rdfs:isDefinedBy    acco: ;
        rdfs:label          "max (0..1)"@en ;
        rdfs:range          rdfs:Literal ;
        rdfs:subPropertyOf  v1:datatypeProductOrServiceProperty .

acco:MeetingRoom  a       owl:Class ;
        rdfs:comment      "A meeting room, conference room, or conference hall is a room provided for singular events such as business conferences and meetings. (Source: Wikipedia, the free encyclopedia, see http://en.wikipedia.org/wiki/Conference_hall)  "@en ;
        rdfs:isDefinedBy  acco: ;
        rdfs:label        "Meeting Room (gr:ProductOrService, gr:Location)"@en ;
        rdfs:subClassOf   acco:Accommodation .

acco:CompoundPrice  a     owl:Class ;
        rdfs:comment      "A compound price specification is one that bundles multiple prices that all apply in combination for different dimensions of consumption. Use gr:name for indicating the dimension (e.g. \"electricity\" or \"final cleaning\")."@en ;
        rdfs:isDefinedBy  acco: ;
        rdfs:label        "Compound Price"@en ;
        rdfs:subClassOf   v1:PriceSpecification .

acco:CaliforniaKing  a    acco:BedType ;
        rdfs:comment      "A California King or King Long bed. The actual dimension may vary by country, see http://en.wikipedia.org/wiki/Bed_size."@en ;
        rdfs:isDefinedBy  acco: ;
        rdfs:label        "California King or King Long bed (acco:BedType)"@en .

<http://purl.org/acco/ns>
        a                  foaf:Document ;
        foaf:primaryTopic  acco: .

acco:   a                    owl:Ontology ;
        rdfs:comment         "ACCO: The Accommodation Ontology\n    \nA Web vocabulary for hotels, vacation homes, camping sites, and other accommodation offers for e-commerce.\n\nVocabulary:    http://purl.org/acco/ns#\nNamespace:     http://purl.org/acco/ns#\n\nThe Accommodation Ontology is designed to be used in combination with GoodRelations, a standard vocabulary for the commercial aspects of offers for sale or rental. \n\nSee http://purl.org/goodrelations/ for more information."@en ;
        rdfs:label           "Accommodation Ontology"@en ;
        dcterms:contributor  "Michael Fried, Birgit Leiter, and Dieter Fensel. Some class and property definitions are inspired by or based on abstracts from Wikipedia, the free encyclopedia."@en ;
        dcterms:creator      "Martin Hepp (Hepp Research GmbH)"@en ;
        dcterms:license      <http://creativecommons.org/licenses/by/3.0/> ;
        dcterms:rights       "The Accommodation Ontology ontology is available under the Creative Commons Attribution 3.0 Unported license; see http://creativecommons.org/licenses/by/3.0/. \nIn a nutshell, you are free to copy, distribute and transmit the work; to remix/adapt the work (e.g. to import the ontology and create specializations of its elements), \nas long as you attribute the work in the manner specified by the author or licensor (but not in any way that suggests that they endorse you or your use of the work)."@en ;
        dcterms:subject      "E-Commerce, E-Business, GoodRelations, Ontology, Tourism, Hotels, Camping, Vacation homes"@en ;
        dcterms:title        "ACCO: The Accommodation Ontology for Semantic Web-based E-Commerce"@en ;
        owl:imports          <http://purl.org/goodrelations/v1> ;
        owl:versionInfo      "V 1.0, Release 2013-03-25" .

acco:HotelRoom  a         owl:Class ;
        rdfs:comment      "A hotel room is a single room in a hotel."@en ;
        rdfs:isDefinedBy  acco: ;
        rdfs:label        "Hotel Room (gr:ProductOrService, gr:Location)"@en ;
        rdfs:subClassOf   acco:Accommodation .

acco:occupancyMinors  a     owl:ObjectProperty ;
        rdfs:comment        "The allowed total occupancy of minors (in the sense of not fully paying guests) for the accommodation in persons. The exact definition of what constitutes a minor varies across regions and will typically not match the legal definition of being a minor. \nTypical unit code(s): C62 for person"@en ;
        rdfs:domain         acco:Accommodation ;
        rdfs:isDefinedBy    acco: ;
        rdfs:label          "occupancy minors (0..1)"@en ;
        rdfs:range          v1:QuantitativeValue ;
        rdfs:subPropertyOf  v1:quantitativeProductOrServiceProperty .

acco:propertyID  a          owl:DatatypeProperty ;
        rdfs:comment        "A global identifier, e.g. a URI, a prefixed string, or any other identifier that can be used to refer to a standardized property type.\n\nThe following prefixes and values are reserved:\nstarRating:HOTREC \nstarRating:DEHOGA\nstarRating:WHR\nstarRating:Hotelstars\n"@en ;
        rdfs:domain         acco:AccommodationFeature ;
        rdfs:isDefinedBy    acco: ;
        rdfs:label          "property ID (0..1)"@en ;
        rdfs:range          rdfs:Literal ;
        rdfs:subPropertyOf  v1:datatypeProductOrServiceProperty .

acco:Resort  a            owl:Class ;
        rdfs:comment      "A resort is a place used for relaxation or recreation, attracting visitors for holidays or vacations. Resorts are places, towns or sometimes commercial establishment operated by a single company. (Source: Wikipedia, the free encyclopedia, see http://en.wikipedia.org/wiki/Resort)"@en ;
        rdfs:isDefinedBy  acco: ;
        rdfs:label        "Resort (gr:ProductOrService, gr:Location)"@en ;
        rdfs:subClassOf   acco:Accommodation .

acco:Lunch  a             owl:Class ;
        rdfs:comment      "A luncheon, commonly abbreviated to lunch, is a middle of the day meal. (Source: Wikipedia, the free encyclopedia, see http://en.wikipedia.org/wiki/Lunch)"@en ;
        rdfs:isDefinedBy  acco: ;
        rdfs:label        "Lunch (gr:ProductOrService)"@en ;
        rdfs:subClassOf   acco:Meal .

acco:bed  a                 owl:ObjectProperty ;
        rdfs:comment        "The type of bed or beds included in the accommodation. For the single case of just one bed of a certain type, you use acco:bed directly with acco:BedType instances. If you want to indicate the quantity of a certain acco:BedType, use an instance of acco:BedDetails. For more detailed information, use acco:feature."@en ;
        rdfs:domain         [ a            owl:Class ;
                              owl:unionOf  ( acco:HotelRoom acco:Suite acco:House acco:Apartment )
                            ] ;
        rdfs:isDefinedBy    acco: ;
        rdfs:label          "bed (0..*)"@en ;
        rdfs:range          [ a            owl:Class ;
                              owl:unionOf  ( acco:BedType acco:BedDetails )
                            ] ;
        rdfs:subPropertyOf  v1:qualitativeProductOrServiceProperty .

acco:feature  a           owl:ObjectProperty ;
        rdfs:comment      "A feature (e.g. a characteristic or service) of the acco:Accommodation. This generic property does not make a statement about whether the feature is included in the offer for the main accommodation or available at extra costs. "@en ;
        rdfs:domain       acco:Accommodation ;
        rdfs:isDefinedBy  acco: ;
        rdfs:label        "feature (0..*)"@en ;
        rdfs:range        acco:AccommodationFeature .

<http://purl.org/acco/ns.owl>
        a                  foaf:Document ;
        foaf:primaryTopic  acco: .

acco:petsAllowed  a         owl:DatatypeProperty ;
        rdfs:comment        "Indicates whether pets are allowed to enter the accommodation."@en ;
        rdfs:domain         acco:Accommodation ;
        rdfs:isDefinedBy    acco: ;
        rdfs:label          "pets allowed (0..1)"@en ;
        rdfs:range          xsd:boolean ;
        rdfs:subPropertyOf  v1:datatypeProductOrServiceProperty .

<http://ontologies.sti-innsbruck.at/acco/ns.html>
        a                  foaf:Document ;
        foaf:primaryTopic  acco: .

acco:min  a                 owl:DatatypeProperty ;
        rdfs:comment        "The lower bound of the value for the feature. It is best to use this property with numerical datatypes, e.g. xsd:decimal, xsd:int, or xsd:float."@en ;
        rdfs:domain         acco:AccommodationFeature ;
        rdfs:isDefinedBy    acco: ;
        rdfs:label          "min (0..1)"@en ;
        rdfs:range          rdfs:Literal ;
        rdfs:subPropertyOf  v1:datatypeProductOrServiceProperty .

foaf:Document  a          owl:Class , rdfs:Class ;
        rdfs:comment      "A document." ;
        rdfs:isDefinedBy  foaf: ;
        rdfs:label        "Documento"@es , "Document"@en , "Document" ;
        owl:disjointWith  foaf:Project , foaf:Organization ;
        ns2:term_status   "testing" .

acco:AccommodationFeature
        a                 owl:Class ;
        rdfs:comment      "An accommodation feature is a structured value representing the feature of an accommodation as a property-value pair of varying degrees of formality."@en ;
        rdfs:isDefinedBy  acco: ;
        rdfs:label        "Accommodation Feature"@en .

acco:unit  a                owl:DatatypeProperty ;
        rdfs:comment        "A textual representation of the unit of measurement, e.g. global identifier, e.g. \"m\" or \"meter\". When you have the UN/CEFACT Common Code for the unit available, it is better to use acco:unitCode. This property is for the cases where a standardized unit code is not available from the data source."@en ;
        rdfs:domain         [ a            owl:Class ;
                              owl:unionOf  ( acco:AccommodationFeature v1:UnitPriceSpecification )
                            ] ;
        rdfs:isDefinedBy    acco: ;
        rdfs:label          "unit (0..1)"@en ;
        rdfs:range          rdfs:Literal ;
        rdfs:subPropertyOf  v1:datatypeProductOrServiceProperty .

acco:Suite  a             owl:Class ;
        rdfs:comment      "A suite in a hotel or other public accommodation, denotes a class of luxury accommodations, the key feature of which is multiple rooms. (Source: Wikipedia, the free encyclopedia, see http://en.wikipedia.org/wiki/Suite_(hotel)) "@en ;
        rdfs:isDefinedBy  acco: ;
        rdfs:label        "Suite (gr:ProductOrService, gr:Location)"@en ;
        rdfs:subClassOf   acco:Accommodation .

acco:availabilityTimes
        a                 owl:ObjectProperty ;
        rdfs:comment      "Indicates the times of availability of a particular accommodation feature. Example: The sauna is available from 8:00 - 10:00 a.m. on weekdays."@en ;
        rdfs:domain       acco:AccommodationFeature ;
        rdfs:isDefinedBy  acco: ;
        rdfs:label        "availability times (0..1)"@en ;
        rdfs:range        v1:OpeningHoursSpecification .

pproc:remedyResolutionDate
        a                   owl:FunctionalProperty , owl:DatatypeProperty ;
        rdfs:domain         pproc:Remedy ;
        rdfs:label          "Fecha de resolución del recurso"@es , "Remedy resolution date"@en ;
        rdfs:range          xsd:date ;
        rdfs:subPropertyOf  dcterms:date .

pproc:contractOrProcedureExtinction
        a             owl:ObjectProperty ;
        rdfs:comment  "Propiedad abstracta que indica la extinción de un contrato por resolución, renuncia o abandono. O bien la extinción del procedimiento al ser declarado desierto.\n\nUtilizar una de sus subclases."@es , "Abstract property pointing to extinction of contract or procedure. Use any of its subclasses."@en ;
        rdfs:domain   pproc:Contract ;
        rdfs:label    "Extinción de contrato o de procedimiento"@es , "Contract or procedure extinction"@en ;
        rdfs:range    pproc:ContractOrProcedureExtinction .

pproc:ContractOrProcedureExtinction
        a             owl:Class ;
        rdfs:comment  "Clase abstracta. Existe una serie de circunstancias que derivan en la extinctión del contrato o procedimiento. Para describir estas situaciones se hace uso de una de sus subclases."@es , "Abstract class. There are some circumstances resulting in the extinction of the procedure of the contract or the contract itself. To describe that situations we may use one of its subclasses."@en ;
        rdfs:label    "Extinción del contrato o del procedimiento"@es , "Contract or procedure extinction"@en .

<http://es.linkedin.com/pub/guillermo-esteban-p%C3%A9rez/56/210/5a8>
        a       foaf:Person , owl:NamedIndividual .

pproc:contractModification
        a             owl:ObjectProperty ;
        rdfs:comment  "Indica la modificación efectuada en un contrato."@es , "Points to contract modifications being made."@en ;
        rdfs:domain   pproc:Contract ;
        rdfs:label    "Modificación de contrato"@es , "Contract modification"@en ;
        rdfs:range    pproc:ContractModification .

pproc:MixedCapitalCompanyContract
        a                owl:Class ;
        rdfs:comment     "Los contrato de sociedad de economia mixta son aquellos en que la Administración participe, por sí o por medio de una entidad pública, en concurrencia con personas naturales o jurídicas."@es , "Class describing the contracts where the contracting authority participates concurrently with the natural or legal person."@en ;
        rdfs:label       "Contrato de sociedad de economia mixta"@es , "Mixed capital company contract"@en ;
        rdfs:subClassOf  pproc:PublicServicesManagementContract .

pproc:duration  a   owl:DatatypeProperty ;
        rdfs:label  "Duración"@es , "Duration"@en ;
        rdfs:range  xsd:duration .

pproc:ContractExecutionConditions
        a             owl:Class ;
        rdfs:comment  "Clase que define las condiciones de ejecución de un contrato (e.g. condiciones especiales ó subcontratación)."@es , "Class that defines the execution conditions of the contract (e.g. special execution conditions or subcontracting percentage amounts)."@en ;
        rdfs:label    "Condiciones de ejecución del contrato"@es , "Contract execution conditions"@en .

pproc:UrgencyTypeScheme
        a             skos:ConceptScheme , owl:NamedIndividual ;
        rdfs:comment  "Scheme that defines the kinds of urgency a procedure can follow."@en ;
        rdfs:label    "Esquema de tipos de urgencia"@es , "Urgency type scheme"@en .

<http://contsem.unizar.es/def/sector-publico/contsem>
        a              owl:NamedIndividual ;
        dcterms:title  "ontologia CONTSEM"@es , "CONTSEM ontology"@en .

pproc:tenderInformationProvider
        a            owl:ObjectProperty ;
        rdfs:domain  pproc:ContractProcedureSpecifications ;
        rdfs:label   "Proveedor de información sobre la licitación"@es , "Tender information provider"@en ;
        rdfs:range   pproc:InformationProvider .

s:addressCountry  a       owl:DatatypeProperty ;
        rdfs:isDefinedBy  s: ;
        rdfs:label        "País"@es , "Address country"@en .

pc:Contract  a            owl:Class ;
        rdfs:isDefinedBy  pc: ;
        rdfs:label        "Contrato"@es , "Contract"@en .

pproc:lot  a                owl:ObjectProperty ;
        rdfs:domain         pproc:ContractWithLots ;
        rdfs:label          "Lot"@en , "Lote" ;
        rdfs:range          pproc:Lot ;
        rdfs:subPropertyOf  pc:lot .

pproc:awardDate  a                  owl:FunctionalProperty , owl:DatatypeProperty ;
        rdfs:domain                 pc:Tender ;
        rdfs:label                  "Fecha de adjudicación"@es , "Date of award"@en ;
        rdfs:range                  xsd:date ;
        rdfs:subPropertyOf          dcterms:date ;
        owl:backwardCompatibleWith  pc:awardDate .

dcterms:description  a    owl:DatatypeProperty ;
        rdfs:isDefinedBy  dcterms: ;
        rdfs:label        "Descripción"@es , "Description"@en .

pproc:ExtendableContract
        a                owl:Class ;
        rdfs:comment     "Contratos públicos cuya fecha de ejecución puede ser pospuesta o extendida."@es , "Class describing contracts whose end date can be extended."@en ;
        rdfs:label       "Contrato prorrogable"@es , "Extendable contract"@en ;
        rdfs:subClassOf  pproc:Contract .

pproc:maxFinalPriceChange
        a             owl:FunctionalProperty , owl:DatatypeProperty ;
        rdfs:comment  "El rango en esta propiedad indica un porcentaje, por lo que el rango del número real a utilizar debe estar comprendido entre 0.0 y 100.0."@es , "The range of this property must be a percentage (i.e. float between 0.0 and 100.0)"@en ;
        rdfs:domain   pproc:ContractModificationConditions ;
        rdfs:label    "Modificación máxima sobre precio final"@es , "Maximum final price change"@en ;
        rdfs:range    xsd:float .

pproc:AdditionalInformationNotice
        a                owl:Class ;
        rdfs:label       "Anuncio de información adicional"@es , "Additional information notice"@en ;
        rdfs:subClassOf  pproc:Notice .

pproc:mainObject  a                 owl:FunctionalProperty , owl:ObjectProperty ;
        rdfs:comment                "Representación CPV del objeto de un contrato.\n\nDebe apuntar a un concepto de objeto siguiendo la clasificación CPV de algún esquema de conceptos SKOS, como http://cpv.data.ac.uk/."@es , "Property that points to the concept of the CPV code of an object.\n\nThe concept used should be a valid representation of a CPV code, as it is in http://cpv.data.ac.uk/."@en ;
        rdfs:domain                 pproc:ContractObject ;
        rdfs:label                  "Principal objeto del contrato"@es , "Main object of contract"@en ;
        rdfs:range                  skos:Concept ;
        owl:backwardCompatibleWith  pc:mainObject .

pproc:contractingBody
        a            owl:FunctionalProperty , owl:ObjectProperty ;
        rdfs:domain  pproc:Contract ;
        rdfs:label   "Órgano de contratación"@es , "Contracting body"@en ;
        rdfs:range   org:Organization .

pc:offeredPrice  a          owl:ObjectProperty ;
        rdfs:isDefinedBy    pc: ;
        rdfs:label          "Precio ofrecido"@es , "Offered price"@en ;
        rdfs:subPropertyOf  v1:hasPriceSpecification .

pproc:noticeDate  a         owl:FunctionalProperty , owl:DatatypeProperty ;
        rdfs:domain         pproc:Notice ;
        rdfs:label          "Fecha de publicación del anuncio"@es , "Date of notice publication"@en ;
        rdfs:range          xsd:date ;
        rdfs:subPropertyOf  dcterms:date .

pproc:SubjectiveAwardCriterion
        a                owl:Class ;
        rdfs:comment     "Clase para especificar los criterios que dependen de una opinion subjetiva."@es , "Class used to describe criteria that depend on a subjetive opinion."@en ;
        rdfs:label       "Criterio de adjudicación subjetivo"@es , "Subjective award criterion"@en ;
        rdfs:subClassOf  pc:AwardCriterion .

pproc:remedyInterposedTo
        a            owl:DatatypeProperty ;
        rdfs:domain  pproc:Remedy ;
        rdfs:label   "Recurso interpuesto a"@es , "Remedy interposed to"@en ;
        rdfs:range   xsd:string .

pproc:additionalObject
        a                           owl:ObjectProperty ;
        rdfs:comment                "Representación CPV del objeto de un contrato.\n\nDebe apuntar a un concepto de objeto siguiendo la clasificación CPV de algún esquema de conceptos SKOS, como http://cpv.data.ac.uk/."@es , "Property that points to the concept of the CPV code of an object.\n\nThe concept used should be a valid representation of a CPV code, as it is in http://cpv.data.ac.uk/."@en ;
        rdfs:domain                 pproc:ContractObject ;
        rdfs:label                  "Objeto adicional del contrato"@es , "Additional object of contract"@en ;
        rdfs:range                  skos:Concept ;
        owl:backwardCompatibleWith  pc:additionalObject .

pproc:priceReviewAllowable
        a            owl:FunctionalProperty , owl:DatatypeProperty ;
        rdfs:domain  pproc:ContractEconomicConditions ;
        rdfs:label   "Revisión de precios permitida"@es , "Price review allowable"@en ;
        rdfs:range   xsd:boolean .

pproc:earlyTramitation
        a            owl:FunctionalProperty , owl:DatatypeProperty ;
        rdfs:domain  pproc:ContractProcedureSpecifications ;
        rdfs:label   "Tramitación anticipada"@es , "Early tramitation"@en ;
        rdfs:range   xsd:boolean .

s:postalAddress  a        owl:DatatypeProperty ;
        rdfs:isDefinedBy  s: ;
        rdfs:label        "Dirección postal"@es , "Postal address"@en .

skos:broader  a           owl:ObjectProperty ;
        rdfs:isDefinedBy  skos: ;
        rdfs:label        "Más amplio"@es , "Broader"@en .

foaf:member  a            owl:ObjectProperty , rdf:Property ;
        rdfs:comment      "Indicates a member of a Group" ;
        rdfs:domain       foaf:Group ;
        rdfs:isDefinedBy  foaf: ;
        rdfs:label        "Miembro"@es , "Member"@en , "member" ;
        rdfs:range        foaf:Agent ;
        ns2:term_status   "stable" .

pproc:ContractWithLots
        a                owl:Class ;
        rdfs:comment     "Clase de los contratos dividos en lotes.\n\nCuando un contrato de muy grande, este puede ser dividido en diversos lotes por la entidad contratante. Las empresas presentan las ofertas a estos lotes separadamente (y no al contrato \"raíz\"), realizándose la adjudicación de la misma manera."@es , "Class of the contract that have lots."@en ;
        rdfs:label       "Contrato con lotes"@es , "Contract with lots"@en ;
        rdfs:subClassOf  pproc:Contract ;
        rdfs:subClassOf  [ a                   owl:Restriction ;
                           owl:onProperty      pproc:lot ;
                           owl:someValuesFrom  pproc:Lot
                         ] .

skos:ConceptScheme  a     owl:Class ;
        rdfs:isDefinedBy  skos: ;
        rdfs:label        "Esquema de conceptos"@es , "Concept scheme"@en .

pproc:ProcedureTypeScheme
        a             skos:ConceptScheme , owl:NamedIndividual ;
        rdfs:comment  "Scheme defining the procedure to be followed in a tender."@en ;
        rdfs:label    "Esquema de tipos de procedimiento"@es , "Procedure type scheme"@en .

pproc:executionRequeriments
        a             owl:DatatypeProperty ;
        rdfs:comment  "Campo para definir las condiciones de ejecución del contrato si las hubiera (e.g. forma jurídica a adoptar por la agrupación de contratistas)"@es , "Property to define alternative execution requirements (e.g. legal form to be adopted by tenderers)."@en ;
        rdfs:domain   pproc:ContractExecutionConditions ;
        rdfs:label    "Condiciones de ejecución"@es , "Execution requeriments"@en ;
        rdfs:range    xsd:string .

pproc:  a                owl:Ontology ;
        rdfs:comment     "Ontología creada con objeto de publicar datos sobre contratación publica española en RDF. Se ha desarrollado durante el transcurso del proyecto \"Optimización de la contratación pública mediante la utilización de técnicas semánticas\" (CONTSEM), en el que participan la empresa iASoft (OESIA), la Universidad de Zaragoza y, como administraciones usuarias, el Gobierno de Aragón, la Diputación Provincial de Huesca y los ayuntamientos de Zaragoza y Huesca.\n\nFinanciado por la Acción Estratégica de Telecomunicaciones y Sociedad de la Información. Año 2012. Ministerio de Industria, Comercio y Turismo (TSI-020606-2012-4), y desarrollado entre noviembre de 2012 y diciembre de 2014."@es ;
        rdfs:label       "ontología de contratación pública"@es , "public procurement ontology"@en ;
        rdfs:seeAlso     <http://figshare.com/articles/Ontology_Requirements_Specification_Document_ORSD_/1314591> ;
        dcterms:creator  <http://www.araid.es/en/users/jfm#profile-investigador> , <https://www.linkedin.com/profile/view?id=218098827> , <http://es.linkedin.com/pub/guillermo-esteban-p%C3%A9rez/56/210/5a8> , <http://webdiis.unizar.es/~seron/> ;
        owl:versionInfo  "Cambios de la versión 0.1.4 a la versión 1.0.0:\n\n- Cambios menores en la documentación RDF\n- Añadido nuevo axioma (pproc:ContractWithoutLots rdfs:subClassOf pproc:numberOfLots value 0)\n- Cambios en la documentación web\n- Arreglado un error donde pproc:criterion tenía a pc:AwardCriteriaCombination como (en vez de pc:AwardCriterion)\n- Añadida pproc:additionalObject para enlazar con múltiples CPVs\n- Añadida pproc:endMode para pproc:ElectronicAuctionPhase"@es , "Changes from 0.1.4 to 1.0.0:\n\n- Minor RDF documentation changes\n- Added new axiom (pproc:ContractWithoutLots rdfs:subClassOf pproc:numberOfLots value 0)\n- Web documentation changes\n- Fixed an error where pproc:criterion had pc:AwardCriteriaCombination as range (instead pc:AwardCriterion)\n- Added missing pproc:additionalObject to link multiple CPVs\n- Added missing pproc:endMode from pproc:ElectronicAuctionPhase"@en , "1.0.0" .

pproc:remedyResult  a  owl:DatatypeProperty ;
        rdfs:comment  "Contiene el resultado del recurso interpuesto en un contrato. Normalmente el valor de esta propiedad incluirá valores como \"Estimado\", \"Estimado parcialmente\" o \"Desestimado\"."@es , "Contains the result of a lodged remedy. Normally it would contains values like \"Estimated\", \"Rejected\" or \"Partially estimated\"."@en ;
        rdfs:domain   pproc:Remedy ;
        rdfs:label    "Resultado del recurso"@es , "Remedy result"@en ;
        rdfs:range    xsd:string .

pproc:ContractNotice  a  owl:Class ;
        rdfs:label       "Anuncio de licitación"@es , "Contract notice"@en ;
        rdfs:subClassOf  pproc:Notice .

pproc:legalDocumentReference
        a                   owl:ObjectProperty ;
        rdfs:domain         pproc:Contract ;
        rdfs:label          "Pliego de cláusulas administrativas"@es , "Legal document reference"@en ;
        rdfs:subPropertyOf  pproc:documentReference .

pproc:InformationKindScheme
        a             skos:ConceptScheme , owl:NamedIndividual ;
        rdfs:comment  "Scheme that indicates the type of the information that can be provided."@en ;
        rdfs:label    "Esquema de tipos de información"@es , "Information kind scheme"@en .

pproc:FrameworkAgreement
        a             owl:Class ;
        rdfs:comment  "Clase a utilizar cuando estemos ante un contrato que consiste en la declaración, tanto de un acuerdo marco como de un sistema dinámico de contratación."@es , "Class used to describe a contract that is a declaration of a framework agreement or a dynamic purchasing system."@en ;
        rdfs:label    "Acuerdo marco o Sistema Dinámico de contratación"@es , "Framework agreement or dynamic purchasing system"@en .

pproc:otherGuarantee  a  owl:DatatypeProperty ;
        rdfs:domain  pproc:ContractAdditionalObligations ;
        rdfs:label   "Otras garantías"@es , "Other guarantee"@en ;
        rdfs:range   xsd:string .

pproc:electronicAuctionWeb
        a             owl:ObjectProperty ;
        rdfs:comment  "Apunta a la web donde puede se realiza la subasta electrónica, o en su defecto, donde se pueda encontrar más información acerca de la subasta electrónica."@es , "Property that indicated where the electronic auction is made or where we can look for more information about the auction."@en ;
        rdfs:domain   pproc:ElectronicAuction ;
        rdfs:label    "Web de la subasta electrónica"@es , "Electronic auction web"@en ;
        rdfs:range    foaf:Document .

pproc:tenderBriefing  a  owl:ObjectProperty ;
        rdfs:domain  pproc:Contract ;
        rdfs:label   "Reunión informativa"@es , "Tender briefing"@en ;
        rdfs:range   pproc:Briefing .

pproc:NegotiatedWithoutPublicity
        a              skos:Concept , owl:NamedIndividual ;
        rdfs:label     "Negociado sin publicidad"@es , "Negotiated without publicity"@en ;
        skos:broader   pproc:Negotiated ;
        skos:inScheme  pproc:ProcedureTypeScheme .

s:address  a              owl:DatatypeProperty ;
        rdfs:isDefinedBy  s: ;
        rdfs:label        "Dirección"@es , "Address"@en .

pproc:tenderCommitteeAppointmentDate
        a                   owl:FunctionalProperty , owl:DatatypeProperty ;
        rdfs:domain         pproc:Committee ;
        rdfs:label          "Fecha de nombramiento"@es , "Tender committee appointment date"@en ;
        rdfs:range          xsd:date ;
        rdfs:subPropertyOf  dcterms:date .

xsd:date  a     rdfs:Datatype .

pproc:ContractAwardNotice
        a                owl:Class ;
        rdfs:label       "Anuncio de adjudicación"@es , "Contract award notice"@en ;
        rdfs:subClassOf  pproc:Notice .

pproc:procedureType  a  owl:FunctionalProperty , owl:ObjectProperty ;
        rdfs:domain   pproc:ContractProcedureSpecifications ;
        rdfs:label    "Tipo de procedimiento"@es , "Procedure type"@en ;
        rdfs:range    skos:Concept ;
        rdfs:range    [ a               owl:Restriction ;
                        owl:hasValue    pproc:ProcedureTypeScheme ;
                        owl:onProperty  skos:inScheme
                      ] ;
        rdfs:seeAlso  pproc:ProcedureTypeScheme .

pproc:fullMember  a         owl:ObjectProperty ;
        rdfs:comment        "Miembro titular en una mesa de contratación."@es , "Points to a full member of a committee."@en ;
        rdfs:domain         pproc:Committee ;
        rdfs:label          "Miembro titular"@es , "Full member"@en ;
        rdfs:range          pproc:CommitteeMember ;
        rdfs:subPropertyOf  foaf:member .

pproc:constructionSubsidies
        a             owl:DatatypeProperty ;
        rdfs:comment  "Descripción de las aportaciones públicas a la construcción."@es , "Description of the public subsidies to construction works contracts."@en ;
        rdfs:domain   pproc:ContractEconomicConditions ;
        rdfs:label    "Aportaciones públicas"@es , "Construction subsidies"@en ;
        rdfs:range    xsd:string .

pproc:noticeSite  a   owl:DatatypeProperty ;
        rdfs:comment  "Esta propiedad se refiere al medio donde ha publicado el anuncio. Habitualmente este será un boletín o diario oficial, por ejemplo, el DOUE, BOE o boletín autonómico correspondiente, pero puede ser que sea publicado en prensa u otros medios."@es , "Property that indicates the sire where the notice is published. Normally it would be an official source, like the Official Jounral of the European Union, but it can be anywhere else, like press."@en ;
        rdfs:domain   pproc:Notice ;
        rdfs:label    "Medio de publicación del anuncio"@es , "Notice site"@en ;
        rdfs:range    xsd:string .

pproc:TechnicalCommittee
        a                owl:Class ;
        rdfs:label       "Organismo técnico"@es , "Technical committee"@en ;
        rdfs:subClassOf  pproc:Committee .

pproc:reservedContractRestrictions
        a            owl:DatatypeProperty ;
        rdfs:domain  pproc:TenderersRequirements ;
        rdfs:label   "Contratos reservados"@es , "Reserved contract restrictions"@en ;
        rdfs:range   xsd:string .

pproc:tenderRequirements
        a            owl:FunctionalProperty , owl:ObjectProperty ;
        rdfs:domain  pproc:Contract ;
        rdfs:label   "Requisitos para las ofertas"@es , "Tender requirements"@en ;
        rdfs:range   pproc:TenderRequirements .

pproc:complementaryContract
        a             owl:ObjectProperty ;
        rdfs:comment  "Relaciona un contrato con otro contrato complementario."@es , "Relates a contract with a complementary contract."@en ;
        rdfs:domain   pproc:Contract ;
        rdfs:label    "Contrato complementario"@es , "Complementary contract"@en ;
        rdfs:range    pproc:Contract .

pproc:offeredEndDate  a     owl:FunctionalProperty , owl:DatatypeProperty ;
        rdfs:domain         pc:Tender ;
        rdfs:label          "Fecha de finalización ofertada"@es , "Offered end date"@en ;
        rdfs:range          xsd:date ;
        rdfs:subPropertyOf  dcterms:date .

pproc:OrdinaryAdministrativeRemedy
        a                owl:Class ;
        rdfs:label       "Recurso administrativo ordinario"@es , "Ordinary administrative remedy"@en ;
        rdfs:subClassOf  pproc:Remedy .

pc:Tender  a              owl:Class ;
        rdfs:isDefinedBy  pc: ;
        rdfs:label        "Oferta de licitación"@es , "Tender"@en .

pproc:price  a      owl:ObjectProperty ;
        rdfs:label  "Precio"@es , "Price"@en ;
        rdfs:range  v1:PriceSpecification .

pc:criteronName  a        owl:DatatypeProperty ;
        rdfs:isDefinedBy  pc: ;
        rdfs:label        "Nombre del criterio"@es , "Criterion name"@en .

pproc:SimpleOpen  a        skos:Concept , owl:NamedIndividual ;
        rdfs:label         "Abierto simple"@es , "Simple open"@en ;
        skos:inScheme      pproc:ProcedureTypeScheme ;
        skos:topConceptOf  pproc:ProcedureTypeScheme .

pproc:PrecomercialProcurement
        a                owl:Class ;
        rdfs:label       "Compra pública pre-comercial"@es , "Precomercial procurement"@en ;
        rdfs:subClassOf  pproc:Contract .

pproc:SharedResultAgreementContract
        a                owl:Class ;
        rdfs:comment     "Clase de los contrato en cuya virtud la Administración y el empresario participarán en los resultados de la explotación del servicio en la proporción que se establezca en el contrato."@es , "Class describing contracts whose operation results are shared among the contracting authority and the tenderer."@en ;
        rdfs:label       "Gestión interesada"@es , "Shared result agreement contract"@en ;
        rdfs:subClassOf  pproc:PublicServicesManagementContract .

s:startDate  a            owl:DatatypeProperty ;
        rdfs:isDefinedBy  s: ;
        rdfs:label        "Fecha de inicio"@es , "Start date"@en .

pproc:criterionEvaluationMode
        a             owl:DatatypeProperty ;
        rdfs:comment  "Propiedad para describir la forma de valoración del criterio."@es , "Property textually describing the criterion evaluarion mode."@en ;
        rdfs:domain   pc:AwardCriterion ;
        rdfs:label    "Forma de evaluación del criterio"@es , "Criterion evaluation mode"@en ;
        rdfs:range    xsd:string .

pproc:ProcedureWaive  a  owl:Class ;
        rdfs:label       "Renuncia del procedimiento"@es , "Procedure waive"@en ;
        rdfs:subClassOf  pproc:ContractOrProcedureExtinction .

skos:Concept  a           owl:Class ;
        rdfs:isDefinedBy  skos: ;
        rdfs:label        "Concepto"@es , "Concept"@en .

pproc:procedureVoid  a      owl:ObjectProperty ;
        rdfs:label          "Procedimiento desierto"@es , "Procedure void"@en ;
        rdfs:range          pproc:ProcedureVoid ;
        rdfs:subPropertyOf  pproc:contractOrProcedureExtinction .

pc:awardCriteriaCombination
        a                 owl:ObjectProperty ;
        rdfs:isDefinedBy  pc: ;
        rdfs:label        "Combinación de criterios para la adjudicación"@es , "Award criteria combination"@en .

pproc:ContractingBodyAgreement
        a           owl:Class ;
        rdfs:label  "Acuerdo del órgano de contratación"@es , "Contracting body agreement"@en .

pproc:extinctionCause
        a            owl:DatatypeProperty ;
        rdfs:domain  pproc:ContractOrProcedureExtinction ;
        rdfs:label   "Causa de extinctión"@es , "Extinction cause"@en ;
        rdfs:range   xsd:string .

pproc:noticeSentDate  a     owl:FunctionalProperty , owl:DatatypeProperty ;
        rdfs:domain         pproc:Notice ;
        rdfs:label          "Fecha de envio del anuncio"@es , "Notice sent date"@en ;
        rdfs:range          xsd:date ;
        rdfs:subPropertyOf  dcterms:date .

pproc:expectedCauseModification
        a            owl:DatatypeProperty ;
        rdfs:domain  pproc:ContractModificationConditions ;
        rdfs:label   "Causas previstas de modificación"@es , "Expected cause modification"@en ;
        rdfs:range   xsd:string .

pc:lot  a                 owl:ObjectProperty ;
        rdfs:isDefinedBy  pc: ;
        rdfs:label        "Lote"@es , "Lot"@en .

<https://www.linkedin.com/profile/view?id=218098827>
        a       foaf:Person , owl:NamedIndividual .

s:PostalAddress  a        owl:Class ;
        rdfs:isDefinedBy  s: ;
        rdfs:label        "Dirección postal"@es , "Postal address"@en .

pc:tender  a              owl:ObjectProperty ;
        rdfs:isDefinedBy  pc: ;
        rdfs:label        "Oferta presentada"@es , "Submitted tender"@en .

pproc:LeaseContract  a   owl:Class ;
        rdfs:comment     "Clase de los contratos de suministros cuyo objeto es el arrendamiento financiero de bienes.\n\nPopularmente conocido como 'renting' en España."@es , "Class defining supplies contracts aimed to lease supplies."@en ;
        rdfs:label       "Arrendamiento financiero"@es , "Lease contract"@en ;
        rdfs:subClassOf  pproc:SuppliesContract .

[ a            owl:AllDisjointClasses ;
  owl:members  ( pproc:MixedContract pproc:PrecomercialProcurement pproc:PrivateContract pproc:PublicPrivatePartnershipContract pproc:PublicServicesManagementContract pproc:PublicWorksConcessionContract pproc:ServicesContract pproc:SpecialAdministrativeContract pproc:SuppliesContract pproc:WorksContract )
] .

pproc:PriorInformationNotice
        a                owl:Class ;
        rdfs:label       "Anuncio de información previa"@es , "Prior information notice"@en ;
        rdfs:subClassOf  pproc:Notice .

s:streetAddress  a        owl:DatatypeProperty ;
        rdfs:isDefinedBy  s: ;
        rdfs:label        "Calle"@es , "Street address"@en .

pproc:ContractResolution
        a                owl:Class ;
        rdfs:label       "Resolución del contrato"@es , "Contract resolution"@en ;
        rdfs:subClassOf  pproc:ContractOrProcedureExtinction .

pproc:PublicWorksConcessionContract
        a                owl:Class ;
        rdfs:label       "Contrato de concesión de obras públicas"@es , "Public works concession contract"@en ;
        rdfs:subClassOf  pproc:Contract .

pproc:ProcedureResignation
        a                owl:Class ;
        rdfs:label       "Desistimiento del procedimiento"@es , "Procedure resignation"@en ;
        rdfs:subClassOf  pproc:ContractOrProcedureExtinction .

pproc:LegalRemedy  a     owl:Class ;
        rdfs:label       "Recurso legal"@es , "Legal remedy"@en ;
        rdfs:subClassOf  pproc:Remedy .

pproc:SpecialAdministrativeContract
        a                owl:Class ;
        rdfs:label       "Contrato administrativo especial"@es , "Special administrative contract"@en ;
        rdfs:subClassOf  pproc:Contract .

pproc:tenderCommitteeRole
        a             owl:FunctionalProperty , owl:DatatypeProperty ;
        rdfs:comment  "Indica el cargo que una persona ostenta dentro del comité del contratación."@es , "Indicated the role of a person inside the committee."@en ;
        rdfs:domain   pproc:CommitteeMember ;
        rdfs:label    "Cargo en el comité de contratación"@es , "Tender committee role"@en ;
        rdfs:range    xsd:string .

[ a            owl:AllDisjointClasses ;
  owl:members  ( pproc:BuyContract pproc:LeaseContract pproc:RentContract )
] .

pproc:NegotiatedWithPublicity
        a              skos:Concept , owl:NamedIndividual ;
        rdfs:label     "Negociado con publicidad"@es , "Negotiated with publicity"@en ;
        skos:broader   pproc:Negotiated ;
        skos:inScheme  pproc:ProcedureTypeScheme .

pproc:maxInvitations  a  owl:DatatypeProperty ;
        rdfs:domain  pproc:ContractProcedureSpecifications ;
        rdfs:label   "Número máximo de invitaciones"@es , "Maximum number of invitations"@en ;
        rdfs:range   xsd:string .

pproc:RentContract  a    owl:Class ;
        rdfs:comment     "Clase de los contratos de suministros cuyo objeto es el alquiler de bienes."@es , "Class defining supplies contracts aimed to rent supplies."@en ;
        rdfs:label       "Contrato de alquiler"@es , "Rent contract"@en ;
        rdfs:subClassOf  pproc:SuppliesContract .

pproc:actualDuration  a     owl:FunctionalProperty , owl:DatatypeProperty ;
        rdfs:domain         pproc:Contract ;
        rdfs:label          "Duración final"@es , "Actual duration"@en ;
        rdfs:subPropertyOf  pproc:duration .

[ a            owl:AllDisjointClasses ;
  owl:members  ( pproc:ContractWithLots pproc:ContractWithoutLots pproc:Lot )
] .

pproc:AdministrativeInformation
        a                  skos:Concept , owl:NamedIndividual ;
        rdfs:label         "Información administrativa"@es , "Administrative information"@en ;
        skos:inScheme      pproc:InformationKindScheme ;
        skos:topConceptOf  pproc:InformationKindScheme .

pproc:contractEconomicConditions
        a            owl:FunctionalProperty , owl:ObjectProperty ;
        rdfs:domain  pproc:ContractObject ;
        rdfs:label   "Condiciones económicas del contrato"@es , "Contract economic conditions"@en ;
        rdfs:range   pproc:ContractEconomicConditions .

pc:actualPrice  a           owl:ObjectProperty ;
        rdfs:isDefinedBy    pc: ;
        rdfs:label          "Precio final"@es , "Actual price"@en ;
        rdfs:subPropertyOf  pproc:price .

pproc:ContractObject  a  owl:Class ;
        rdfs:comment  "Clase que define el objeto del contrato y las diferentes condiciones, obligaciones y modificaciones de este."@es , "Class that defines the object of the contract and the conditions or modifications the contract can have."@en ;
        rdfs:label    "Objeto del contato"@es , "Contract object"@en .

pproc:endMode  a     owl:DatatypeProperty ;
        rdfs:domain  pproc:ElectronicAuctionPhase ;
        rdfs:label   "Modo de finalización"@es , "End mode"@en ;
        rdfs:range   xsd:string .

org:Organization  a       owl:Class ;
        rdfs:isDefinedBy  org: ;
        rdfs:label        "Organización"@es , "Organization"@en .

skos:topConceptOf  a      owl:ObjectProperty ;
        rdfs:isDefinedBy  skos: ;
        rdfs:label        "Concepto superior"@es , "Top concept of"@en .

[ a            owl:AllDisjointClasses ;
  owl:members  ( pproc:AgreementContract pproc:ConcessionContract pproc:MixedCapitalCompanyContract pproc:SharedResultAgreementContract )
] .

pproc:ExpertCommittee
        a                owl:Class ;
        rdfs:label       "Comité de expertos"@es , "Expert committee"@en ;
        rdfs:subClassOf  pproc:Committee .

pproc:documentReference
        a             owl:ObjectProperty ;
        rdfs:comment  "Enlace a documentación.\n\nPropiedad similar a pc:attachment, pero sin dominio fijo, pues esta misma propiedad puede utilizarse con múltiples clases (e.g. pc:Contract ó contsem:TenderMeeting)"@es , "Links to external documents."@en ;
        rdfs:label    "Documentación"@es , "Document reference"@en ;
        rdfs:range    foaf:Document ;
        rdfs:seeAlso  pc:attachment .

pproc:contractActivites
        a            owl:FunctionalProperty , owl:ObjectProperty ;
        rdfs:domain  pproc:ContractProcedureSpecifications ;
        rdfs:label   "Trámites del contrato"@es , "Contract activities"@en ;
        rdfs:range   pproc:ContractActivities .

pproc:procedureWaive  a     owl:ObjectProperty ;
        rdfs:label          "Renuncia del procedimiento"@es , "Procedure waive"@en ;
        rdfs:range          pproc:ProcedureWaive ;
        rdfs:subPropertyOf  pproc:contractOrProcedureExtinction .

pproc:electronicAuctionPhase
        a            owl:ObjectProperty ;
        rdfs:domain  pproc:ElectronicAuction ;
        rdfs:label   "Fase de subasta electrónica"@es , "Electronic auction phase"@en ;
        rdfs:range   pproc:ElectronicAuctionPhase .

pproc:otherAbilityRequisites
        a            owl:DatatypeProperty ;
        rdfs:domain  pproc:TenderersRequirements ;
        rdfs:label   "Otros requisitos"@es , "Other ability requisites"@en ;
        rdfs:range   xsd:string .

pproc:Negotiated  a        owl:NamedIndividual , skos:Concept ;
        rdfs:comment       "Abstract concept defining the procedure of the contract as negotiated."@en ;
        rdfs:label         "Negociado"@es , "Negotiated"@en ;
        owl:sameAs         pc:Negotiated ;
        skos:inScheme      pproc:ProcedureTypeScheme ;
        skos:narrower      pproc:NegotiatedWithoutPublicity , pproc:NegotiatedWithPublicity ;
        skos:topConceptOf  pproc:ProcedureTypeScheme .

pproc:technicalDocumentReference
        a                   owl:ObjectProperty ;
        rdfs:domain         pproc:Contract ;
        rdfs:label          "Pliego de prescripciones técnicas"@es , "Technical document reference"@en ;
        rdfs:subPropertyOf  pproc:documentReference .

pproc:ProcedureVoid  a   owl:Class ;
        rdfs:label       "Procedimiento desierto"@es , "Procedure void"@en ;
        rdfs:subClassOf  pproc:ContractOrProcedureExtinction .

pproc:variantDescription
        a             owl:DatatypeProperty ;
        rdfs:comment  "Campo para incluir la descripción, alcance, plazo u otros aspectos que están permitidos al presentar variantes en un contrato."@es , "Property to describe the allowed variantes when submitting a variant of a contract."@en ;
        rdfs:domain   pproc:ContractObject ;
        rdfs:label    "Descripción de las variantes"@es , "Variant description"@en ;
        rdfs:range    xsd:string .

pproc:Regular  a           skos:Concept , owl:NamedIndividual ;
        rdfs:label         "Ordinaria"@es , "Regular"@en ;
        skos:inScheme      pproc:UrgencyTypeScheme ;
        skos:topConceptOf  pproc:UrgencyTypeScheme .

pproc:ContractWithoutLots
        a                owl:Class ;
        rdfs:comment     "Clase de los contratos que no están dividos en lotes."@es , "Class to describe the contract not divided into lots."@en ;
        rdfs:label       "Contrato sin lotes"@es , "Contract without lots"@en ;
        rdfs:subClassOf  pproc:Contract ;
        rdfs:subClassOf  [ a               owl:Restriction ;
                           owl:hasValue    0 ;
                           owl:onProperty  pproc:numberOfLots
                         ] ;
        rdfs:subClassOf  [ a                            owl:Restriction ;
                           owl:maxQualifiedCardinality  "0"^^xsd:nonNegativeInteger ;
                           owl:onClass                  pproc:Lot ;
                           owl:onProperty               pproc:lot
                         ] .

pproc:frameworkAgreement
        a             owl:FunctionalProperty , owl:ObjectProperty ;
        rdfs:comment  "Señala al acuerdo marco o sistema dinámico de contratación en el cual consiste el contrato.\n\nEsta propiedad se utiliza cuando el actual contrato consista en la declaración de un acuerdo marco o un sistema dinámico de contratación."@es , "Property that indicates the framework agreement in which the contract consists.\n\nThis property is used when the actual contract consist in the declaration of a framework agreement or a dynamic purchasing system."@en ;
        rdfs:domain   pproc:Contract ;
        rdfs:label    "Acuerdo marco o sistema dinámico de contratación"@es , "Framework agreement"@en ;
        rdfs:range    pproc:FrameworkAgreement .

pproc:score  a        owl:FunctionalProperty , owl:DatatypeProperty ;
        rdfs:comment  "Indica la puntuación que ha recibido un criterio."@es ;
        rdfs:domain   pproc:CriterionScore ;
        rdfs:label    "Valoración"@es , "Puntuación"@es , "Score"@en ;
        rdfs:range    xsd:float .

pproc:ContractBodies  a  owl:Class ;
        rdfs:comment  "Clase que engloba los órganos relacionados con un contrato (e.g. mesa de contratación ó comité de expertos)."@es , "Class describing the bodies related to the contract."@en ;
        rdfs:label    "Órganos del contrato"@es , "Contract bodies"@en .

pproc:procedureResignation
        a                   owl:ObjectProperty ;
        rdfs:label          "Desistimiento del procedimiento"@es , "Procedure resignation"@en ;
        rdfs:range          pproc:ProcedureResignation ;
        rdfs:subPropertyOf  pproc:contractOrProcedureExtinction .

s:location  a             owl:ObjectProperty ;
        rdfs:isDefinedBy  s: ;
        rdfs:label        "Lugar"@es , "Location"@en .

pc:supplier  a            owl:ObjectProperty ;
        rdfs:isDefinedBy  pc: ;
        rdfs:label        "Proveedor"@es , "Supplier"@en .

pproc:estimatedDuration
        a                   owl:FunctionalProperty , owl:DatatypeProperty ;
        rdfs:domain         [ a            owl:Class ;
                              owl:unionOf  ( pproc:ContractTemporalConditions pproc:FrameworkAgreement v1:Offering )
                            ] ;
        rdfs:label          "Duración estimada"@es , "Estimated duration"@en ;
        rdfs:subPropertyOf  pproc:duration .

pproc:Briefing  a        owl:Class ;
        rdfs:comment     "Reunión informativa sobre la licitación del contrato."@es , "Informative meeting about the public procurement contract."@en ;
        rdfs:label       "Reunión informativa"@es , "Briefing"@en ;
        rdfs:subClassOf  s:Event .

pproc:modificationReason
        a            owl:DatatypeProperty ;
        rdfs:domain  pproc:ContractModification ;
        rdfs:label   "Justificación de la modificación"@es , "Modification reason"@en ;
        rdfs:range   xsd:string .

pproc:InformationProvider
        a             owl:Class ;
        rdfs:comment  "Proveedor de información sobre la licitación del contrato."@es , "Class defining the provider of information about the contract."@en ;
        rdfs:label    "Proveedor de información"@es , "Information provider"@en .

pproc:resolutionDocumentReference
        a                   owl:ObjectProperty ;
        rdfs:domain         pproc:ContractingBodyAgreement ;
        rdfs:label          "Resolución"@es , "Resolution document reference"@en ;
        rdfs:seeAlso        pc:agreement ;
        rdfs:subPropertyOf  pproc:documentReference .

pproc:tenderMeeting  a  owl:ObjectProperty ;
        rdfs:domain  [ a            owl:Class ;
                       owl:unionOf  ( pproc:Committee pproc:ContractActivities )
                     ] ;
        rdfs:label   "Reunión de la mesa de contratación"@es , "Tender meeting"@en ;
        rdfs:range   pproc:TenderMeeting .

pc:Open  a                skos:Concept , owl:NamedIndividual ;
        rdfs:isDefinedBy  pc: .

dcterms:date  a           owl:DatatypeProperty ;
        rdfs:isDefinedBy  dcterms: ;
        rdfs:label        "Fecha"@es , "Date"@en .

pproc:location  a                   owl:ObjectProperty ;
        rdfs:domain                 pproc:ContractObject ;
        rdfs:label                  "Lugar de realización del contrato"@es , "Place of contract's realization"@en ;
        rdfs:range                  s:Place ;
        owl:backwardCompatibleWith  pc:location .

pproc:ObjectiveAwardCriterion
        a                owl:Class ;
        rdfs:comment     "Clase para definir criterios que dependen de un juicio de valor."@es , "Class describing criterioa that depend on a value judgement."@en ;
        rdfs:label       "Criterio de adjudicación objetivo"@es , "Objective award criterion"@en ;
        rdfs:subClassOf  pc:AwardCriterion .

pproc:websiteWithInformation
        a            owl:ObjectProperty ;
        rdfs:domain  pproc:InformationProvider ;
        rdfs:label   "Web con información"@es , "Website with information"@en ;
        rdfs:range   foaf:Document .

pc:criterionWeight  a     owl:DatatypeProperty ;
        rdfs:isDefinedBy  pc: ;
        rdfs:label        "Peso del criterio"@es , "Criterion weight"@en .

pproc:alternateMember
        a                   owl:ObjectProperty ;
        rdfs:comment        "Miembro suplente en una mesa de contratación."@es , "Points to an alternate member of a committee."@en ;
        rdfs:domain         pproc:Committee ;
        rdfs:label          "Miembro suplente"@es , "Alternate member"@en ;
        rdfs:range          pproc:CommitteeMember ;
        rdfs:subPropertyOf  foaf:member .

pproc:ContractEconomicConditions
        a             owl:Class ;
        rdfs:comment  "Clase que define las condiciones económicas del contrato (e.g. presupuesto ó revisión de precios)."@es , "Class defining the actual economic conditions of the contract (e.g. budget or the formula that describes the revision of its price)."@en ;
        rdfs:label    "Condiciones económicas del contrato"@es , "Contract economic conditions"@en .

pproc:contractObject  a  owl:FunctionalProperty , owl:ObjectProperty ;
        rdfs:domain  pproc:Contract ;
        rdfs:label   "Objeto del contrato"@es , "Object of the contract"@en ;
        rdfs:range   pproc:ContractObject .

pproc:tenderSubmissionMode
        a            owl:DatatypeProperty ;
        rdfs:domain  pproc:ContractProcedureSpecifications ;
        rdfs:label   "Modalidad de presentación"@es , "Tender submission mode"@en ;
        rdfs:range   xsd:string .

pproc:tenderersRequirements
        a            owl:FunctionalProperty , owl:ObjectProperty ;
        rdfs:domain  pproc:Contract ;
        rdfs:label   "Requisitos de los licitadores"@es , "Tenderers requirements"@en ;
        rdfs:range   pproc:TenderersRequirements .

pproc:pricePercentageChange
        a             owl:FunctionalProperty , owl:DatatypeProperty ;
        rdfs:comment  "El rango en esta propiedad indica un porcentaje, por lo que el rango del número real a utilizar debe estar comprendido entre 0.0 y 100.0."@es , "The range of this property must be a percentage (i.e. float between 0.0 and 100.0)"@en ;
        rdfs:domain   pproc:ContractModification ;
        rdfs:label    "Porcentaje de variación sobre el precio"@es , "Price percentage change"@en ;
        rdfs:range    xsd:float .

[ a            owl:AllDisjointClasses ;
  owl:members  ( pproc:AdditionalInformationNotice pproc:ContractAwardNotice pproc:ContractNotice pproc:CorrectionNotice pproc:FormalizationNotice pproc:PriorInformationNotice )
] .

pproc:ElectronicAuctionPhase
        a                owl:Class ;
        rdfs:comment     "Fase de la subasta electrónica de uno o más de los criterios de adjudicación del contrato."@es , "Class describing a phase of an electronic auction."@en ;
        rdfs:label       "Fase de subasta electrónica"@es , "Electronic auction phase"@en ;
        rdfs:subClassOf  s:Event .

pproc:Committee  a    owl:Class ;
        rdfs:comment  "Clase abstracta que representa un conjunto de personas en comité y sus roles dentro del esta agrupación."@es , "Abstract class describing a set of persons in committee and its roles."@en ;
        rdfs:label    "Comité de contratación"@es , "Tender committee"@en .

pc:CompetitiveDialogue
        a                  skos:Concept , owl:NamedIndividual ;
        rdfs:isDefinedBy   pc: ;
        rdfs:label         "Diálogo competitvo"@es , "Competitive dialogue"@en ;
        skos:inScheme      pproc:ProcedureTypeScheme ;
        skos:topConceptOf  pproc:ProcedureTypeScheme .

foaf:Person  a            owl:Class , rdfs:Class ;
        rdfs:comment      "A person." ;
        rdfs:isDefinedBy  foaf: ;
        rdfs:label        "Persona"@es , "Person"@en , "Person" ;
        rdfs:subClassOf   <http://www.w3.org/2003/01/geo/wgs84_pos#SpatialThing> , <http://www.w3.org/2000/10/swap/pim/contact#Person> , foaf:Agent ;
        owl:disjointWith  foaf:Project , foaf:Organization ;
        ns2:term_status   "stable" .

pproc:maxBudgetChange
        a             owl:FunctionalProperty , owl:DatatypeProperty ;
        rdfs:comment  "El rango en esta propiedad indica un porcentaje, por lo que el rango del número real a utilizar debe estar comprendido entre 0.0 y 100.0."@es , "The range of this property must be a percentage (i.e. float between 0.0 and 100.0)"@en ;
        rdfs:domain   pproc:ContractModificationConditions ;
        rdfs:label    "Modificación máxima de presupuesto"@es , "Maximum budget change"@en ;
        rdfs:range    xsd:float .

pproc:minSubcontracting
        a             owl:FunctionalProperty , owl:DatatypeProperty ;
        rdfs:comment  "El rango en esta propiedad indica un porcentaje, por lo que el rango del número real a utilizar debe estar comprendido entre 0.0 y 100.0."@es , "The range of this property must be a percentage (i.e. float between 0.0 and 100.0)"@en ;
        rdfs:domain   pproc:ContractExecutionConditions ;
        rdfs:label    "Subcontratación mínima"@es , "Minimum subcontracting"@en ;
        rdfs:range    xsd:float .

pproc:urgencyType  a  owl:FunctionalProperty , owl:ObjectProperty ;
        rdfs:domain   pproc:ContractProcedureSpecifications ;
        rdfs:label    "Tipo de tramitación"@es , "Urgency type"@en ;
        rdfs:range    skos:Concept ;
        rdfs:range    [ a               owl:Restriction ;
                        owl:hasValue    pproc:UrgencyTypeScheme ;
                        owl:onProperty  skos:inScheme
                      ] ;
        rdfs:seeAlso  pproc:UrgencyTypeScheme .

pproc:numberOfLots  a  owl:FunctionalProperty , owl:DatatypeProperty ;
        rdfs:domain  pproc:Contract ;
        rdfs:label   "Número de lotes"@es , "Number of lots"@en ;
        rdfs:range   xsd:nonNegativeInteger .

pproc:AwardedTender  a              owl:Class ;
        rdfs:comment                "Clase para definir las oferta que han sido adjudicadas."@es , "Class describing the awarded tenders."@en ;
        rdfs:label                  "Oferta adjudicada"@es , "Awarded tender"@en ;
        rdfs:subClassOf             pc:Tender ;
        owl:backwardCompatibleWith  pc:awardedTender .

pproc:provisionalFinancialGuarantee
        a            owl:FunctionalProperty , owl:DatatypeProperty ;
        rdfs:domain  pproc:ContractAdditionalObligations ;
        rdfs:label   "Garantía provisional"@es , "Provisional financial guarantee"@en ;
        rdfs:range   xsd:string .

pproc:contractResolution
        a                   owl:ObjectProperty ;
        rdfs:label          "Resolución de contrato"@es , "Contract resolution"@en ;
        rdfs:range          pproc:ContractResolution ;
        rdfs:subPropertyOf  pproc:contractOrProcedureExtinction .

pproc:informationKind
        a             owl:ObjectProperty ;
        rdfs:comment  "Indica el tipo de información que suministra un proveedor de información.\n\nEs posible utilizar esta propiedad numerosas veces para indicar diversos tipos de información."@es , "Property pointing to the type of the information is provided."@en ;
        rdfs:domain   pproc:InformationProvider ;
        rdfs:label    "Tipo de información"@es , "Information kind"@en ;
        rdfs:range    skos:Concept ;
        rdfs:range    [ a               owl:Restriction ;
                        owl:hasValue    pproc:InformationKindScheme ;
                        owl:onProperty  skos:inScheme
                      ] ;
        rdfs:seeAlso  pproc:InformationKindScheme .

pproc:prorogationsExpected
        a            owl:FunctionalProperty , owl:DatatypeProperty ;
        rdfs:domain  pproc:ContractTemporalConditions ;
        rdfs:label   "Prórrogas previstas"@es , "Prorogation number expected"@en ;
        rdfs:range   xsd:nonNegativeInteger .

pproc:contractBodies  a  owl:FunctionalProperty , owl:ObjectProperty ;
        rdfs:domain  pproc:ContractProcedureSpecifications ;
        rdfs:label   "Órganos del contrato"@es , "Contract bodies"@en ;
        rdfs:range   pproc:ContractBodies .

pproc:criterionMaxAndMinScores
        a            owl:DatatypeProperty ;
        rdfs:domain  pc:AwardCriterion ;
        rdfs:label   "Puntuación máxima y mínima del criterio"@es , "Criterion maximum and minimum score"@en ;
        rdfs:range   xsd:string .

pproc:Minor  a             skos:Concept , owl:NamedIndividual ;
        rdfs:label         "Menor"@es , "Minor"@en ;
        skos:inScheme      pproc:ProcedureTypeScheme ;
        skos:topConceptOf  pproc:ProcedureTypeScheme .

pproc:ConcessionContract
        a                owl:Class ;
        rdfs:comment     "Clase de los contratos en los que el empresario gestionará el servicio a su propio riesgo y ventura."@es , "Class of the contracts in which the awarded tenderer manage the public service themselves."@en ;
        rdfs:label       "Concesión"@es , "Concession contract"@en ;
        rdfs:subClassOf  pproc:PublicServicesManagementContract .

pproc:briefing  a    owl:ObjectProperty ;
        rdfs:domain  pproc:ContractProcedureSpecifications ;
        rdfs:label   "Reunión informativa"@es , "Briefing"@en ;
        rdfs:range   pproc:Briefing .

pproc:minInvitations  a  owl:DatatypeProperty ;
        rdfs:domain  pproc:ContractProcedureSpecifications ;
        rdfs:label   "Número mínimo de invitaciones"@es , "Minimum number of invitations"@en ;
        rdfs:range   xsd:string .

pproc:tenderManteinanceDuration
        a                   owl:FunctionalProperty , owl:DatatypeProperty ;
        rdfs:domain         pproc:TenderRequirements ;
        rdfs:label          "Plazo de vigencia de las ofertas"@es , "Tender manteinance duration"@en ;
        rdfs:subPropertyOf  pproc:duration .

pproc:TenderMeeting  a   owl:Class ;
        rdfs:comment     "Clase para describir las reuniones que la mesa de contratación, comité de expertos u organismos técnicas han realizado."@es , "Class describing the meetings of tender committee."@en ;
        rdfs:label       "Reunión de la mesa de contratación"@es , "Tender meeting"@en ;
        rdfs:subClassOf  s:Event .

skos:inScheme  a          owl:ObjectProperty ;
        rdfs:isDefinedBy  skos: ;
        rdfs:label        "En esquema"@es , "In scheme"@en .

pproc:ContractModification
        a             owl:Class ;
        rdfs:comment  "Durante un contrato se puede dar también la necesidad de modificarlo una vez iniciada su ejecución, para plasmar este tipo de casos se debe utilizar esta clase."@es , "During the execution of a contract it could happen that the contract should be modified, to describe these kind of situations we use this class."@en ;
        rdfs:label    "Modificación del contrato"@es , "Contract modification"@en .

pproc:ContractTemporalConditions
        a             owl:Class ;
        rdfs:comment  "Clase que define las condiciones temporales de un contrato (e.g. plazo ó prórrogas)."@es , "Class that describes the temporal conditions of the contract."@en ;
        rdfs:label    "Condiciones temporales del contrato"@es , "Contract temporal conditions"@en .

pproc:tenderDocumentNeeds
        a             owl:DatatypeProperty ;
        rdfs:comment  "Define la documentación necesaria a presentar en las ofertas."@es , "Defines the necessary documentation a tender must include."@en ;
        rdfs:domain   pproc:TenderRequirements ;
        rdfs:label    "Documentación a presentar"@es , "Tender document needs"@en ;
        rdfs:range    xsd:string .

<http://webdiis.unizar.es/~seron/>
        a       foaf:Person , owl:NamedIndividual .

pproc:durationChange  a  owl:FunctionalProperty , owl:DatatypeProperty ;
        rdfs:domain  pproc:ContractModification ;
        rdfs:label   "Variación del plazo"@es , "Duration change"@en ;
        rdfs:range   xsd:string .

pproc:tenderDeadline  a     owl:FunctionalProperty , owl:DatatypeProperty ;
        rdfs:domain         pproc:ContractProcedureSpecifications ;
        rdfs:label          "Fecha límite para la presentación de ofertas o de peticiones a participar"@es , "Time-limit for submission of tenders or requests to participate"@en ;
        rdfs:range          xsd:dateTime ;
        rdfs:subPropertyOf  dcterms:date .

pproc:requiredEconomicAndFinancialStanding
        a            owl:DatatypeProperty ;
        rdfs:domain  pproc:TenderersRequirements ;
        rdfs:label   "Solvencia económica y financiera requerida"@es , "Required economic and financial standing"@en ;
        rdfs:range   xsd:string .

pproc:CriterionScore  a  owl:Class ;
        rdfs:comment  "Clase para valorar individualmente un criterio de adjudicación. Esta formada por una puntuación (contsem:score) y un criterio (contsem:criterion)."@es , "Class to describe an award criterion and its score."@en ;
        rdfs:label    "Valoración de criterio"@es , "Criterion score"@en .

s:Event  a                owl:Class ;
        rdfs:isDefinedBy  s: ;
        rdfs:label        "Evento"@es , "Event"@en .

pproc:FrameworkDerivativeContract
        a                owl:Class ;
        rdfs:comment     "Clase de los contratos derivados de un acuerdo marco"@es , "Class describing contracts derived from a framework agreement."@en ;
        rdfs:label       "Contrato derivado de un acuerdo marco"@es , "Framework derivative contract"@en ;
        rdfs:subClassOf  pproc:DerivativeContract .

pproc:Contract  a        owl:Class ;
        rdfs:label       "Contrato público"@es , "Public contract"@en ;
        rdfs:subClassOf  pc:Contract .

pproc:BuyContract  a     owl:Class ;
        rdfs:comment     "Clase de los contratos de suministros cuyo objeto es la compra de bienes."@es , "Class to describe the supplies contracts aimed to buy supplies."@en ;
        rdfs:label       "Contrato de compra"@es , "Buy contract"@en ;
        rdfs:subClassOf  pproc:SuppliesContract .

pproc:Lot  a             owl:Class ;
        rdfs:comment     "Clase de los contratos que representan un lote perteneciente a otro contrato."@es , "Class describing contracts that are an actual lot of another contract."@en ;
        rdfs:label       "Lote"@es , "Lot"@en ;
        rdfs:subClassOf  pproc:Contract .

pproc:estimatedValue  a             owl:FunctionalProperty , owl:ObjectProperty ;
        rdfs:domain                 pproc:ContractEconomicConditions ;
        rdfs:label                  "Valor estimado del contrato"@es , "Estimated value of the contract"@en ;
        rdfs:range                  pproc:BundlePriceSpecification ;
        rdfs:subPropertyOf          pproc:price ;
        owl:backwardCompatibleWith  pc:estimatedPrice .

pproc:criterion  a   owl:FunctionalProperty , owl:ObjectProperty ;
        rdfs:domain  pproc:CriterionScore ;
        rdfs:label   "Criterio"@es , "Criterion"@en ;
        rdfs:range   pc:AwardCriterion .

pproc:delegatingAuthority
        a             owl:FunctionalProperty , owl:ObjectProperty ;
        rdfs:comment  "Indica la entidad que delega la licitación de este contrato."@es , "Points to the authority that is delegating the contract."@en ;
        rdfs:domain   pproc:Contract ;
        rdfs:label    "Entidad delegante"@es , "Delegating authority"@en ;
        rdfs:range    org:Organization .

pproc:WorksContract  a   owl:Class ;
        rdfs:label       "Contrato de obras"@es , "Works contract"@en ;
        rdfs:subClassOf  pproc:Contract .

pproc:ContractProcedureSpecifications
        a             owl:Class ;
        rdfs:comment  "Clase que define las especificaciones del procedimiento de un contrato (e.g. tipo de procedimiento o de tramitación)."@es , "Class that specifies the procedure of a contract (e.g. type of procedure or its urgency)."@en ;
        rdfs:label    "Procedimiento del contrato"@es , "Contract procedure"@en .

pproc:noticeWeb  a   owl:FunctionalProperty , owl:ObjectProperty ;
        rdfs:domain  pproc:Notice ;
        rdfs:label   "Web del anuncio"@es , "Notice web"@en ;
        rdfs:range   foaf:Document .

pproc:offeredDuration
        a                   owl:FunctionalProperty , owl:DatatypeProperty ;
        rdfs:domain         pc:Tender ;
        rdfs:label          "Plazo de ejecución ofertado"@es , "Offered duration"@en ;
        rdfs:subPropertyOf  pproc:duration .

pproc:PublicServicesManagementContract
        a                owl:Class ;
        rdfs:label       "Contrato de gestión de servicios públicos"@es , "Public services management contract"@en ;
        rdfs:subClassOf  pproc:Contract .

pproc:ContractModificationConditions
        a             owl:Class ;
        rdfs:comment  "Clase que define las condiciones para la modificación de un contrato (e.g. porcentaje máximo de modificación del presupuesto)."@es , "Class describing the conditions for which a contract can be modified (e.g. maximum percentage of its price or budget)."@en ;
        rdfs:label    "Condiciones para la modificación del contrato"@es , "Contract modification conditions"@en .

pproc:additionalDocumentReference
        a                   owl:ObjectProperty ;
        rdfs:domain         pproc:Contract ;
        rdfs:label          "Documentación adicional"@es , "Additional document reference"@en ;
        rdfs:subPropertyOf  pproc:documentReference .

<http://www.araid.es/en/users/jfm#profile-investigador>
        a       foaf:Person , owl:NamedIndividual .

pproc:Notice  a     owl:Class ;
        rdfs:label  "Anuncio"@es , "Notice"@en .

pproc:advertisementAmount
        a            owl:DatatypeProperty ;
        rdfs:domain  pproc:ContractAdditionalObligations ;
        rdfs:label   "Gastos de publicidad"@es , "Advertisement amount"@en ;
        rdfs:range   xsd:string .

pproc:awardAgreement  a  owl:ObjectProperty ;
        rdfs:comment  "Indica el acuerdo del órgano de contratación donde se ha adjudicado el contrato a un licitador."@es , "Points to the body agreement where a tender has been awarded."@en ;
        rdfs:domain   pc:Tender ;
        rdfs:label    "Acuerdo de adjudicación"@es , "Award agreement"@en ;
        rdfs:range    pproc:ContractingBodyAgreement .

pproc:ContractActivities
        a             owl:Class ;
        rdfs:comment  "Clase que engloba todos los trámites de un contrato (e.g. reuniones ó acuerdos del órgano de contratación)."@es , "Class describing all activities of a contract (e.g. meetings or agreements of the contracting body)."@en ;
        rdfs:label    "Trámites del contrato"@es , "Contract activites"@en .

pproc:isNegotiable  a  owl:FunctionalProperty , owl:DatatypeProperty ;
        rdfs:domain  pc:AwardCriterion ;
        rdfs:label   "Es negociable"@es , "Is negotiable"@en ;
        rdfs:range   xsd:boolean .

pproc:otherAwardTerms
        a            owl:DatatypeProperty ;
        rdfs:domain  pc:Tender ;
        rdfs:label   "Otras condiciones de la adjudicación"@es , "Other award terms"@en ;
        rdfs:range   xsd:string .

xsd:duration  a  rdfs:Datatype .

pproc:FormalizedTender
        a                owl:Class ;
        rdfs:comment     "Clase para definir la oferta que se ha formalizado."@es , "Class describing tenders being formalized."@en ;
        rdfs:label       "Oferta formalizada"@es , "Formalized tender"@en ;
        rdfs:subClassOf  pc:Tender ;
        rdfs:subClassOf  [ a                   owl:Restriction ;
                           owl:onProperty      pproc:formalizedDate ;
                           owl:someValuesFrom  xsd:date
                         ] .

pproc:formalizedDate  a     owl:FunctionalProperty , owl:DatatypeProperty ;
        rdfs:domain         pc:Tender ;
        rdfs:label          "Fecha de formalización"@es , "Formalized date"@en ;
        rdfs:range          xsd:date ;
        rdfs:subPropertyOf  dcterms:date .

pc:Negotiated  a          skos:Concept , owl:NamedIndividual ;
        rdfs:isDefinedBy  pc: .

pc:AwardCriterion  a      owl:Class ;
        rdfs:isDefinedBy  pc: ;
        rdfs:label        "Criterio de adjudicación"@es , "Award criterion"@en .

skos:narrower  a          owl:ObjectProperty ;
        rdfs:isDefinedBy  skos: ;
        rdfs:label        "Más concreto"@es , "Narrower"@en .

pproc:DerivativeContract
        a                owl:Class ;
        rdfs:comment     "Clase de los contratos derivados de un acuerdo marco o un sistema dinámico de contratación."@es , "Class describing contracts derived from a framework agreement or a dynamic purchasing system."@en ;
        rdfs:label       "Contrato derivado"@es , "Derivative contract"@en ;
        rdfs:subClassOf  pproc:Contract .

pproc:remedy  a      owl:ObjectProperty ;
        rdfs:domain  pproc:Contract ;
        rdfs:label   "Recurso"@es , "Remedy"@en ;
        rdfs:range   pproc:Remedy .

pproc:CorrectionNotice
        a                owl:Class ;
        rdfs:label       "Anuncio de corrección"@es , "Correction notice"@en ;
        rdfs:subClassOf  pproc:Notice .

pproc:minutesDocumentReference
        a                   owl:ObjectProperty ;
        rdfs:domain         pproc:TenderMeeting ;
        rdfs:label          "Acta"@es , "Minutes document reference"@en ;
        rdfs:subPropertyOf  pproc:documentReference .

pproc:contractTemporalConditions
        a            owl:FunctionalProperty , owl:ObjectProperty ;
        rdfs:domain  pproc:ContractObject ;
        rdfs:label   "Condiciones temporales del contrato"@es , "Contract temporal conditions"@en ;
        rdfs:range   pproc:ContractTemporalConditions .

pc:contractingAuthority
        a                 owl:ObjectProperty ;
        rdfs:isDefinedBy  pc: ;
        rdfs:label        "Entidad contratante"@es , "Contracting authority"@en .

pproc:finalFinancialGuaranteeDuration
        a                   owl:FunctionalProperty , owl:DatatypeProperty ;
        rdfs:domain         pproc:ContractAdditionalObligations ;
        rdfs:label          "Plazo de la garantía definitiva"@es , "Final financial guarantee duration"@en ;
        rdfs:subPropertyOf  pproc:duration .

s:addressLocality  a      owl:DatatypeProperty ;
        rdfs:isDefinedBy  s: ;
        rdfs:label        "Localidad"@es , "Address locality"@en .

pproc:DynamicPurchasingSystemConclusionContract
        a                owl:Class ;
        rdfs:comment     "Clase de los contratos que consisten en el establecimiento de un sistema dinámico de contratación."@es , "Class describing the contracts consisting in the conclusion of a dynamic purchasing system."@en ;
        rdfs:label       "Contrato de establecimiento de un sistema dinámico de contratación"@es , "Dynamic purchasing system conclusion contract"@en ;
        rdfs:subClassOf  pproc:ConclusionContract .

pproc:priceReviewIndex
        a            owl:DatatypeProperty ;
        rdfs:domain  pproc:ContractEconomicConditions ;
        rdfs:label   "Fórmula de revisión de precios"@es , "Price Review Index"@en ;
        rdfs:range   xsd:string .

pproc:ElectronicAuction
        a             owl:Class ;
        rdfs:comment  "Clase para especificar la realización de una subasta electrónica de uno o más criterios de adjudicación."@es , "Class that specifies the existence of an electronic auction of one or more of the award criterions."@en ;
        rdfs:label    "Subasta electrónica"@es , "Electronic auction"@en .

pproc:notice  a      owl:ObjectProperty ;
        rdfs:domain  [ a            owl:Class ;
                       owl:unionOf  ( pproc:ContractActivities pproc:ContractProcedureSpecifications )
                     ] ;
        rdfs:label   "Anuncio"@es , "Notice"@en ;
        rdfs:range   pproc:Notice .

pproc:modificationScope
        a            owl:DatatypeProperty ;
        rdfs:domain  pproc:ContractModification ;
        rdfs:label   "Alcance de la modificación"@es , "Modification scope"@en ;
        rdfs:range   xsd:string .

pc:AwardCriteriaCombination
        a                 owl:Class ;
        rdfs:isDefinedBy  pc: ;
        rdfs:label        "Combinación de criterios para la adjudicación"@es , "Award criteria combination"@en .

pproc:contractProcedureSpecifications
        a            owl:FunctionalProperty , owl:ObjectProperty ;
        rdfs:domain  pproc:Contract ;
        rdfs:label   "Especificaciones del procedimiento del contrato"@es , "Contract procedure specifications"@en ;
        rdfs:range   pproc:ContractProcedureSpecifications .

pproc:ServicesContract
        a                owl:Class ;
        rdfs:label       "Contrato de servicios"@es , "Services contract"@en ;
        rdfs:subClassOf  pproc:Contract .

pproc:requiredClassification
        a            owl:DatatypeProperty ;
        rdfs:domain  pproc:TenderersRequirements ;
        rdfs:label   "Clasificación requerida"@es , "Required classification"@en ;
        rdfs:range   xsd:string .

pproc:MultiannualContract
        a                owl:Class ;
        rdfs:comment     "Clase de los contrato plurianuales (i.e. contratos cuya duración se extiende durante más de un ejercicio contable)."@es , "Class describing the multiannual contracts (i.e. contract whose duration extends over more than one financial year)."@en ;
        rdfs:label       "Contrato plurianual"@es , "Multiannual contract"@en ;
        rdfs:subClassOf  pproc:Contract .

pproc:contractingBodyAgreement
        a            owl:ObjectProperty ;
        rdfs:domain  [ a            owl:Class ;
                       owl:unionOf  ( pproc:ContractActivities pproc:ContractModification pproc:ContractOrProcedureExtinction pproc:ContractProcedureSpecifications )
                     ] ;
        rdfs:label   "Acuerdo del órgano de contratación"@es , "Contracting body agreement"@en ;
        rdfs:range   pproc:ContractingBodyAgreement .

pproc:tenderSubmissionSupportedLanguage
        a            owl:DatatypeProperty ;
        rdfs:domain  pproc:TenderRequirements ;
        rdfs:label   "Idioma admitido en la presentación de oferta"@es , "Tender submission supported language"@en ;
        rdfs:range   xsd:string .

pproc:HarmonizedContract
        a                owl:Class ;
        rdfs:comment     "Clase de los contratos armonizados (i.e. contratos que alcanzan el umbral para actuar conforme a las Directivas del Parlamento Europeo y del Consejo en contratos públicos)"@es , "Class to describe harmonized contracts (i.e. contracts that reachs the threshold to be treated as highlighted in the procurement Directives of the European Commision and European Council)."@en ;
        rdfs:label       "Contrato armonizado"@es , "Harmonized contract"@en ;
        rdfs:subClassOf  pproc:Contract .

pproc:criterionScore  a  owl:ObjectProperty ;
        rdfs:comment  "Especifica la valoración de un único criterio, por lo que se utilizará una vez por cada criterio de adjudicación presente en el contrato."@es , "Property that points to an unique criterion and its score."@en ;
        rdfs:domain   pc:Tender ;
        rdfs:label    "Valoración de criterio"@es , "Criterion score"@en ;
        rdfs:range    pproc:CriterionScore .

pproc:frameworkAgreementDerivativeContract
        a            owl:InverseFunctionalProperty , owl:ObjectProperty ;
        rdfs:domain  pproc:ConclusionContract ;
        rdfs:label   "Contrato derivado de un acuerdo marco"@es , "Framework agreement derivative contract"@en ;
        rdfs:range   pproc:DerivativeContract .

pproc:PublicPrivatePartnershipContract
        a                owl:Class ;
        rdfs:label       "Contrato de colaboración público-privada"@es , "Public-private partnership contract"@en ;
        rdfs:subClassOf  pproc:Contract .

pproc:BundlePriceSpecification
        a                owl:Class ;
        rdfs:comment     "Clase que representa el precio de conjuntos de objetos o un paquete determinado.\n\nSe utiliza para especificar el precio de la clase gr:Offering cuando este precio se refiere al del conjunto de los objetos (y no a su precio unitario)."@es , "Class used to describe the price a set of objets.\n\nCan be used to define the total price of an gr:Offering. Its value must be equal to the gr:UnitPriceSpecification multiplied by the number of items."@en ;
        rdfs:label       "Precio de paquete"@es , "Bundle price"@en ;
        rdfs:subClassOf  v1:PriceSpecification .

pproc:DynamicPurchasingSystemDerivativeContract
        a                owl:Class ;
        rdfs:comment     "Clase de los contratos derivados de un sistema dinámico de contratación"@es , "Class describing contracts derived from a dynamic purchasing system."@en ;
        rdfs:label       "Contrato derivado de un sistema dinámico de contratación"@es , "Dynamic purchasing system derivative contract"@en ;
        rdfs:subClassOf  pproc:DerivativeContract .

pproc:maxNumberOfOperators
        a            owl:FunctionalProperty , owl:DatatypeProperty ;
        rdfs:domain  pproc:FrameworkAgreement ;
        rdfs:label   "Número máximo de participantes"@es , "Maximum number of operators"@en ;
        rdfs:range   xsd:nonNegativeInteger .

pc:onBehalfOf  a          owl:ObjectProperty ;
        rdfs:isDefinedBy  pc: ;
        rdfs:label        "En nombre de"@es , "On behalf of"@en .

pproc:FormalizationNotice
        a                owl:Class ;
        rdfs:label       "Anuncio de formalización"@es , "Formalization notice"@en ;
        rdfs:subClassOf  pproc:Notice .

pproc:maxSubcontracting
        a             owl:FunctionalProperty , owl:DatatypeProperty ;
        rdfs:comment  "El rango en esta propiedad indica un porcentaje, por lo que el rango del número real a utilizar debe estar comprendido entre 0.0 y 100.0."@es , "The range of this property must be a percentage (i.e. float between 0.0 and 100.0)"@en ;
        rdfs:domain   pproc:ContractExecutionConditions ;
        rdfs:label    "Subcontratación máxima"@es , "Maximum subcontracting"@en ;
        rdfs:range    xsd:float .

pproc:assumptionProtectingProcedureType
        a            owl:DatatypeProperty ;
        rdfs:domain  pproc:ContractProcedureSpecifications ;
        rdfs:label   "Supuesto que ampara el uso del procedimiento elegido"@es , "Assumption protecting the chosen procedure type"@en ;
        rdfs:range   xsd:string .

pproc:item  a                       owl:ObjectProperty ;
        rdfs:comment                "Property for attachment of an item to a tender."@en ;
        rdfs:domain                 pc:Tender ;
        rdfs:label                  "Artículo"@es , "Item"@en ;
        rdfs:range                  v1:Offering ;
        owl:backwardCompatibleWith  pc:item .

pproc:managingDepartment
        a             owl:FunctionalProperty , owl:ObjectProperty ;
        rdfs:comment  "Servicio perteneciente a la entidad contratante que se encarga de la publicación y administración de este contrato."@es , "Property that indicates the managing departament responsible of the contract."@en ;
        rdfs:domain   pproc:Contract ;
        rdfs:label    "Servicio gestor"@es , "Managing department"@en ;
        rdfs:range    org:Organization .

pproc:budgetPrice  a        owl:FunctionalProperty , owl:ObjectProperty ;
        rdfs:domain         pproc:ContractEconomicConditions ;
        rdfs:label          "Presupuesto del contrato"@es , "Contract budget price"@en ;
        rdfs:range          pproc:BundlePriceSpecification ;
        rdfs:subPropertyOf  pproc:price .

pproc:Emergency  a         skos:Concept , owl:NamedIndividual ;
        rdfs:label         "Emergencia"@es , "Emergency"@en ;
        skos:inScheme      pproc:UrgencyTypeScheme ;
        skos:topConceptOf  pproc:UrgencyTypeScheme .

pproc:provision  a                  owl:ObjectProperty ;
        rdfs:domain                 pproc:ContractObject ;
        rdfs:label                  "Prestación"@es , "Provision"@en ;
        rdfs:range                  v1:Offering ;
        owl:backwardCompatibleWith  pc:item .

pproc:electronicAuction
        a            owl:FunctionalProperty , owl:ObjectProperty ;
        rdfs:domain  pproc:ContractProcedureSpecifications ;
        rdfs:label   "Subasta electrónica"@es , "Electronic auction"@en ;
        rdfs:range   pproc:ElectronicAuction .

pproc:TenderersRequirements
        a             owl:Class ;
        rdfs:comment  "Clase que define los requisitos exigidos a los licitadores (e.g. clasificación profesional ó solvencia económica)."@es , "Class defining the tenderers requirements (e.g. required classification or financial capability)."@en ;
        rdfs:label    "Requisitos de los licitadores"@es , "Tenderers requirements"@en .

pproc:lodgedRemedyDate
        a                   owl:FunctionalProperty , owl:DatatypeProperty ;
        rdfs:comment        "Fecha en la cual se ha interpuesto el recurso ante el órgano oficial."@es , "Date where a remedy is lodged."@en ;
        rdfs:domain         pproc:Remedy ;
        rdfs:label          "Fecha de interposición del recurso"@es , "Lodged remedy date"@en ;
        rdfs:range          xsd:date ;
        rdfs:subPropertyOf  dcterms:date .

pproc:FrameworkConclusionContract
        a                owl:Class ;
        rdfs:comment     "Clase de los contratos que consisten en el establecimiento de un acuerdo marco."@es , "Class describing the contracts consisting in the conclusion of a framework agreement."@en ;
        rdfs:label       "Contrato de establecimiento de un acuerdo marco"@es , "Framework conclusion contract"@en ;
        rdfs:subClassOf  pproc:ConclusionContract .

pproc:variantAdmission
        a            owl:FunctionalProperty , owl:DatatypeProperty ;
        rdfs:domain  pproc:ContractObject ;
        rdfs:label   "Admisión de variantes"@es , "Variant admission"@en ;
        rdfs:range   xsd:boolean .

pproc:CommitteeMember
        a                owl:Class ;
        rdfs:comment     "Miembro perteneciente a un comité de contratación concreto."@es , "Class that describes the member a committee."@en ;
        rdfs:label       "Miembro del comité"@es , "Committee member"@en ;
        rdfs:subClassOf  foaf:Person .

pproc:contractModificationConditions
        a            owl:FunctionalProperty , owl:ObjectProperty ;
        rdfs:domain  pproc:ContractObject ;
        rdfs:label   "Condiciones para la modificación del contrato"@es , "Contract modification conditions"@en ;
        rdfs:range   pproc:ContractModificationConditions .

pc:awardCriterion  a      owl:ObjectProperty ;
        rdfs:isDefinedBy  pc: ;
        rdfs:label        "Criterio de adjudicación"@es , "Award criterion"@en .

pc:Restricted  a           skos:Concept , owl:NamedIndividual ;
        rdfs:isDefinedBy   pc: ;
        rdfs:label         "Restringido"@es , "Restricted"@en ;
        skos:inScheme      pproc:ProcedureTypeScheme ;
        skos:topConceptOf  pproc:ProcedureTypeScheme .

pproc:requiredTechnicalAndProfessionalAbility
        a            owl:DatatypeProperty ;
        rdfs:domain  pproc:TenderersRequirements ;
        rdfs:label   "Solvencia técnica y profesional requerida"@es , "Required technical and professional ability"@en ;
        rdfs:range   xsd:string .

pproc:Express  a           skos:Concept , owl:NamedIndividual ;
        rdfs:label         "Urgente"@es , "Express"@en ;
        skos:inScheme      pproc:UrgencyTypeScheme ;
        skos:topConceptOf  pproc:UrgencyTypeScheme .

pproc:tenderDossierStartDate
        a                   owl:FunctionalProperty , owl:DatatypeProperty ;
        rdfs:domain         pproc:ContractProcedureSpecifications ;
        rdfs:label          "Fecha de la resolución del inicio del expediente de contratación"@es , "Start date of the tender dossier"@en ;
        rdfs:range          xsd:date ;
        rdfs:subPropertyOf  dcterms:date .

pproc:contractExecutionConditions
        a            owl:FunctionalProperty , owl:ObjectProperty ;
        rdfs:domain  pproc:ContractObject ;
        rdfs:label   "Condiciones de ejecución del contrato"@es , "Contract execution conditions"@en ;
        rdfs:range   pproc:ContractExecutionConditions .

pproc:ConclusionContract
        a                 owl:Class ;
        rdfs:comment      "Clase de los contratos que consisten en el establecimiento de un acuerdo marco o un sistema dinámico de contratación."@es , "Class describing the contracts consisting in the conclusion of a framework agreement or a dynamic purchasing system."@en ;
        rdfs:label        "Contrato de establecimiento"@es , "Conclusion contract"@en ;
        rdfs:subClassOf   pproc:Contract ;
        rdfs:subClassOf   [ a                   owl:Restriction ;
                            owl:onProperty      pproc:frameworkAgreement ;
                            owl:someValuesFrom  pproc:FrameworkAgreement
                          ] ;
        owl:disjointWith  pproc:DerivativeContract .

pproc:PrivateContract
        a                owl:Class ;
        rdfs:label       "Contrato privado"@es , "Private contract"@en ;
        rdfs:subClassOf  pproc:Contract .

pproc:Remedy  a       owl:Class ;
        rdfs:comment  "Recurso interpuesto sobre alguna de las resoluciones del proceso de licitación."@es , "Remedy lodged concerning a resolution about the procurement procedure."@en ;
        rdfs:label    "Recurso"@es , "Remedy"@en .

pproc:feePrice  a           owl:FunctionalProperty , owl:ObjectProperty ;
        rdfs:domain         pproc:ContractEconomicConditions ;
        rdfs:label          "Canon"@es , "Fee"@en ;
        rdfs:range          pproc:BundlePriceSpecification ;
        rdfs:subPropertyOf  pproc:price .

pproc:ExcludedTender  a  owl:Class ;
        rdfs:comment     "Define las ofertas que han sido excluídas del proceso de licitación."@es , "Class that defines the tenders excluded from the procurement procedure."@en ;
        rdfs:label       "Oferta excluída"@es , "Excluded tender"@en ;
        rdfs:subClassOf  pc:Tender .

pproc:tenderSubmissionLocation
        a            owl:ObjectProperty ;
        rdfs:domain  pproc:ContractProcedureSpecifications ;
        rdfs:label   "Sede de presentación de las ofertas"@es , "Tender submission location"@en ;
        rdfs:range   s:Place .

pproc:committee  a   owl:ObjectProperty ;
        rdfs:domain  pproc:ContractBodies ;
        rdfs:label   "Comité"@es , "Committee"@en ;
        rdfs:range   pproc:Committee .

pproc:compulsoryMeansForExecution
        a            owl:DatatypeProperty ;
        rdfs:domain  pproc:TenderersRequirements ;
        rdfs:label   "Adscripción de medios"@es , "Compulsory means for execution"@en ;
        rdfs:range   xsd:string .

pproc:tenderAdmissionMeeting
        a            owl:ObjectProperty ;
        rdfs:domain  pproc:ContractProcedureSpecifications ;
        rdfs:label   "Reunión sobre admisión de licitadores"@es , "Tender admission meeting"@en ;
        rdfs:range   pproc:TenderMeeting .

pc:actualEndDate  a         owl:DatatypeProperty ;
        rdfs:isDefinedBy    pc: ;
        rdfs:label          "Fecha de finalización final"@es , "Actual end date"@en ;
        rdfs:subPropertyOf  dcterms:date .

pproc:remedyReason  a  owl:DatatypeProperty ;
        rdfs:domain  pproc:Remedy ;
        rdfs:label   "Causa del recurso"@es , "Remedy reason"@en ;
        rdfs:range   xsd:string .

pproc:TenderCommittee
        a                owl:Class ;
        rdfs:label       "Mesa de contratación"@es , "Tender committee"@en ;
        rdfs:subClassOf  pproc:Committee .

pproc:RegularOpen  a       skos:Concept , owl:NamedIndividual ;
        rdfs:label         "Abierto ordinario"@es , "Regular open"@en ;
        owl:sameAs         pc:Open ;
        skos:inScheme      pproc:ProcedureTypeScheme ;
        skos:topConceptOf  pproc:ProcedureTypeScheme .

pproc:TenderRequirements
        a             owl:Class ;
        rdfs:comment  "Clase que define los requisitos exigidos a las ofertas a presentar (e.g. plazo o documentación a presentar)."@es , "Class to define the tender requirements needed to submit a tender (e.g. tender document needs)."@en ;
        rdfs:label    "Requisitos para las ofertas"@es , "Tender requirements"@en .

pproc:SpecialAdministrativeRemedy
        a                owl:Class ;
        rdfs:label       "Recurso administrativo especial"@es , "Special administrative remedy"@en ;
        rdfs:subClassOf  pproc:Remedy .

pproc:contractAdditionalObligations
        a            owl:FunctionalProperty , owl:ObjectProperty ;
        rdfs:domain  pproc:ContractProcedureSpecifications ;
        rdfs:label   "Obligaciones accesorias del contrato"@es , "Contract additional obligations"@en ;
        rdfs:range   pproc:ContractAdditionalObligations .

pproc:ContractAdditionalObligations
        a             owl:Class ;
        rdfs:comment  "Clase que define las obligaciones accesorias de un contrato (e.g. garantías ó gastos de publicidad)."@es , "Class describing the additional obligations the contract needs (e.g. guarantees or advertisement costs)"@en ;
        rdfs:label    "Obligaciones accesorias del contrato"@es , "Contract additional obligations"@en .

pproc:AcceptedTender  a   owl:Class ;
        rdfs:comment      "Clase para definir las ofertas que se han admitido a licitación."@es , "Class describing the tenders accepted in the procurement public contract."@en ;
        rdfs:label        "Oferta admitida"@es , "Accepted tender"@en ;
        rdfs:subClassOf   pc:Tender ;
        owl:disjointWith  pproc:ExcludedTender .

pproc:AgreementContract
        a                owl:Class ;
        rdfs:comment     "Contrato de los conciertos con persona natural o jurídica que venga realizando prestaciones análogas a las que constituyen el servicio público de que se trate."@es , "Class describing the contract concerts with natural or legal person performing similar services at the public service in question."@en ;
        rdfs:label       "Concierto"@es , "Agreement contract"@en ;
        rdfs:subClassOf  pproc:PublicServicesManagementContract .

pproc:SuppliesContract
        a                owl:Class ;
        rdfs:comment     "Clase de los contratos cuyo objeto es la adquisición de suministros. Esta adquisición puede ser bien mediante compra, alquiler o arrendamiento financiero."@es , "Class describing contracts whose object is the acquisition of supplies."@en ;
        rdfs:label       "Contrato de suministros"@es , "Supplies contract"@en ;
        rdfs:subClassOf  pproc:Contract .

pproc:TechnicalInformation
        a                  skos:Concept , owl:NamedIndividual ;
        rdfs:label         "Información técnica"@es , "Technical information"@en ;
        skos:inScheme      pproc:InformationKindScheme ;
        skos:topConceptOf  pproc:InformationKindScheme .

pproc:recurrentRemedy
        a            owl:DatatypeProperty ;
        rdfs:domain  pproc:Remedy ;
        rdfs:label   "Recurso recurrente"@es , "Recurrent remedy"@en ;
        rdfs:range   xsd:string .

pproc:tenderPurpose  a  owl:DatatypeProperty ;
        rdfs:comment  "Indica, de manera textual, el propósito de la reunión de contratación (e.g. apertura de sobre A)"@es , "Indicates the purpose of the meeting (e.g. opening of first envelope)."@en ;
        rdfs:domain   pproc:TenderMeeting ;
        rdfs:label    "Propósito de la reunión"@es , "Tender purpose"@en ;
        rdfs:range    xsd:string .

pproc:minNumberOfOperators
        a            owl:FunctionalProperty , owl:DatatypeProperty ;
        rdfs:domain  pproc:FrameworkAgreement ;
        rdfs:label   "Número mínimo de participantes"@es , "Minimum number of operators"@en ;
        rdfs:range   xsd:nonNegativeInteger .

pproc:MixedContract  a   owl:Class ;
        rdfs:label       "Contrato mixto"@es , "Mixed contract"@en ;
        rdfs:subClassOf  pproc:Contract .

pproc:remedyResolution
        a            owl:DatatypeProperty ;
        rdfs:domain  pproc:Remedy ;
        rdfs:label   "Resolución del recurso"@es , "Remedy resolution"@en ;
        rdfs:range   xsd:string .

[ a       <http://www.w3.org/1999/xhtmlhtml> ;
  <http://www.w3.org/1999/xhtmlhead>
          [ a             <http://www.w3.org/1999/xhtmlmeta> ;
            <content>     "text/html; charset=utf-8"@en ;
            <http-equiv>  "Content-Type"@en
          ] ;
  <lang>  "en"@en
] .

ns:photo  a                     owl:ObjectProperty ;
        rdfs:comment            "This object property has been mapped"@en ;
        rdfs:isDefinedBy        <http://www.w3.org/2006/vcard/ns> ;
        rdfs:label              "photo"@en ;
        owl:equivalentProperty  ns:hasPhoto .

ns:hasPhoto  a                  owl:ObjectProperty ;
        rdfs:comment            "To specify an image or photograph information that annotates some aspect of the object"@en ;
        rdfs:isDefinedBy        <http://www.w3.org/2006/vcard/ns> ;
        rdfs:label              "has photo"@en ;
        owl:equivalentProperty  ns:photo .

ns:Friend  a              owl:Class ;
        rdfs:isDefinedBy  <http://www.w3.org/2006/vcard/ns> ;
        rdfs:label        "Friend"@en ;
        rdfs:subClassOf   ns:RelatedType .

ns:Colleague  a           owl:Class ;
        rdfs:isDefinedBy  <http://www.w3.org/2006/vcard/ns> ;
        rdfs:label        "Colleague"@en ;
        rdfs:subClassOf   ns:RelatedType .

ns:hasCountryName  a      owl:ObjectProperty ;
        rdfs:comment      "Used to support property parameters for the country name data property"@en ;
        rdfs:isDefinedBy  <http://www.w3.org/2006/vcard/ns> ;
        rdfs:label        "has country name"@en .

ns:Msg  a                 owl:Class ;
        rdfs:comment      "This class is deprecated"@en ;
        rdfs:isDefinedBy  <http://www.w3.org/2006/vcard/ns> ;
        rdfs:label        "Msg"@en ;
        rdfs:subClassOf   ns:TelephoneType ;
        owl:deprecated    true .

ns:Coresident  a          owl:Class ;
        rdfs:isDefinedBy  <http://www.w3.org/2006/vcard/ns> ;
        rdfs:label        "Coresident"@en ;
        rdfs:subClassOf   ns:RelatedType .

ns:n    a                       owl:ObjectProperty ;
        rdfs:comment            "This object property has been mapped"@en ;
        rdfs:isDefinedBy        <http://www.w3.org/2006/vcard/ns> ;
        rdfs:label              "name"@en ;
        owl:equivalentProperty  ns:hasName .

ns:hasAddress  a          owl:ObjectProperty ;
        rdfs:comment      "To specify the components of the delivery address for the object"@en ;
        rdfs:isDefinedBy  <http://www.w3.org/2006/vcard/ns> ;
        rdfs:label        "has address"@en ;
        rdfs:range        ns:Address .

ns:hasRegion  a           owl:ObjectProperty ;
        rdfs:comment      "Used to support property parameters for the region data property"@en ;
        rdfs:isDefinedBy  <http://www.w3.org/2006/vcard/ns> ;
        rdfs:label        "has region"@en .

ns:Neighbor  a            owl:Class ;
        rdfs:isDefinedBy  <http://www.w3.org/2006/vcard/ns> ;
        rdfs:label        "Neighbor"@en ;
        rdfs:subClassOf   ns:RelatedType .

ns:Coworker  a            owl:Class ;
        rdfs:isDefinedBy  <http://www.w3.org/2006/vcard/ns> ;
        rdfs:label        "Coworker"@en ;
        rdfs:subClassOf   ns:RelatedType .

ns:RelatedType  a         owl:Class ;
        rdfs:comment      "Used for relation type codes. The URI of the relation type code must be used as the value for the Relation Type."@en ;
        rdfs:isDefinedBy  <http://www.w3.org/2006/vcard/ns> ;
        rdfs:label        "Relation Type"@en .

ns:Me   a                 owl:Class ;
        rdfs:isDefinedBy  <http://www.w3.org/2006/vcard/ns> ;
        rdfs:label        "Me"@en ;
        rdfs:subClassOf   ns:RelatedType .

ns:None  a                owl:Class ;
        rdfs:isDefinedBy  <http://www.w3.org/2006/vcard/ns> ;
        rdfs:label        "None"@en ;
        rdfs:subClassOf   ns:Gender .

ns:hasUID  a              owl:ObjectProperty ;
        rdfs:comment      "To specify a value that represents a globally unique identifier corresponding to the object"@en ;
        rdfs:isDefinedBy  <http://www.w3.org/2006/vcard/ns> ;
        rdfs:label        "has uid"@en .

ns:Organization  a        owl:Class ;
        rdfs:comment      "An object representing an organization.  An organization is a single entity, and might represent a business or government, a department or division within a business or government, a club, an association, or the like.\n"@en ;
        rdfs:isDefinedBy  <http://www.w3.org/2006/vcard/ns> ;
        rdfs:label        "Organization"@en ;
        rdfs:subClassOf   ns:Kind .

<http://www.w3.org/2006/vcard/ns>
        a                owl:Ontology ;
        rdfs:comment     "Ontology for vCard based on RFC6350"@en ;
        rdfs:label       "Ontology for vCard"@en ;
        owl:versionInfo  "Final"@en .

ns:hasRelated  a          owl:ObjectProperty ;
        rdfs:comment      "To specify a relationship between another entity and the entity represented by this object"@en ;
        rdfs:isDefinedBy  <http://www.w3.org/2006/vcard/ns> ;
        rdfs:label        "has related"@en .

ns:Video  a               owl:Class ;
        rdfs:isDefinedBy  <http://www.w3.org/2006/vcard/ns> ;
        rdfs:label        "Video"@en ;
        rdfs:subClassOf   ns:TelephoneType .

ns:ISDN  a                owl:Class ;
        rdfs:comment      "This class is deprecated"@en ;
        rdfs:isDefinedBy  <http://www.w3.org/2006/vcard/ns> ;
        rdfs:label        "ISDN"@en ;
        rdfs:subClassOf   ns:Type ;
        owl:deprecated    true .

ns:X400  a                owl:Class ;
        rdfs:comment      "This class is deprecated"@en ;
        rdfs:isDefinedBy  <http://www.w3.org/2006/vcard/ns> ;
        rdfs:label        "X400"@en ;
        rdfs:subClassOf   ns:Type ;
        owl:deprecated    true .

ns:Label  a               owl:Class ;
        rdfs:comment      "This class is deprecated"@en ;
        rdfs:isDefinedBy  <http://www.w3.org/2006/vcard/ns> ;
        rdfs:label        "Label"@en ;
        rdfs:subClassOf   ns:Type ;
        owl:deprecated    true .

ns:post-office-box  a     owl:DatatypeProperty ;
        rdfs:comment      "This data property has been deprecated"@en ;
        rdfs:isDefinedBy  <http://www.w3.org/2006/vcard/ns> ;
        rdfs:label        "post office box"@en ;
        owl:deprecated    true .

ns:title  a               owl:DatatypeProperty ;
        rdfs:comment      "To specify the position or job of the object"@en ;
        rdfs:isDefinedBy  <http://www.w3.org/2006/vcard/ns> ;
        rdfs:label        "title"@en ;
        rdfs:range        xsd:string .

ns:VCard  a                  owl:Class ;
        rdfs:comment         "The vCard class is  equivalent to the new Kind class, which is the parent for the four explicit types of vCards (Individual, Organization, Location, Group)"@en ;
        rdfs:isDefinedBy     <http://www.w3.org/2006/vcard/ns> ;
        rdfs:label           "VCard"@en ;
        owl:equivalentClass  ns:Kind .

ns:Female  a              owl:Class ;
        rdfs:isDefinedBy  <http://www.w3.org/2006/vcard/ns> ;
        rdfs:label        "Female"@en ;
        rdfs:subClassOf   ns:Gender .

ns:hasMember  a           owl:ObjectProperty ;
        rdfs:comment      "To include a member in the group this object represents. (This property can only be used by Group individuals)"@en ;
        rdfs:domain       ns:Group ;
        rdfs:isDefinedBy  <http://www.w3.org/2006/vcard/ns> ;
        rdfs:label        "has member"@en ;
        rdfs:range        ns:Kind .

ns:key  a                       owl:ObjectProperty ;
        rdfs:comment            "This object property has been mapped"@en ;
        rdfs:isDefinedBy        <http://www.w3.org/2006/vcard/ns> ;
        rdfs:label              "key"@en ;
        owl:equivalentProperty  ns:hasKey .

ns:Location  a            owl:Class ;
        rdfs:comment      "An object representing a named geographical place"@en ;
        rdfs:isDefinedBy  <http://www.w3.org/2006/vcard/ns> ;
        rdfs:label        "Location"@en ;
        rdfs:subClassOf   ns:Kind ;
        owl:disjointWith  ns:Organization .

ns:rev  a                 owl:DatatypeProperty ;
        rdfs:comment      "To specify revision information about the object"@en ;
        rdfs:isDefinedBy  <http://www.w3.org/2006/vcard/ns> ;
        rdfs:label        "revision"@en ;
        rdfs:range        xsd:dateTime .

ns:Sweetheart  a          owl:Class ;
        rdfs:isDefinedBy  <http://www.w3.org/2006/vcard/ns> ;
        rdfs:label        "Sweetheart"@en ;
        rdfs:subClassOf   ns:RelatedType .

ns:logo  a                      owl:ObjectProperty ;
        rdfs:comment            "This object property has been mapped"@en ;
        rdfs:isDefinedBy        <http://www.w3.org/2006/vcard/ns> ;
        rdfs:label              "logo"@en ;
        owl:equivalentProperty  ns:hasLogo .

ns:Contact  a             owl:Class ;
        rdfs:isDefinedBy  <http://www.w3.org/2006/vcard/ns> ;
        rdfs:label        "Contact"@en ;
        rdfs:subClassOf   ns:RelatedType .

ns:language  a            owl:DatatypeProperty ;
        rdfs:comment      "To specify the language that may be used for contacting the object. May also be used as a property parameter."@en ;
        rdfs:isDefinedBy  <http://www.w3.org/2006/vcard/ns> ;
        rdfs:label        "language"@en .

ns:Cell  a                owl:Class ;
        rdfs:comment      "Also called mobile telephone"@en ;
        rdfs:isDefinedBy  <http://www.w3.org/2006/vcard/ns> ;
        rdfs:label        "Cell"@en ;
        rdfs:subClassOf   ns:TelephoneType .

ns:Acquaintance  a        owl:Class ;
        rdfs:isDefinedBy  <http://www.w3.org/2006/vcard/ns> ;
        rdfs:label        "Acquaintance"@en ;
        rdfs:subClassOf   ns:RelatedType .

ns:Intl  a                owl:Class ;
        rdfs:comment      "This class is deprecated"@en ;
        rdfs:isDefinedBy  <http://www.w3.org/2006/vcard/ns> ;
        rdfs:label        "Intl"@en ;
        rdfs:subClassOf   ns:Type ;
        owl:deprecated    true .

ns:Modem  a               owl:Class ;
        rdfs:comment      "This class is deprecated"@en ;
        rdfs:isDefinedBy  <http://www.w3.org/2006/vcard/ns> ;
        rdfs:label        "Modem"@en ;
        rdfs:subClassOf   ns:TelephoneType ;
        owl:deprecated    true .

ns:Emergency  a           owl:Class ;
        rdfs:isDefinedBy  <http://www.w3.org/2006/vcard/ns> ;
        rdfs:label        "Emergency"@en ;
        rdfs:subClassOf   ns:RelatedType .

ns:organization-name  a   owl:DatatypeProperty ;
        rdfs:comment      "To specify the organizational name associated with the object"@en ;
        rdfs:isDefinedBy  <http://www.w3.org/2006/vcard/ns> ;
        rdfs:label        "organization name"@en ;
        rdfs:range        xsd:string .

ns:hasSource  a           owl:ObjectProperty ;
        rdfs:comment      "To identify the source of directory information of the object"@en ;
        rdfs:isDefinedBy  <http://www.w3.org/2006/vcard/ns> ;
        rdfs:label        "has source"@en .

ns:label  a               owl:DatatypeProperty ;
        rdfs:comment      "This data property has been deprecated"@en ;
        rdfs:isDefinedBy  <http://www.w3.org/2006/vcard/ns> ;
        rdfs:label        "label"@en ;
        owl:deprecated    true .

ns:geo  a                       owl:ObjectProperty ;
        rdfs:comment            "This object property has been mapped"@en ;
        rdfs:isDefinedBy        <http://www.w3.org/2006/vcard/ns> ;
        rdfs:label              "geo"@en ;
        owl:equivalentProperty  ns:hasGeo .

ns:hasStreetAddress  a    owl:ObjectProperty ;
        rdfs:comment      "Used to support property parameters for the street address data property"@en ;
        rdfs:isDefinedBy  <http://www.w3.org/2006/vcard/ns> ;
        rdfs:label        "has street address"@en .

ns:hasGeo  a              owl:ObjectProperty ;
        rdfs:comment      "To specify information related to the global positioning of the object. May also be used as a property parameter."@en ;
        rdfs:isDefinedBy  <http://www.w3.org/2006/vcard/ns> ;
        rdfs:label        "has geo"@en .

ns:Internet  a            owl:Class ;
        rdfs:comment      "This class is deprecated"@en ;
        rdfs:isDefinedBy  <http://www.w3.org/2006/vcard/ns> ;
        rdfs:label        "Internet"@en ;
        rdfs:subClassOf   ns:Type ;
        owl:deprecated    true .

ns:hasGender  a           owl:ObjectProperty ;
        rdfs:comment      "To specify  the sex or gender identity of the object. URIs are recommended to enable interoperable sex and gender codes to be used."@en ;
        rdfs:isDefinedBy  <http://www.w3.org/2006/vcard/ns> ;
        rdfs:label        "has gender"@en .

ns:sort-string  a         owl:DatatypeProperty ;
        rdfs:comment      "To specify the string to be used for national-language-specific sorting. Used as a property parameter only."@en ;
        rdfs:isDefinedBy  <http://www.w3.org/2006/vcard/ns> ;
        rdfs:label        "sort as"@en ;
        rdfs:range        xsd:string .

ns:Other  a               owl:Class ;
        rdfs:isDefinedBy  <http://www.w3.org/2006/vcard/ns> ;
        rdfs:label        "Other"@en ;
        rdfs:subClassOf   ns:Gender .

ns:Spouse  a              owl:Class ;
        rdfs:isDefinedBy  <http://www.w3.org/2006/vcard/ns> ;
        rdfs:label        "Spouse"@en ;
        rdfs:subClassOf   ns:RelatedType .

ns:hasURL  a                    owl:ObjectProperty ;
        rdfs:comment            "To specify a uniform resource locator associated with the object"@en ;
        rdfs:isDefinedBy        <http://www.w3.org/2006/vcard/ns> ;
        rdfs:label              "has url"@en ;
        owl:equivalentProperty  ns:url .

ns:Parcel  a              owl:Class ;
        rdfs:comment      "This class is deprecated"@en ;
        rdfs:isDefinedBy  <http://www.w3.org/2006/vcard/ns> ;
        rdfs:label        "Parcel"@en ;
        rdfs:subClassOf   ns:Type ;
        owl:deprecated    true .

ns:family-name  a         owl:DatatypeProperty ;
        rdfs:comment      "The family name associated with the object"@en ;
        rdfs:isDefinedBy  <http://www.w3.org/2006/vcard/ns> ;
        rdfs:label        "family name"@en ;
        rdfs:range        xsd:string .

ns:Postal  a              owl:Class ;
        rdfs:comment      "This class is deprecated"@en ;
        rdfs:isDefinedBy  <http://www.w3.org/2006/vcard/ns> ;
        rdfs:label        "Postal"@en ;
        rdfs:subClassOf   ns:Type ;
        owl:deprecated    true .

ns:locality  a            owl:DatatypeProperty ;
        rdfs:comment      "The locality (e.g. city or town) associated with the address of the object"@en ;
        rdfs:isDefinedBy  <http://www.w3.org/2006/vcard/ns> ;
        rdfs:label        "locality"@en ;
        rdfs:range        xsd:string .

ns:category  a            owl:DatatypeProperty ;
        rdfs:comment      "The category information about the object, also known as tags"@en ;
        rdfs:isDefinedBy  <http://www.w3.org/2006/vcard/ns> ;
        rdfs:label        "category"@en ;
        rdfs:range        xsd:string .

ns:tel  a                       owl:ObjectProperty ;
        rdfs:comment            "This object property has been mapped"@en ;
        rdfs:isDefinedBy        <http://www.w3.org/2006/vcard/ns> ;
        rdfs:label              "telephone"@en ;
        owl:equivalentProperty  ns:hasTelephone .

ns:latitude  a            owl:DatatypeProperty ;
        rdfs:comment      "This data property has been deprecated. See hasGeo"@en ;
        rdfs:isDefinedBy  <http://www.w3.org/2006/vcard/ns> ;
        rdfs:label        "latitude"@en ;
        owl:deprecated    true .

ns:Work  a                owl:Class ;
        rdfs:comment      "This implies that the property is related to an individual's work place"@en ;
        rdfs:isDefinedBy  <http://www.w3.org/2006/vcard/ns> ;
        rdfs:label        "Work"@en ;
        rdfs:subClassOf   ns:Type .

ns:hasPostalCode  a       owl:ObjectProperty ;
        rdfs:comment      "Used to support property parameters for the postal code data property"@en ;
        rdfs:isDefinedBy  <http://www.w3.org/2006/vcard/ns> ;
        rdfs:label        "has postal code"@en .

ns:Sibling  a             owl:Class ;
        rdfs:isDefinedBy  <http://www.w3.org/2006/vcard/ns> ;
        rdfs:label        "Sibling"@en ;
        rdfs:subClassOf   ns:RelatedType .

ns:bday  a                owl:DatatypeProperty ;
        rdfs:comment      "To specify the birth date of the object"@en ;
        rdfs:isDefinedBy  <http://www.w3.org/2006/vcard/ns> ;
        rdfs:label        "birth date"@en ;
        rdfs:range        [ a            rdfs:Datatype ;
                            owl:unionOf  ( xsd:dateTime xsd:dateTimeStamp xsd:gYear )
                          ] .

ns:Car  a                 owl:Class ;
        rdfs:comment      "This class is deprecated"@en ;
        rdfs:isDefinedBy  <http://www.w3.org/2006/vcard/ns> ;
        rdfs:label        "Car"@en ;
        rdfs:subClassOf   ns:TelephoneType ;
        owl:deprecated    true .

ns:hasLanguage  a         owl:ObjectProperty ;
        rdfs:comment      "Used to support property parameters for the language data property"@en ;
        rdfs:isDefinedBy  <http://www.w3.org/2006/vcard/ns> ;
        rdfs:label        "has language"@en .

ns:Child  a               owl:Class ;
        rdfs:isDefinedBy  <http://www.w3.org/2006/vcard/ns> ;
        rdfs:label        "Child"@en ;
        rdfs:subClassOf   ns:RelatedType .

ns:Email  a               owl:Class ;
        rdfs:comment      "To specify the electronic mail address for communication with the object the vCard represents. Use the hasEmail object property."@en ;
        rdfs:isDefinedBy  <http://www.w3.org/2006/vcard/ns> ;
        rdfs:label        "Email"@en ;
        owl:deprecated    true .

ns:Male  a                owl:Class ;
        rdfs:isDefinedBy  <http://www.w3.org/2006/vcard/ns> ;
        rdfs:label        "Male"@en ;
        rdfs:subClassOf   ns:Gender .

ns:adr  a                       owl:ObjectProperty ;
        rdfs:comment            "This object property has been mapped"@en ;
        rdfs:isDefinedBy        <http://www.w3.org/2006/vcard/ns> ;
        rdfs:label              "address"@en ;
        owl:equivalentProperty  ns:hasAddress .

ns:hasFN  a               owl:ObjectProperty ;
        rdfs:comment      "Used to support property parameters for the formatted name data property"@en ;
        rdfs:isDefinedBy  <http://www.w3.org/2006/vcard/ns> ;
        rdfs:label        "has formatted name"@en .

ns:tz   a                 owl:DatatypeProperty ;
        rdfs:comment      "To indicate time zone information that is specific to the object. May also be used as a property parameter."@en ;
        rdfs:isDefinedBy  <http://www.w3.org/2006/vcard/ns> ;
        rdfs:label        "time zone"@en ;
        rdfs:range        xsd:string .

ns:Pref  a                owl:Class ;
        rdfs:comment      "This class is deprecated"@en ;
        rdfs:isDefinedBy  <http://www.w3.org/2006/vcard/ns> ;
        rdfs:label        "Pref"@en ;
        rdfs:subClassOf   ns:Type ;
        owl:deprecated    true .

ns:Text  a                owl:Class ;
        rdfs:comment      "Also called sms telephone"@en ;
        rdfs:isDefinedBy  <http://www.w3.org/2006/vcard/ns> ;
        rdfs:label        "Text"@en ;
        rdfs:subClassOf   ns:TelephoneType .

ns:Group  a                  owl:Class ;
        rdfs:comment         "Object representing a group of persons or entities.  A group object will usually contain hasMember properties to specify the members of the group."@en ;
        rdfs:isDefinedBy     <http://www.w3.org/2006/vcard/ns> ;
        rdfs:label           "Group"@en ;
        rdfs:subClassOf      ns:Kind ;
        owl:disjointWith     ns:Organization , ns:Location , ns:Individual ;
        owl:equivalentClass  [ a                   owl:Class ;
                               owl:intersectionOf  ( [ a                   owl:Restriction ;
                                                       owl:onProperty      ns:hasMember ;
                                                       owl:someValuesFrom  ns:Kind
                                                     ]
                                                     [ a                            owl:Restriction ;
                                                       owl:minQualifiedCardinality  "1"^^xsd:nonNegativeInteger ;
                                                       owl:onClass                  ns:Kind ;
                                                       owl:onProperty               ns:hasMember
                                                     ]
                                                   )
                             ] .

ns:hasTelephone  a              owl:ObjectProperty ;
        rdfs:comment            "To specify the telephone number for telephony communication with the object"@en ;
        rdfs:isDefinedBy        <http://www.w3.org/2006/vcard/ns> ;
        rdfs:label              "has telephone"@en ;
        owl:equivalentProperty  ns:tel .

ns:hasOrganizationName
        a                 owl:ObjectProperty ;
        rdfs:comment      "Used to support property parameters for the organization name data property"@en ;
        rdfs:isDefinedBy  <http://www.w3.org/2006/vcard/ns> ;
        rdfs:label        "has organization name"@en .

ns:Kin  a                 owl:Class ;
        rdfs:isDefinedBy  <http://www.w3.org/2006/vcard/ns> ;
        rdfs:label        "Kin"@en ;
        rdfs:subClassOf   ns:RelatedType .

ns:Muse  a                owl:Class ;
        rdfs:isDefinedBy  <http://www.w3.org/2006/vcard/ns> ;
        rdfs:label        "Muse"@en ;
        rdfs:subClassOf   ns:RelatedType .

ns:TelephoneType  a       owl:Class ;
        rdfs:comment      "Used for telephone type codes. The URI of the telephone type code must be used as the value for the Telephone Type."@en ;
        rdfs:isDefinedBy  <http://www.w3.org/2006/vcard/ns> ;
        rdfs:label        "Phone"@en .

ns:hasGivenName  a        owl:ObjectProperty ;
        rdfs:comment      "Used to support property parameters for the given name data property"@en ;
        rdfs:isDefinedBy  <http://www.w3.org/2006/vcard/ns> ;
        rdfs:label        "has given name"@en .

ns:region  a              owl:DatatypeProperty ;
        rdfs:comment      "The region (e.g. state or province) associated with the address of the object"@en ;
        rdfs:isDefinedBy  <http://www.w3.org/2006/vcard/ns> ;
        rdfs:label        "region"@en ;
        rdfs:range        xsd:string .

ns:Kind  a                   owl:Class ;
        rdfs:comment         "The parent class for all objects"@en ;
        rdfs:isDefinedBy     <http://www.w3.org/2006/vcard/ns> ;
        rdfs:label           "Kind"@en ;
        owl:equivalentClass  ns:VCard ;
        owl:equivalentClass  [ a                            owl:Restriction ;
                               owl:minQualifiedCardinality  "1"^^xsd:nonNegativeInteger ;
                               owl:onDataRange              xsd:string ;
                               owl:onProperty               ns:fn
                             ] .

ns:nickname  a            owl:DatatypeProperty ;
        rdfs:comment      "The nick name associated with the object"@en ;
        rdfs:isDefinedBy  <http://www.w3.org/2006/vcard/ns> ;
        rdfs:label        "nickname"@en ;
        rdfs:range        xsd:string .

ns:given-name  a          owl:DatatypeProperty ;
        rdfs:comment      "The given name associated with the object"@en ;
        rdfs:isDefinedBy  <http://www.w3.org/2006/vcard/ns> ;
        rdfs:label        "given name"@en ;
        rdfs:range        xsd:string .

ns:Agent  a               owl:Class ;
        rdfs:isDefinedBy  <http://www.w3.org/2006/vcard/ns> ;
        rdfs:label        "Agent"@en ;
        rdfs:subClassOf   ns:RelatedType .

ns:hasTitle  a            owl:ObjectProperty ;
        rdfs:comment      "Used to support property parameters for the title data property"@en ;
        rdfs:isDefinedBy  <http://www.w3.org/2006/vcard/ns> ;
        rdfs:label        "has title"@en .

ns:hasHonorificPrefix
        a                 owl:ObjectProperty ;
        rdfs:comment      "Used to support property parameters for the honorific prefix data property"@en ;
        rdfs:isDefinedBy  <http://www.w3.org/2006/vcard/ns> ;
        rdfs:label        "has honorific prefix"@en .

ns:BBS  a                 owl:Class ;
        rdfs:comment      "This class is deprecated"@en ;
        rdfs:isDefinedBy  <http://www.w3.org/2006/vcard/ns> ;
        rdfs:label        "BBS"@en ;
        rdfs:subClassOf   ns:TelephoneType ;
        owl:deprecated    true .

ns:organization-unit  a     owl:DatatypeProperty ;
        rdfs:comment        "To specify the organizational unit name associated with the object"@en ;
        rdfs:isDefinedBy    <http://www.w3.org/2006/vcard/ns> ;
        rdfs:label          "organizational unit name"@en ;
        rdfs:range          xsd:string ;
        rdfs:subPropertyOf  ns:organization-name .

ns:Date  a                owl:Class ;
        rdfs:isDefinedBy  <http://www.w3.org/2006/vcard/ns> ;
        rdfs:label        "Date"@en ;
        rdfs:subClassOf   ns:RelatedType .

ns:hasFamilyName  a       owl:ObjectProperty ;
        rdfs:comment      "Used to support property parameters for the family name data property"@en ;
        rdfs:isDefinedBy  <http://www.w3.org/2006/vcard/ns> ;
        rdfs:label        "has family name"@en .

ns:sound  a                     owl:ObjectProperty ;
        rdfs:comment            "This object property has been mapped"@en ;
        rdfs:isDefinedBy        <http://www.w3.org/2006/vcard/ns> ;
        rdfs:label              "sound"@en ;
        owl:equivalentProperty  ns:hasSound .

ns:hasCategory  a         owl:ObjectProperty ;
        rdfs:comment      "Used to support property parameters for the category data property"@en ;
        rdfs:isDefinedBy  <http://www.w3.org/2006/vcard/ns> ;
        rdfs:label        "has category"@en .

ns:hasLocality  a         owl:ObjectProperty ;
        rdfs:comment      "Used to support property parameters for the locality data property"@en ;
        rdfs:isDefinedBy  <http://www.w3.org/2006/vcard/ns> ;
        rdfs:label        "has locality"@en .

ns:hasSound  a                  owl:ObjectProperty ;
        rdfs:comment            "To specify a digital sound content information that annotates some aspect of the object"@en ;
        rdfs:isDefinedBy        <http://www.w3.org/2006/vcard/ns> ;
        rdfs:label              "has sound"@en ;
        owl:equivalentProperty  ns:sound .

ns:prodid  a              owl:DatatypeProperty ;
        rdfs:comment      "To specify the identifier for the product that created the object"@en ;
        rdfs:isDefinedBy  <http://www.w3.org/2006/vcard/ns> ;
        rdfs:label        "product id"@en ;
        rdfs:range        xsd:string .

ns:Pager  a               owl:Class ;
        rdfs:isDefinedBy  <http://www.w3.org/2006/vcard/ns> ;
        rdfs:label        "Pager"@en ;
        rdfs:subClassOf   ns:TelephoneType .

ns:hasKey  a                    owl:ObjectProperty ;
        rdfs:comment            "To specify a public key or authentication certificate associated with the object"@en ;
        rdfs:isDefinedBy        <http://www.w3.org/2006/vcard/ns> ;
        rdfs:label              "has key"@en ;
        owl:equivalentProperty  ns:key .

ns:fn   a                 owl:DatatypeProperty ;
        rdfs:comment      "The formatted text corresponding to the name of the object"@en ;
        rdfs:isDefinedBy  <http://www.w3.org/2006/vcard/ns> ;
        rdfs:label        "formatted name"@en ;
        rdfs:range        xsd:string .

ns:Met  a                 owl:Class ;
        rdfs:isDefinedBy  <http://www.w3.org/2006/vcard/ns> ;
        rdfs:label        "Met"@en ;
        rdfs:subClassOf   ns:RelatedType .

ns:email  a                     owl:ObjectProperty ;
        rdfs:comment            "This object property has been mapped"@en ;
        rdfs:isDefinedBy        <http://www.w3.org/2006/vcard/ns> ;
        rdfs:label              "email"@en ;
        owl:equivalentProperty  ns:hasEmail .

ns:hasEmail  a            owl:ObjectProperty ;
        rdfs:comment      "To specify the electronic mail address for communication with the object"@en ;
        rdfs:isDefinedBy  <http://www.w3.org/2006/vcard/ns> ;
        rdfs:label        "has email"@en ;
        rdfs:range        ns:Email .

ns:postal-code  a         owl:DatatypeProperty ;
        rdfs:comment      "The postal code associated with the address of the object"@en ;
        rdfs:isDefinedBy  <http://www.w3.org/2006/vcard/ns> ;
        rdfs:label        "postal code"@en ;
        rdfs:range        xsd:string .

ns:hasInstantMessage  a   owl:ObjectProperty ;
        rdfs:comment      "To specify the instant messaging and presence protocol communications with the object. (Was called IMPP in RFC6350)"@en ;
        rdfs:isDefinedBy  <http://www.w3.org/2006/vcard/ns> ;
        rdfs:label        "has messaging"@en .

ns:Gender  a              owl:Class ;
        rdfs:comment      "Used for gender codes. The URI of the gender code must be used as the value for Gender."@en ;
        rdfs:isDefinedBy  <http://www.w3.org/2006/vcard/ns> ;
        rdfs:label        "Gender"@en .

ns:Voice  a               owl:Class ;
        rdfs:isDefinedBy  <http://www.w3.org/2006/vcard/ns> ;
        rdfs:label        "Voice"@en ;
        rdfs:subClassOf   ns:TelephoneType .

ns:note  a                owl:DatatypeProperty ;
        rdfs:comment      "A note associated with the object"@en ;
        rdfs:isDefinedBy  <http://www.w3.org/2006/vcard/ns> ;
        rdfs:label        "note"@en ;
        rdfs:range        xsd:string .

ns:PCS  a                 owl:Class ;
        rdfs:comment      "This class is deprecated"@en ;
        rdfs:isDefinedBy  <http://www.w3.org/2006/vcard/ns> ;
        rdfs:label        "PCS"@en ;
        rdfs:subClassOf   ns:TelephoneType ;
        owl:deprecated    true .

ns:honorific-prefix  a    owl:DatatypeProperty ;
        rdfs:comment      "The honorific prefix of the name associated with the object"@en ;
        rdfs:isDefinedBy  <http://www.w3.org/2006/vcard/ns> ;
        rdfs:label        "honorific prefix"@en ;
        rdfs:range        xsd:string .

ns:Parent  a              owl:Class ;
        rdfs:isDefinedBy  <http://www.w3.org/2006/vcard/ns> ;
        rdfs:label        "Parent"@en ;
        rdfs:subClassOf   ns:RelatedType .

ns:street-address  a      owl:DatatypeProperty ;
        rdfs:comment      "The street address associated with the address of the object"@en ;
        rdfs:isDefinedBy  <http://www.w3.org/2006/vcard/ns> ;
        rdfs:label        "street address"@en ;
        rdfs:range        xsd:string .

ns:mailer  a              owl:DatatypeProperty ;
        rdfs:comment      "This data property has been deprecated"@en ;
        rdfs:isDefinedBy  <http://www.w3.org/2006/vcard/ns> ;
        rdfs:label        "mailer"@en ;
        owl:deprecated    true .

ns:Tel  a                 owl:Class ;
        rdfs:comment      "This class is deprecated. Use the hasTelephone object property."@en ;
        rdfs:isDefinedBy  <http://www.w3.org/2006/vcard/ns> ;
        rdfs:label        "Tel"@en ;
        owl:deprecated    true .

ns:hasNote  a             owl:ObjectProperty ;
        rdfs:comment      "Used to support property parameters for the note data property"@en ;
        rdfs:isDefinedBy  <http://www.w3.org/2006/vcard/ns> ;
        rdfs:label        "has note"@en .

ns:Individual  a          owl:Class ;
        rdfs:comment      "An object representing a single person or entity"@en ;
        rdfs:isDefinedBy  <http://www.w3.org/2006/vcard/ns> ;
        rdfs:label        "Individual"@en ;
        rdfs:subClassOf   ns:Kind ;
        owl:disjointWith  ns:Organization , ns:Location .

ns:hasAdditionalName  a   owl:ObjectProperty ;
        rdfs:comment      "Used to support property parameters for the additional name data property"@en ;
        rdfs:isDefinedBy  <http://www.w3.org/2006/vcard/ns> ;
        rdfs:label        "has additional name"@en .

ns:Unknown  a             owl:Class ;
        rdfs:isDefinedBy  <http://www.w3.org/2006/vcard/ns> ;
        rdfs:label        "Unknown"@en ;
        rdfs:subClassOf   ns:Gender .

ns:agent  a               owl:ObjectProperty ;
        rdfs:comment      "This object property has been deprecated"@en ;
        rdfs:isDefinedBy  <http://www.w3.org/2006/vcard/ns> ;
        rdfs:label        "agent"@en ;
        owl:deprecated    true .

ns:hasLogo  a                   owl:ObjectProperty ;
        rdfs:comment            "To specify a graphic image of a logo associated with the object "@en ;
        rdfs:isDefinedBy        <http://www.w3.org/2006/vcard/ns> ;
        rdfs:label              "has logo"@en ;
        owl:equivalentProperty  ns:logo .

ns:country-name  a        owl:DatatypeProperty ;
        rdfs:comment      "The country name associated with the address of the object"@en ;
        rdfs:isDefinedBy  <http://www.w3.org/2006/vcard/ns> ;
        rdfs:label        "country name"@en ;
        rdfs:range        xsd:string .

ns:hasHonorificSuffix
        a                 owl:ObjectProperty ;
        rdfs:comment      "Used to support property parameters for the honorific suffix data property"@en ;
        rdfs:isDefinedBy  <http://www.w3.org/2006/vcard/ns> ;
        rdfs:label        "has honorific suffix"@en .

ns:hasNickname  a         owl:ObjectProperty ;
        rdfs:comment      "Used to support property parameters for the nickname data property"@en ;
        rdfs:isDefinedBy  <http://www.w3.org/2006/vcard/ns> ;
        rdfs:label        "has nickname"@en ;
        rdfs:seeAlso      ns:nickname .

ns:Type  a                owl:Class ;
        rdfs:comment      "Used for type codes. The URI of the type code must be used as the value for Type."@en ;
        rdfs:isDefinedBy  <http://www.w3.org/2006/vcard/ns> ;
        rdfs:label        "Type"@en .

ns:Fax  a                 owl:Class ;
        rdfs:isDefinedBy  <http://www.w3.org/2006/vcard/ns> ;
        rdfs:label        "Fax"@en ;
        rdfs:subClassOf   ns:TelephoneType .

ns:extended-address  a    owl:DatatypeProperty ;
        rdfs:comment      "This data property has been deprecated"@en ;
        rdfs:isDefinedBy  <http://www.w3.org/2006/vcard/ns> ;
        rdfs:label        "extended address"@en ;
        owl:deprecated    true .

ns:TextPhone  a           owl:Class ;
        rdfs:isDefinedBy  <http://www.w3.org/2006/vcard/ns> ;
        rdfs:label        "Text phone"@en ;
        rdfs:subClassOf   ns:TelephoneType .

ns:hasName  a                   owl:ObjectProperty ;
        rdfs:comment            "To specify the components of the name of the object"@en ;
        rdfs:isDefinedBy        <http://www.w3.org/2006/vcard/ns> ;
        rdfs:label              "has name"@en ;
        rdfs:range              ns:Name ;
        owl:equivalentProperty  ns:n .

ns:role  a                owl:DatatypeProperty ;
        rdfs:comment      "To specify the function or part played in a particular situation by the object"@en ;
        rdfs:isDefinedBy  <http://www.w3.org/2006/vcard/ns> ;
        rdfs:label        "role"@en ;
        rdfs:range        xsd:string .

ns:hasCalendarLink  a     owl:ObjectProperty ;
        rdfs:comment      "To specify the calendar associated with the object. (Was called CALURI in RFC6350)"@en ;
        rdfs:isDefinedBy  <http://www.w3.org/2006/vcard/ns> ;
        rdfs:label        "has calendar link"@en .

ns:value  a               owl:DatatypeProperty ;
        rdfs:comment      "Used to indicate the literal value of a data property that requires property parameters"@en ;
        rdfs:isDefinedBy  <http://www.w3.org/2006/vcard/ns> ;
        rdfs:label        "value"@en .

ns:longitude  a           owl:DatatypeProperty ;
        rdfs:comment      "This data property has been deprecated. See hasGeo"@en ;
        rdfs:isDefinedBy  <http://www.w3.org/2006/vcard/ns> ;
        rdfs:label        "longitude"@en ;
        owl:deprecated    true .

ns:hasValue  a            owl:ObjectProperty ;
        rdfs:comment      "Used to indicate the resource value of an object property that requires property parameters"@en ;
        rdfs:isDefinedBy  <http://www.w3.org/2006/vcard/ns> ;
        rdfs:label        "has value"@en .

ns:Dom  a                 owl:Class ;
        rdfs:comment      "This class is deprecated"@en ;
        rdfs:isDefinedBy  <http://www.w3.org/2006/vcard/ns> ;
        rdfs:label        "Dom"@en ;
        rdfs:subClassOf   ns:Type ;
        owl:deprecated    true .

ns:anniversary  a         owl:DatatypeProperty ;
        rdfs:comment      "The date of marriage, or equivalent, of the object"@en ;
        rdfs:isDefinedBy  <http://www.w3.org/2006/vcard/ns> ;
        rdfs:label        "anniversary"@en ;
        rdfs:range        [ a            rdfs:Datatype ;
                            owl:unionOf  ( xsd:dateTime xsd:gYear )
                          ] .

ns:Home  a                owl:Class ;
        rdfs:comment      "This implies that the property is related to an individual's personal life"@en ;
        rdfs:isDefinedBy  <http://www.w3.org/2006/vcard/ns> ;
        rdfs:label        "Home"@en ;
        rdfs:subClassOf   ns:Type .

ns:Crush  a               owl:Class ;
        rdfs:isDefinedBy  <http://www.w3.org/2006/vcard/ns> ;
        rdfs:label        "Crush"@en ;
        rdfs:subClassOf   ns:RelatedType .

ns:hasOrganizationUnit
        a                 owl:ObjectProperty ;
        rdfs:comment      "Used to support property parameters for the organization unit name data property"@en ;
        rdfs:isDefinedBy  <http://www.w3.org/2006/vcard/ns> ;
        rdfs:label        "has organization unit name"@en .

ns:honorific-suffix  a    owl:DatatypeProperty ;
        rdfs:comment      "The honorific suffix of the name associated with the object"@en ;
        rdfs:isDefinedBy  <http://www.w3.org/2006/vcard/ns> ;
        rdfs:label        "honorific suffix"@en ;
        rdfs:range        xsd:string .

ns:class  a               owl:DatatypeProperty ;
        rdfs:comment      "This data property has been deprecated"@en ;
        rdfs:isDefinedBy  <http://www.w3.org/2006/vcard/ns> ;
        rdfs:label        "class"@en ;
        owl:deprecated    true .

ns:org  a                       owl:ObjectProperty ;
        rdfs:comment            "This object property has been mapped. Use the organization-name data property."@en ;
        rdfs:isDefinedBy        <http://www.w3.org/2006/vcard/ns> ;
        rdfs:label              "organization"@en ;
        owl:equivalentProperty  ns:organization-name .

ns:additional-name  a     owl:DatatypeProperty ;
        rdfs:comment      "The additional name associated with the object"@en ;
        rdfs:isDefinedBy  <http://www.w3.org/2006/vcard/ns> ;
        rdfs:label        "additional name"@en ;
        rdfs:range        xsd:string .

ns:hasRole  a             owl:ObjectProperty ;
        rdfs:comment      "Used to support property parameters for the role data property"@en ;
        rdfs:isDefinedBy  <http://www.w3.org/2006/vcard/ns> ;
        rdfs:label        "has role"@en .

ns:Address  a                owl:Class ;
        rdfs:comment         "To specify the components of the delivery address for the  object"@en ;
        rdfs:isDefinedBy     <http://www.w3.org/2006/vcard/ns> ;
        rdfs:label           "Address"@en ;
        owl:equivalentClass  [ a            owl:Class ;
                               owl:unionOf  ( [ a                   owl:Class ;
                                                owl:intersectionOf  ( [ a                   owl:Restriction ;
                                                                        owl:onProperty      ns:country-name ;
                                                                        owl:someValuesFrom  xsd:string
                                                                      ]
                                                                      [ a                   owl:Restriction ;
                                                                        owl:maxCardinality  "1"^^xsd:nonNegativeInteger ;
                                                                        owl:onProperty      ns:country-name
                                                                      ]
                                                                    )
                                              ]
                                              [ a                   owl:Class ;
                                                owl:intersectionOf  ( [ a                   owl:Restriction ;
                                                                        owl:onProperty      ns:locality ;
                                                                        owl:someValuesFrom  xsd:string
                                                                      ]
                                                                      [ a                   owl:Restriction ;
                                                                        owl:maxCardinality  "1"^^xsd:nonNegativeInteger ;
                                                                        owl:onProperty      ns:locality
                                                                      ]
                                                                    )
                                              ]
                                              [ a                   owl:Class ;
                                                owl:intersectionOf  ( [ a                   owl:Restriction ;
                                                                        owl:onProperty      ns:postal-code ;
                                                                        owl:someValuesFrom  xsd:string
                                                                      ]
                                                                      [ a                   owl:Restriction ;
                                                                        owl:maxCardinality  "1"^^xsd:nonNegativeInteger ;
                                                                        owl:onProperty      ns:postal-code
                                                                      ]
                                                                    )
                                              ]
                                              [ a                   owl:Class ;
                                                owl:intersectionOf  ( [ a                   owl:Restriction ;
                                                                        owl:onProperty      ns:region ;
                                                                        owl:someValuesFrom  xsd:string
                                                                      ]
                                                                      [ a                   owl:Restriction ;
                                                                        owl:maxCardinality  "1"^^xsd:nonNegativeInteger ;
                                                                        owl:onProperty      ns:region
                                                                      ]
                                                                    )
                                              ]
                                              [ a                   owl:Class ;
                                                owl:intersectionOf  ( [ a                   owl:Restriction ;
                                                                        owl:onProperty      ns:street-address ;
                                                                        owl:someValuesFrom  xsd:string
                                                                      ]
                                                                      [ a                   owl:Restriction ;
                                                                        owl:maxCardinality  "1"^^xsd:nonNegativeInteger ;
                                                                        owl:onProperty      ns:street-address
                                                                      ]
                                                                    )
                                              ]
                                            )
                             ] .

ns:url  a                       owl:ObjectProperty ;
        rdfs:comment            "This object property has been mapped"@en ;
        rdfs:isDefinedBy        <http://www.w3.org/2006/vcard/ns> ;
        rdfs:label              "url"@en ;
        owl:equivalentProperty  ns:hasURL .

ns:Name  a                   owl:Class ;
        rdfs:comment         "To specify the components of the name of the object"@en ;
        rdfs:isDefinedBy     <http://www.w3.org/2006/vcard/ns> ;
        rdfs:label           "Name"@en ;
        owl:equivalentClass  [ a            owl:Class ;
                               owl:unionOf  ( [ a                   owl:Class ;
                                                owl:intersectionOf  ( [ a                   owl:Restriction ;
                                                                        owl:onProperty      ns:additional-name ;
                                                                        owl:someValuesFrom  xsd:string
                                                                      ]
                                                                      [ a                   owl:Restriction ;
                                                                        owl:minCardinality  "0"^^xsd:nonNegativeInteger ;
                                                                        owl:onProperty      ns:additional-name
                                                                      ]
                                                                    )
                                              ]
                                              [ a                   owl:Class ;
                                                owl:intersectionOf  ( [ a                   owl:Restriction ;
                                                                        owl:onProperty      ns:family-name ;
                                                                        owl:someValuesFrom  xsd:string
                                                                      ]
                                                                      [ a                   owl:Restriction ;
                                                                        owl:maxCardinality  "1"^^xsd:nonNegativeInteger ;
                                                                        owl:onProperty      ns:family-name
                                                                      ]
                                                                    )
                                              ]
                                              [ a                   owl:Class ;
                                                owl:intersectionOf  ( [ a                   owl:Restriction ;
                                                                        owl:onProperty      ns:given-name ;
                                                                        owl:someValuesFrom  xsd:string
                                                                      ]
                                                                      [ a                   owl:Restriction ;
                                                                        owl:maxCardinality  "1"^^xsd:nonNegativeInteger ;
                                                                        owl:onProperty      ns:given-name
                                                                      ]
                                                                    )
                                              ]
                                              [ a                   owl:Class ;
                                                owl:intersectionOf  ( [ a                   owl:Restriction ;
                                                                        owl:onProperty      ns:honorific-prefix ;
                                                                        owl:someValuesFrom  xsd:string
                                                                      ]
                                                                      [ a                   owl:Restriction ;
                                                                        owl:minCardinality  "0"^^xsd:nonNegativeInteger ;
                                                                        owl:onProperty      ns:honorific-prefix
                                                                      ]
                                                                    )
                                              ]
                                              [ a                   owl:Class ;
                                                owl:intersectionOf  ( [ a                   owl:Restriction ;
                                                                        owl:onProperty      ns:honorific-suffix ;
                                                                        owl:someValuesFrom  xsd:string
                                                                      ]
                                                                      [ a                   owl:Restriction ;
                                                                        owl:minCardinality  "0"^^xsd:nonNegativeInteger ;
                                                                        owl:onProperty      ns:honorific-suffix
                                                                      ]
                                                                    )
                                              ]
                                            )
                             ] .

ns:hasCalendarBusy  a     owl:ObjectProperty ;
        rdfs:comment      "To specify the busy time associated with the object. (Was called FBURL in RFC6350)"@en ;
        rdfs:isDefinedBy  <http://www.w3.org/2006/vcard/ns> ;
        rdfs:label        "has calendar busy"@en .

ns:hasCalendarRequest
        a                 owl:ObjectProperty ;
        rdfs:comment      "To specify the calendar user address to which a scheduling request be sent for the object. (Was called CALADRURI in RFC6350)"@en ;
        rdfs:isDefinedBy  <http://www.w3.org/2006/vcard/ns> ;
        rdfs:label        "has calendar request"@en .

foaf:knows  a             owl:ObjectProperty , rdf:Property ;
        rdfs:comment      "A person known by this person (indicating some level of reciprocated interaction between the parties)." ;
        rdfs:domain       foaf:Person ;
        rdfs:isDefinedBy  foaf: ;
        rdfs:label        "knows" ;
        rdfs:range        foaf:Person ;
        ns2:term_status   "stable" .

foaf:firstName  a         owl:DatatypeProperty , rdf:Property ;
        rdfs:comment      "The first name of a person." ;
        rdfs:domain       foaf:Person ;
        rdfs:isDefinedBy  foaf: ;
        rdfs:label        "firstName" ;
        rdfs:range        rdfs:Literal ;
        ns2:term_status   "testing" .

foaf:icqChatID  a           owl:InverseFunctionalProperty , rdf:Property , owl:DatatypeProperty ;
        rdfs:comment        "An ICQ chat ID" ;
        rdfs:domain         foaf:Agent ;
        rdfs:isDefinedBy    foaf: ;
        rdfs:label          "ICQ chat ID" ;
        rdfs:range          rdfs:Literal ;
        rdfs:subPropertyOf  foaf:nick ;
        ns2:term_status     "testing" .

foaf:birthday  a          owl:DatatypeProperty , owl:FunctionalProperty , rdf:Property ;
        rdfs:comment      "The birthday of this Agent, represented in mm-dd string form, eg. '12-31'." ;
        rdfs:domain       foaf:Agent ;
        rdfs:isDefinedBy  foaf: ;
        rdfs:label        "birthday" ;
        rdfs:range        rdfs:Literal ;
        ns2:term_status   "unstable" .

foaf:givenname  a         owl:DatatypeProperty , rdf:Property ;
        rdfs:comment      "The given name of some person." ;
        rdfs:isDefinedBy  foaf: ;
        rdfs:label        "Given name" ;
        ns2:term_status   "archaic" .

foaf:focus  a             owl:ObjectProperty , rdf:Property ;
        rdfs:comment      "The underlying or 'focal' entity associated with some SKOS-described concept." ;
        rdfs:domain       skos:Concept ;
        rdfs:isDefinedBy  foaf: ;
        rdfs:label        "focus" ;
        rdfs:range        owl:Thing ;
        ns2:term_status   "testing" .

foaf:phone  a             owl:ObjectProperty , rdf:Property ;
        rdfs:comment      "A phone, specified using fully qualified tel: URI scheme (refs: http://www.w3.org/Addressing/schemes.html#tel)." ;
        rdfs:isDefinedBy  foaf: ;
        rdfs:label        "phone" ;
        ns2:term_status   "testing" .

foaf:accountServiceHomepage
        a                 owl:ObjectProperty , rdf:Property ;
        rdfs:comment      "Indicates a homepage of the service provide for this online account." ;
        rdfs:domain       foaf:OnlineAccount ;
        rdfs:isDefinedBy  foaf: ;
        rdfs:label        "account service homepage" ;
        rdfs:range        foaf:Document ;
        ns2:term_status   "testing" .

foaf:openid  a              owl:ObjectProperty , rdf:Property , owl:InverseFunctionalProperty ;
        rdfs:comment        "An OpenID for an Agent." ;
        rdfs:domain         foaf:Agent ;
        rdfs:isDefinedBy    foaf: ;
        rdfs:label          "openid" ;
        rdfs:range          foaf:Document ;
        rdfs:subPropertyOf  foaf:isPrimaryTopicOf ;
        ns2:term_status     "testing" .

foaf:isPrimaryTopicOf
        a                   owl:InverseFunctionalProperty , rdf:Property ;
        rdfs:comment        "A document that this thing is the primary topic of." ;
        rdfs:domain         owl:Thing ;
        rdfs:isDefinedBy    foaf: ;
        rdfs:label          "is primary topic of" ;
        rdfs:range          foaf:Document ;
        rdfs:subPropertyOf  foaf:page ;
        owl:inverseOf       foaf:primaryTopic ;
        ns2:term_status     "stable" .

foaf:givenName  a         owl:DatatypeProperty , rdf:Property ;
        rdfs:comment      "The given name of some person." ;
        rdfs:isDefinedBy  foaf: ;
        rdfs:label        "Given name" ;
        ns2:term_status   "testing" .

foaf:depicts  a           owl:ObjectProperty , rdf:Property ;
        rdfs:comment      "A thing depicted in this representation." ;
        rdfs:domain       foaf:Image ;
        rdfs:isDefinedBy  foaf: ;
        rdfs:label        "depicts" ;
        rdfs:range        owl:Thing ;
        owl:inverseOf     foaf:depiction ;
        ns2:term_status   "testing" .

foaf:Project  a           owl:Class , rdfs:Class ;
        rdfs:comment      "A project (a collective endeavour of some kind)." ;
        rdfs:isDefinedBy  foaf: ;
        rdfs:label        "Project" ;
        owl:disjointWith  foaf:Document , foaf:Person ;
        ns2:term_status   "testing" .

foaf:account  a           owl:ObjectProperty , rdf:Property ;
        rdfs:comment      "Indicates an account held by this agent." ;
        rdfs:domain       foaf:Agent ;
        rdfs:isDefinedBy  foaf: ;
        rdfs:label        "account" ;
        rdfs:range        foaf:OnlineAccount ;
        ns2:term_status   "testing" .

foaf:skypeID  a             owl:DatatypeProperty , rdf:Property ;
        rdfs:comment        "A Skype ID" ;
        rdfs:domain         foaf:Agent ;
        rdfs:isDefinedBy    foaf: ;
        rdfs:label          "Skype ID" ;
        rdfs:range          rdfs:Literal ;
        rdfs:subPropertyOf  foaf:nick ;
        ns2:term_status     "testing" .

foaf:Image  a             owl:Class , rdfs:Class ;
        rdfs:comment      "An image." ;
        rdfs:isDefinedBy  foaf: ;
        rdfs:label        "Image" ;
        rdfs:subClassOf   foaf:Document ;
        ns2:term_status   "testing" .

foaf:page  a              owl:ObjectProperty , rdf:Property ;
        rdfs:comment      "A page or document about this thing." ;
        rdfs:domain       owl:Thing ;
        rdfs:isDefinedBy  foaf: ;
        rdfs:label        "page" ;
        rdfs:range        foaf:Document ;
        owl:inverseOf     foaf:topic ;
        ns2:term_status   "testing" .

foaf:OnlineEcommerceAccount
        a                 owl:Class , rdfs:Class ;
        rdfs:comment      "An online e-commerce account." ;
        rdfs:isDefinedBy  foaf: ;
        rdfs:label        "Online E-commerce Account" ;
        rdfs:subClassOf   foaf:OnlineAccount ;
        ns2:term_status   "unstable" .

foaf:lastName  a          owl:DatatypeProperty , rdf:Property ;
        rdfs:comment      "The last name of a person." ;
        rdfs:domain       foaf:Person ;
        rdfs:isDefinedBy  foaf: ;
        rdfs:label        "lastName" ;
        rdfs:range        rdfs:Literal ;
        ns2:term_status   "testing" .

foaf:yahooChatID  a         owl:DatatypeProperty , rdf:Property , owl:InverseFunctionalProperty ;
        rdfs:comment        "A Yahoo chat ID" ;
        rdfs:domain         foaf:Agent ;
        rdfs:isDefinedBy    foaf: ;
        rdfs:label          "Yahoo chat ID" ;
        rdfs:range          rdfs:Literal ;
        rdfs:subPropertyOf  foaf:nick ;
        ns2:term_status     "testing" .

foaf:membershipClass  a   owl:AnnotationProperty , rdf:Property ;
        rdfs:comment      "Indicates the class of individuals that are a member of a Group" ;
        rdfs:isDefinedBy  foaf: ;
        rdfs:label        "membershipClass" ;
        ns2:term_status   "unstable" .

foaf:topic_interest  a    owl:ObjectProperty , rdf:Property ;
        rdfs:comment      "A thing of interest to this person." ;
        rdfs:domain       foaf:Agent ;
        rdfs:isDefinedBy  foaf: ;
        rdfs:label        "topic_interest" ;
        rdfs:range        owl:Thing ;
        ns2:term_status   "testing" .

foaf:dnaChecksum  a       owl:DatatypeProperty , rdf:Property ;
        rdfs:comment      "A checksum for the DNA of some thing. Joke." ;
        rdfs:isDefinedBy  foaf: ;
        rdfs:label        "DNA checksum" ;
        rdfs:range        rdfs:Literal ;
        ns2:term_status   "archaic" .

foaf:gender  a            owl:DatatypeProperty , owl:FunctionalProperty , rdf:Property ;
        rdfs:comment      "The gender of this Agent (typically but not necessarily 'male' or 'female')." ;
        rdfs:domain       foaf:Agent ;
        rdfs:isDefinedBy  foaf: ;
        rdfs:label        "gender" ;
        rdfs:range        rdfs:Literal ;
        ns2:term_status   "testing" .

foaf:mbox_sha1sum  a      owl:DatatypeProperty , owl:InverseFunctionalProperty , rdf:Property ;
        rdfs:comment      "The sha1sum of the URI of an Internet mailbox associated with exactly one owner, the first owner of the mailbox." ;
        rdfs:domain       foaf:Agent ;
        rdfs:isDefinedBy  foaf: ;
        rdfs:label        "sha1sum of a personal mailbox URI name" ;
        rdfs:range        rdfs:Literal ;
        ns2:term_status   "testing" .

foaf:img  a                 owl:ObjectProperty , rdf:Property ;
        rdfs:comment        "An image that can be used to represent some thing (ie. those depictions which are particularly representative of something, eg. one's photo on a homepage)." ;
        rdfs:domain         foaf:Person ;
        rdfs:isDefinedBy    foaf: ;
        rdfs:label          "image" ;
        rdfs:range          foaf:Image ;
        rdfs:subPropertyOf  foaf:depiction ;
        ns2:term_status     "testing" .

foaf:fundedBy  a          owl:ObjectProperty , rdf:Property ;
        rdfs:comment      "An organization funding a project or person." ;
        rdfs:domain       owl:Thing ;
        rdfs:isDefinedBy  foaf: ;
        rdfs:label        "funded by" ;
        rdfs:range        owl:Thing ;
        ns2:term_status   "archaic" .

foaf:interest  a          owl:ObjectProperty , rdf:Property ;
        rdfs:comment      "A page about a topic of interest to this person." ;
        rdfs:domain       foaf:Agent ;
        rdfs:isDefinedBy  foaf: ;
        rdfs:label        "interest" ;
        rdfs:range        foaf:Document ;
        ns2:term_status   "testing" .

foaf:familyName  a        owl:DatatypeProperty , rdf:Property ;
        rdfs:comment      "The family name of some person." ;
        rdfs:domain       foaf:Person ;
        rdfs:isDefinedBy  foaf: ;
        rdfs:label        "familyName" ;
        rdfs:range        rdfs:Literal ;
        ns2:term_status   "testing" .

foaf:status  a            owl:DatatypeProperty , rdf:Property ;
        rdfs:comment      "A string expressing what the user is happy for the general public (normally) to know about their current activity." ;
        rdfs:domain       foaf:Agent ;
        rdfs:isDefinedBy  foaf: ;
        rdfs:label        "status" ;
        rdfs:range        rdfs:Literal ;
        ns2:term_status   "unstable" .

foaf:msnChatID  a           owl:InverseFunctionalProperty , rdf:Property , owl:DatatypeProperty ;
        rdfs:comment        "An MSN chat ID" ;
        rdfs:domain         foaf:Agent ;
        rdfs:isDefinedBy    foaf: ;
        rdfs:label          "MSN chat ID" ;
        rdfs:range          rdfs:Literal ;
        rdfs:subPropertyOf  foaf:nick ;
        ns2:term_status     "testing" .

foaf:sha1  a              owl:DatatypeProperty , rdf:Property ;
        rdfs:comment      "A sha1sum hash, in hex." ;
        rdfs:domain       foaf:Document ;
        rdfs:isDefinedBy  foaf: ;
        rdfs:label        "sha1sum (hex)" ;
        ns2:term_status   "unstable" .

foaf:PersonalProfileDocument
        a                 owl:Class , rdfs:Class ;
        rdfs:comment      "A personal profile RDF document." ;
        rdfs:isDefinedBy  foaf: ;
        rdfs:label        "PersonalProfileDocument" ;
        rdfs:subClassOf   foaf:Document ;
        ns2:term_status   "testing" .

foaf:workInfoHomepage
        a                 owl:ObjectProperty , rdf:Property ;
        rdfs:comment      "A work info homepage of some person; a page about their work for some organization." ;
        rdfs:domain       foaf:Person ;
        rdfs:isDefinedBy  foaf: ;
        rdfs:label        "work info homepage" ;
        rdfs:range        foaf:Document ;
        ns2:term_status   "testing" .

foaf:currentProject  a    owl:ObjectProperty , rdf:Property ;
        rdfs:comment      "A current project this person works on." ;
        rdfs:domain       foaf:Person ;
        rdfs:isDefinedBy  foaf: ;
        rdfs:label        "current project" ;
        rdfs:range        owl:Thing ;
        ns2:term_status   "testing" .

foaf:mbox  a              owl:ObjectProperty , owl:InverseFunctionalProperty , rdf:Property ;
        rdfs:comment      "A personal mailbox, ie. an Internet mailbox associated with exactly one owner, the first owner of this mailbox. This is a 'static inverse functional property', in that there is (across time and change) at most one individual that ever has any particular value for foaf:mbox." ;
        rdfs:domain       foaf:Agent ;
        rdfs:isDefinedBy  foaf: ;
        rdfs:label        "personal mailbox" ;
        rdfs:range        owl:Thing ;
        ns2:term_status   "stable" .

foaf:schoolHomepage  a    owl:ObjectProperty , rdf:Property ;
        rdfs:comment      "A homepage of a school attended by the person." ;
        rdfs:domain       foaf:Person ;
        rdfs:isDefinedBy  foaf: ;
        rdfs:label        "schoolHomepage" ;
        rdfs:range        foaf:Document ;
        ns2:term_status   "testing" .

foaf:   a               owl:Ontology ;
        dc:description  "The Friend of a Friend (FOAF) RDF vocabulary, described using W3C RDF Schema and the Web Ontology Language." ;
        dc:title        "Friend of a Friend (FOAF) vocabulary" .

foaf:Organization  a      owl:Class , rdfs:Class ;
        rdfs:comment      "An organization." ;
        rdfs:isDefinedBy  foaf: ;
        rdfs:label        "Organization" ;
        rdfs:subClassOf   foaf:Agent ;
        owl:disjointWith  foaf:Document , foaf:Person ;
        ns2:term_status   "stable" .

foaf:maker  a                   rdf:Property , owl:ObjectProperty ;
        rdfs:comment            "An agent that made this thing." ;
        rdfs:domain             owl:Thing ;
        rdfs:isDefinedBy        foaf: ;
        rdfs:label              "maker" ;
        rdfs:range              foaf:Agent ;
        owl:equivalentProperty  dcterms:creator ;
        owl:inverseOf           foaf:made ;
        ns2:term_status         "stable" .

foaf:holdsAccount  a      owl:ObjectProperty , rdf:Property ;
        rdfs:comment      "Indicates an account held by this agent." ;
        rdfs:domain       foaf:Agent ;
        rdfs:isDefinedBy  foaf: ;
        rdfs:label        "account" ;
        rdfs:range        foaf:OnlineAccount ;
        ns2:term_status   "archaic" .

foaf:pastProject  a       owl:ObjectProperty , rdf:Property ;
        rdfs:comment      "A project this person has previously worked on." ;
        rdfs:domain       foaf:Person ;
        rdfs:isDefinedBy  foaf: ;
        rdfs:label        "past project" ;
        rdfs:range        owl:Thing ;
        ns2:term_status   "testing" .

foaf:jabberID  a          owl:InverseFunctionalProperty , owl:DatatypeProperty , rdf:Property ;
        rdfs:comment      "A jabber ID for something." ;
        rdfs:domain       foaf:Agent ;
        rdfs:isDefinedBy  foaf: ;
        rdfs:label        "jabber ID" ;
        rdfs:range        rdfs:Literal ;
        ns2:term_status   "testing" .

foaf:OnlineChatAccount
        a                 owl:Class , rdfs:Class ;
        rdfs:comment      "An online chat account." ;
        rdfs:isDefinedBy  foaf: ;
        rdfs:label        "Online Chat Account" ;
        rdfs:subClassOf   foaf:OnlineAccount ;
        ns2:term_status   "unstable" .

foaf:accountName  a       owl:DatatypeProperty , rdf:Property ;
        rdfs:comment      "Indicates the name (identifier) associated with this online account." ;
        rdfs:domain       foaf:OnlineAccount ;
        rdfs:isDefinedBy  foaf: ;
        rdfs:label        "account name" ;
        rdfs:range        rdfs:Literal ;
        ns2:term_status   "testing" .

foaf:name  a                owl:DatatypeProperty , rdf:Property ;
        rdfs:comment        "A name for some thing." ;
        rdfs:domain         owl:Thing ;
        rdfs:isDefinedBy    foaf: ;
        rdfs:label          "name" ;
        rdfs:range          rdfs:Literal ;
        rdfs:subPropertyOf  rdfs:label ;
        ns2:term_status     "testing" .

foaf:OnlineAccount  a     owl:Class , rdfs:Class ;
        rdfs:comment      "An online account." ;
        rdfs:isDefinedBy  foaf: ;
        rdfs:label        "Online Account" ;
        rdfs:subClassOf   owl:Thing ;
        ns2:term_status   "testing" .

foaf:tipjar  a              owl:ObjectProperty , rdf:Property ;
        rdfs:comment        "A tipjar document for this agent, describing means for payment and reward." ;
        rdfs:domain         foaf:Agent ;
        rdfs:isDefinedBy    foaf: ;
        rdfs:label          "tipjar" ;
        rdfs:range          foaf:Document ;
        rdfs:subPropertyOf  foaf:page ;
        ns2:term_status     "testing" .

foaf:myersBriggs  a       owl:DatatypeProperty , rdf:Property ;
        rdfs:comment      "A Myers Briggs (MBTI) personality classification." ;
        rdfs:domain       foaf:Person ;
        rdfs:isDefinedBy  foaf: ;
        rdfs:label        "myersBriggs" ;
        rdfs:range        rdfs:Literal ;
        ns2:term_status   "testing" .

foaf:age  a               owl:DatatypeProperty , owl:FunctionalProperty , rdf:Property ;
        rdfs:comment      "The age in years of some agent." ;
        rdfs:domain       foaf:Agent ;
        rdfs:isDefinedBy  foaf: ;
        rdfs:label        "age" ;
        rdfs:range        rdfs:Literal ;
        ns2:term_status   "unstable" .

foaf:Agent  a                rdfs:Class , owl:Class ;
        rdfs:comment         "An agent (eg. person, group, software or physical artifact)." ;
        rdfs:isDefinedBy     foaf: ;
        rdfs:label           "Agent" ;
        owl:equivalentClass  dcterms:Agent ;
        ns2:term_status      "stable" .

foaf:OnlineGamingAccount
        a                 owl:Class , rdfs:Class ;
        rdfs:comment      "An online gaming account." ;
        rdfs:isDefinedBy  foaf: ;
        rdfs:label        "Online Gaming Account" ;
        rdfs:subClassOf   foaf:OnlineAccount ;
        ns2:term_status   "unstable" .

foaf:workplaceHomepage
        a                 owl:ObjectProperty , rdf:Property ;
        rdfs:comment      "A workplace homepage of some person; the homepage of an organization they work for." ;
        rdfs:domain       foaf:Person ;
        rdfs:isDefinedBy  foaf: ;
        rdfs:label        "workplace homepage" ;
        rdfs:range        foaf:Document ;
        ns2:term_status   "testing" .

foaf:weblog  a              rdf:Property , owl:InverseFunctionalProperty , owl:ObjectProperty ;
        rdfs:comment        "A weblog of some thing (whether person, group, company etc.)." ;
        rdfs:domain         foaf:Agent ;
        rdfs:isDefinedBy    foaf: ;
        rdfs:label          "weblog" ;
        rdfs:range          foaf:Document ;
        rdfs:subPropertyOf  foaf:page ;
        ns2:term_status     "testing" .

foaf:title  a             owl:DatatypeProperty , rdf:Property ;
        rdfs:comment      "Title (Mr, Mrs, Ms, Dr. etc)" ;
        rdfs:isDefinedBy  foaf: ;
        rdfs:label        "title" ;
        ns2:term_status   "testing" .

foaf:thumbnail  a         owl:ObjectProperty , rdf:Property ;
        rdfs:comment      "A derived thumbnail image." ;
        rdfs:domain       foaf:Image ;
        rdfs:isDefinedBy  foaf: ;
        rdfs:label        "thumbnail" ;
        rdfs:range        foaf:Image ;
        ns2:term_status   "testing" .

foaf:made  a              owl:ObjectProperty , rdf:Property ;
        rdfs:comment      "Something that was made by this agent." ;
        rdfs:domain       foaf:Agent ;
        rdfs:isDefinedBy  foaf: ;
        rdfs:label        "made" ;
        rdfs:range        owl:Thing ;
        owl:inverseOf     foaf:maker ;
        ns2:term_status   "stable" .

foaf:LabelProperty  a     owl:Class , rdfs:Class ;
        rdfs:comment      "A foaf:LabelProperty is any RDF property with texual values that serve as labels." ;
        rdfs:isDefinedBy  foaf: ;
        rdfs:label        "Label Property" ;
        ns2:term_status   "unstable" .

foaf:nick  a              owl:DatatypeProperty , rdf:Property ;
        rdfs:comment      "A short informal nickname characterising an agent (includes login identifiers, IRC and other chat nicknames)." ;
        rdfs:isDefinedBy  foaf: ;
        rdfs:label        "nickname" ;
        ns2:term_status   "testing" .

foaf:based_near  a        owl:ObjectProperty , rdf:Property ;
        rdfs:comment      "A location that something is based near, for some broadly human notion of near." ;
        rdfs:domain       <http://www.w3.org/2003/01/geo/wgs84_pos#SpatialThing> ;
        rdfs:isDefinedBy  foaf: ;
        rdfs:label        "based near" ;
        rdfs:range        <http://www.w3.org/2003/01/geo/wgs84_pos#SpatialThing> ;
        ns2:term_status   "testing" .

foaf:surname  a           owl:DatatypeProperty , rdf:Property ;
        rdfs:comment      "The surname of some person." ;
        rdfs:domain       foaf:Person ;
        rdfs:isDefinedBy  foaf: ;
        rdfs:label        "Surname" ;
        rdfs:range        rdfs:Literal ;
        ns2:term_status   "archaic" .

foaf:plan  a              owl:DatatypeProperty , rdf:Property ;
        rdfs:comment      "A .plan comment, in the tradition of finger and '.plan' files." ;
        rdfs:domain       foaf:Person ;
        rdfs:isDefinedBy  foaf: ;
        rdfs:label        "plan" ;
        rdfs:range        rdfs:Literal ;
        ns2:term_status   "testing" .

foaf:aimChatID  a           rdf:Property , owl:DatatypeProperty , owl:InverseFunctionalProperty ;
        rdfs:comment        "An AIM chat ID" ;
        rdfs:domain         foaf:Agent ;
        rdfs:isDefinedBy    foaf: ;
        rdfs:label          "AIM chat ID" ;
        rdfs:range          rdfs:Literal ;
        rdfs:subPropertyOf  foaf:nick ;
        ns2:term_status     "testing" .

foaf:Group  a             owl:Class , rdfs:Class ;
        rdfs:comment      "A class of Agents." ;
        rdfs:isDefinedBy  foaf: ;
        rdfs:label        "Group" ;
        rdfs:subClassOf   foaf:Agent ;
        ns2:term_status   "stable" .

foaf:geekcode  a          owl:DatatypeProperty , rdf:Property ;
        rdfs:comment      "A textual geekcode for this person, see http://www.geekcode.com/geek.html" ;
        rdfs:domain       foaf:Person ;
        rdfs:isDefinedBy  foaf: ;
        rdfs:label        "geekcode" ;
        rdfs:range        rdfs:Literal ;
        ns2:term_status   "archaic" .

foaf:topic  a             owl:ObjectProperty , rdf:Property ;
        rdfs:comment      "A topic of some page or document." ;
        rdfs:domain       foaf:Document ;
        rdfs:isDefinedBy  foaf: ;
        rdfs:label        "topic" ;
        rdfs:range        owl:Thing ;
        owl:inverseOf     foaf:page ;
        ns2:term_status   "testing" .

foaf:theme  a             owl:ObjectProperty , rdf:Property ;
        rdfs:comment      "A theme." ;
        rdfs:domain       owl:Thing ;
        rdfs:isDefinedBy  foaf: ;
        rdfs:label        "theme" ;
        rdfs:range        owl:Thing ;
        ns2:term_status   "archaic" .

foaf:publications  a      owl:ObjectProperty , rdf:Property ;
        rdfs:comment      "A link to the publications of this person." ;
        rdfs:domain       foaf:Person ;
        rdfs:isDefinedBy  foaf: ;
        rdfs:label        "publications" ;
        rdfs:range        foaf:Document ;
        ns2:term_status   "testing" .
